<?xml version="1.0"?>
<rdf:RDF xmlns="http://example.org/virtualhome2kg/ontology/"
     xml:base="http://example.org/virtualhome2kg/ontology/"
     xmlns:owl="http://www.w3.org/2002/07/owl#"
     xmlns:rdf="http://www.w3.org/1999/02/22-rdf-syntax-ns#"
     xmlns:xml="http://www.w3.org/XML/1998/namespace"
     xmlns:xsd="http://www.w3.org/2001/XMLSchema#"
     xmlns:rdfs="http://www.w3.org/2000/01/rdf-schema#"
     xmlns:skos="http://www.w3.org/2004/02/skos/core#"
     xmlns:swrla="http://swrl.stanford.edu/ontologies/3.3/swrla.owl#"
     xmlns:terms="http://purl.org/dc/terms/">
    <owl:Ontology rdf:about="http://example.org/virtualhome2kg/ontology/">
        <rdfs:comment>This ontology offers vocabularies for representing activities of daily living (ADL) that can be run in the VirtualHome (http://virtual-home.org/), run-time home situations, objects, and relationships among them.
This ontology is an extended version of the HomeOntology (https://github.com/valexande/HomeOntology).</rdfs:comment>
    </owl:Ontology>
    


    <!-- 
    ///////////////////////////////////////////////////////////////////////////////////////
    //
    // Annotation properties
    //
    ///////////////////////////////////////////////////////////////////////////////////////
     -->


    


    <!-- http://purl.org/dc/terms/description -->


    <owl:AnnotationProperty rdf:about="http://purl.org/dc/terms/description"/>
    


    <!-- http://swrl.stanford.edu/ontologies/3.3/swrla.owl#isRuleEnabled -->


    <owl:AnnotationProperty rdf:about="http://swrl.stanford.edu/ontologies/3.3/swrla.owl#isRuleEnabled"/>
    


    <!-- http://www.w3.org/2004/02/skos/core#closeMatch -->


    <owl:AnnotationProperty rdf:about="http://www.w3.org/2004/02/skos/core#closeMatch"/>
    


    <!-- 
    ///////////////////////////////////////////////////////////////////////////////////////
    //
    // Datatypes
    //
    ///////////////////////////////////////////////////////////////////////////////////////
     -->


    


    <!-- https://www.web3d.org/specifications/X3dOntology4.0#SFDouble -->


    <rdfs:Datatype rdf:about="https://www.web3d.org/specifications/X3dOntology4.0#SFDouble"/>
    


    <!-- https://www.web3d.org/specifications/X3dOntology4.0#SFVec3f -->


    <rdfs:Datatype rdf:about="https://www.web3d.org/specifications/X3dOntology4.0#SFVec3f"/>
    


    <!-- 
    ///////////////////////////////////////////////////////////////////////////////////////
    //
    // Object Properties
    //
    ///////////////////////////////////////////////////////////////////////////////////////
     -->


    


    <!-- http://example.org/virtualhome2kg/ontology/action -->


    <owl:ObjectProperty rdf:about="http://example.org/virtualhome2kg/ontology/action">
        <rdfs:domain rdf:resource="http://example.org/virtualhome2kg/ontology/Event"/>
        <rdfs:range rdf:resource="http://example.org/virtualhome2kg/ontology/Action"/>
    </owl:ObjectProperty>
    


    <!-- http://example.org/virtualhome2kg/ontology/activity -->


    <owl:ObjectProperty rdf:about="http://example.org/virtualhome2kg/ontology/activity">
        <rdfs:domain rdf:resource="http://plod.info/rdf/Episode"/>
        <rdfs:range rdf:resource="http://www.owl-ontologies.com/VirtualHome.owl#Activity"/>
    </owl:ObjectProperty>
    


    <!-- http://example.org/virtualhome2kg/ontology/affords -->


    <owl:ObjectProperty rdf:about="http://example.org/virtualhome2kg/ontology/affords">
        <rdfs:domain rdf:resource="http://example.org/virtualhome2kg/ontology/Object"/>
        <rdfs:range rdf:resource="http://example.org/virtualhome2kg/ontology/Action"/>
    </owl:ObjectProperty>
    


    <!-- http://example.org/virtualhome2kg/ontology/agent -->


    <owl:ObjectProperty rdf:about="http://example.org/virtualhome2kg/ontology/agent">
        <rdfs:domain rdf:resource="http://example.org/virtualhome2kg/ontology/Event"/>
        <rdfs:range rdf:resource="http://example.org/virtualhome2kg/ontology/Character"/>
        <skos:closeMatch rdf:resource="http://purl.org/NET/c4dm/event.owl#agent"/>
    </owl:ObjectProperty>
    


    <!-- http://example.org/virtualhome2kg/ontology/attribute -->


    <owl:ObjectProperty rdf:about="http://example.org/virtualhome2kg/ontology/attribute">
        <rdfs:domain rdf:resource="http://example.org/virtualhome2kg/ontology/Object"/>
        <rdfs:range rdf:resource="http://example.org/virtualhome2kg/ontology/Attribute"/>
    </owl:ObjectProperty>
    


    <!-- http://example.org/virtualhome2kg/ontology/bbox -->


    <owl:ObjectProperty rdf:about="http://example.org/virtualhome2kg/ontology/bbox">
        <owl:inverseOf rdf:resource="http://example.org/virtualhome2kg/ontology/isBboxOf"/>
        <rdfs:domain rdf:resource="http://example.org/virtualhome2kg/ontology/State"/>
        <rdfs:range rdf:resource="https://www.web3d.org/specifications/X3dOntology4.0#Shape"/>
        <rdfs:comment>3D bounding box</rdfs:comment>
    </owl:ObjectProperty>
    


    <!-- http://example.org/virtualhome2kg/ontology/between -->


    <owl:ObjectProperty rdf:about="http://example.org/virtualhome2kg/ontology/between">
        <rdfs:subPropertyOf rdf:resource="http://example.org/virtualhome2kg/ontology/relatedShape"/>
        <rdfs:domain rdf:resource="https://www.web3d.org/specifications/X3dOntology4.0#Shape"/>
        <rdfs:range rdf:resource="https://www.web3d.org/specifications/X3dOntology4.0#Shape"/>
        <rdfs:comment>used for door object, if door is between kitchen and livingroom, we have edges &lt;door, between, livingroom&gt; and &lt;door, between ,kitchen&gt;</rdfs:comment>
    </owl:ObjectProperty>
    


    <!-- http://example.org/virtualhome2kg/ontology/close -->


    <owl:ObjectProperty rdf:about="http://example.org/virtualhome2kg/ontology/close">
        <rdfs:subPropertyOf rdf:resource="http://example.org/virtualhome2kg/ontology/relatedShape"/>
        <rdfs:domain rdf:resource="https://www.web3d.org/specifications/X3dOntology4.0#Shape"/>
        <rdfs:range rdf:resource="https://www.web3d.org/specifications/X3dOntology4.0#Shape"/>
        <rdfs:comment>edge &lt;object1, close, object2&gt; denotes that the distance between center of object1 (object2) to the bounding box of object2 (object1) is &lt; 1.5 units (~meters)</rdfs:comment>
    </owl:ObjectProperty>
    


    <!-- http://example.org/virtualhome2kg/ontology/facing -->


    <owl:ObjectProperty rdf:about="http://example.org/virtualhome2kg/ontology/facing">
        <rdfs:subPropertyOf rdf:resource="http://example.org/virtualhome2kg/ontology/relatedShape"/>
        <rdfs:domain rdf:resource="https://www.web3d.org/specifications/X3dOntology4.0#Shape"/>
        <rdfs:range rdf:resource="https://www.web3d.org/specifications/X3dOntology4.0#Shape"/>
        <rdfs:comment>there is an edge &lt;object1, facing, object2&gt; if object2 is lookable, is visible from object1, and the distance between the centers is &lt; 5 units (~meters). If object1 is a sofa or a chair it should also be turned towards object2</rdfs:comment>
    </owl:ObjectProperty>
    


    <!-- http://example.org/virtualhome2kg/ontology/from -->


    <owl:ObjectProperty rdf:about="http://example.org/virtualhome2kg/ontology/from">
        <rdfs:domain rdf:resource="http://example.org/virtualhome2kg/ontology/Event"/>
        <rdfs:range rdf:resource="http://example.org/virtualhome2kg/ontology/Room"/>
    </owl:ObjectProperty>
    


    <!-- http://example.org/virtualhome2kg/ontology/hasActivity -->


    <owl:ObjectProperty rdf:about="http://example.org/virtualhome2kg/ontology/hasActivity">
        <rdfs:domain rdf:resource="http://plod.info/rdf/Episode"/>
        <rdfs:range rdf:resource="http://www.owl-ontologies.com/VirtualHome.owl#Activity"/>
    </owl:ObjectProperty>
    


    <!-- http://example.org/virtualhome2kg/ontology/hasEvent -->


    <owl:ObjectProperty rdf:about="http://example.org/virtualhome2kg/ontology/hasEvent">
        <rdfs:domain rdf:resource="http://www.owl-ontologies.com/VirtualHome.owl#Activity"/>
        <rdfs:range rdf:resource="http://example.org/virtualhome2kg/ontology/Event"/>
    </owl:ObjectProperty>
    


    <!-- http://example.org/virtualhome2kg/ontology/height -->


    <owl:ObjectProperty rdf:about="http://example.org/virtualhome2kg/ontology/height"/>
    


    <!-- http://example.org/virtualhome2kg/ontology/holds_lh -->


    <owl:ObjectProperty rdf:about="http://example.org/virtualhome2kg/ontology/holds_lh">
        <rdfs:subPropertyOf rdf:resource="http://example.org/virtualhome2kg/ontology/relatedShape"/>
        <rdfs:domain rdf:resource="https://www.web3d.org/specifications/X3dOntology4.0#Shape"/>
        <rdfs:range rdf:resource="https://www.web3d.org/specifications/X3dOntology4.0#Shape"/>
        <rdfs:comment>analogue of holds_rh for left hand</rdfs:comment>
    </owl:ObjectProperty>
    


    <!-- http://example.org/virtualhome2kg/ontology/holds_rh -->


    <owl:ObjectProperty rdf:about="http://example.org/virtualhome2kg/ontology/holds_rh">
        <rdfs:subPropertyOf rdf:resource="http://example.org/virtualhome2kg/ontology/relatedShape"/>
        <rdfs:domain rdf:resource="https://www.web3d.org/specifications/X3dOntology4.0#Shape"/>
        <rdfs:range rdf:resource="https://www.web3d.org/specifications/X3dOntology4.0#Shape"/>
        <rdfs:comment>edge &lt;character, holds_rh, object&gt; is used to indicate that character holds an object in its right hand</rdfs:comment>
    </owl:ObjectProperty>
    


    <!-- http://example.org/virtualhome2kg/ontology/inside -->


    <owl:ObjectProperty rdf:about="http://example.org/virtualhome2kg/ontology/inside">
        <rdfs:subPropertyOf rdf:resource="http://example.org/virtualhome2kg/ontology/relatedShape"/>
        <rdfs:domain rdf:resource="https://www.web3d.org/specifications/X3dOntology4.0#Shape"/>
        <rdfs:range rdf:resource="https://www.web3d.org/specifications/X3dOntology4.0#Shape"/>
    </owl:ObjectProperty>
    


    <!-- http://example.org/virtualhome2kg/ontology/isBboxOf -->


    <owl:ObjectProperty rdf:about="http://example.org/virtualhome2kg/ontology/isBboxOf">
        <rdfs:domain rdf:resource="https://www.web3d.org/specifications/X3dOntology4.0#Shape"/>
    </owl:ObjectProperty>
    


    <!-- http://example.org/virtualhome2kg/ontology/isStateOf -->


    <owl:ObjectProperty rdf:about="http://example.org/virtualhome2kg/ontology/isStateOf">
        <rdfs:domain rdf:resource="http://example.org/virtualhome2kg/ontology/State"/>
        <rdfs:range rdf:resource="http://example.org/virtualhome2kg/ontology/Object"/>
    </owl:ObjectProperty>
    


    <!-- http://example.org/virtualhome2kg/ontology/mainObject -->


    <owl:ObjectProperty rdf:about="http://example.org/virtualhome2kg/ontology/mainObject">
        <rdfs:subPropertyOf rdf:resource="http://www.owl-ontologies.com/VirtualHome.owl#object"/>
        <rdfs:domain rdf:resource="http://example.org/virtualhome2kg/ontology/Event"/>
        <rdfs:range rdf:resource="http://example.org/virtualhome2kg/ontology/Object"/>
        <rdfs:comment>A main object of an event.
If an agent pours milk into a glass, the value of the mainObject is the milk.</rdfs:comment>
    </owl:ObjectProperty>
    


    <!-- http://example.org/virtualhome2kg/ontology/nextActivity -->


    <owl:ObjectProperty rdf:about="http://example.org/virtualhome2kg/ontology/nextActivity">
        <rdfs:subPropertyOf rdf:resource="http://example.org/virtualhome2kg/ontology/relatedActivity"/>
        <rdfs:domain rdf:resource="http://www.owl-ontologies.com/VirtualHome.owl#Activity"/>
        <rdfs:range rdf:resource="http://www.owl-ontologies.com/VirtualHome.owl#Activity"/>
    </owl:ObjectProperty>
    


    <!-- http://example.org/virtualhome2kg/ontology/nextEvent -->


    <owl:ObjectProperty rdf:about="http://example.org/virtualhome2kg/ontology/nextEvent">
        <rdfs:subPropertyOf rdf:resource="http://example.org/virtualhome2kg/ontology/relatedEvent"/>
        <rdfs:domain rdf:resource="http://example.org/virtualhome2kg/ontology/Event"/>
        <rdfs:range rdf:resource="http://example.org/virtualhome2kg/ontology/Event"/>
    </owl:ObjectProperty>
    


    <!-- http://example.org/virtualhome2kg/ontology/nextSituation -->


    <owl:ObjectProperty rdf:about="http://example.org/virtualhome2kg/ontology/nextSituation">
        <rdfs:subPropertyOf rdf:resource="http://example.org/virtualhome2kg/ontology/relatedSituation"/>
        <owl:inverseOf rdf:resource="http://example.org/virtualhome2kg/ontology/previousSituation"/>
        <rdfs:domain rdf:resource="http://example.org/virtualhome2kg/ontology/Situation"/>
        <rdfs:range rdf:resource="http://example.org/virtualhome2kg/ontology/Situation"/>
    </owl:ObjectProperty>
    


    <!-- http://example.org/virtualhome2kg/ontology/nextState -->


    <owl:ObjectProperty rdf:about="http://example.org/virtualhome2kg/ontology/nextState">
        <rdfs:subPropertyOf rdf:resource="http://example.org/virtualhome2kg/ontology/relatedState"/>
        <owl:inverseOf rdf:resource="http://example.org/virtualhome2kg/ontology/previousState"/>
        <rdfs:domain rdf:resource="http://example.org/virtualhome2kg/ontology/State"/>
        <rdfs:range rdf:resource="http://example.org/virtualhome2kg/ontology/State"/>
    </owl:ObjectProperty>
    


    <!-- http://example.org/virtualhome2kg/ontology/on -->


    <owl:ObjectProperty rdf:about="http://example.org/virtualhome2kg/ontology/on">
        <rdfs:subPropertyOf rdf:resource="http://example.org/virtualhome2kg/ontology/relatedShape"/>
        <rdfs:domain rdf:resource="https://www.web3d.org/specifications/X3dOntology4.0#Shape"/>
        <rdfs:range rdf:resource="https://www.web3d.org/specifications/X3dOntology4.0#Shape"/>
    </owl:ObjectProperty>
    


    <!-- http://example.org/virtualhome2kg/ontology/partOf -->


    <owl:ObjectProperty rdf:about="http://example.org/virtualhome2kg/ontology/partOf">
        <rdfs:domain rdf:resource="http://example.org/virtualhome2kg/ontology/State"/>
        <rdfs:range rdf:resource="http://example.org/virtualhome2kg/ontology/Situation"/>
    </owl:ObjectProperty>
    


    <!-- http://example.org/virtualhome2kg/ontology/place -->


    <owl:ObjectProperty rdf:about="http://example.org/virtualhome2kg/ontology/place">
        <rdfs:domain rdf:resource="http://example.org/virtualhome2kg/ontology/Event"/>
        <rdfs:range rdf:resource="http://example.org/virtualhome2kg/ontology/Room"/>
    </owl:ObjectProperty>
    


    <!-- http://example.org/virtualhome2kg/ontology/previousActivity -->


    <owl:ObjectProperty rdf:about="http://example.org/virtualhome2kg/ontology/previousActivity">
        <rdfs:subPropertyOf rdf:resource="http://example.org/virtualhome2kg/ontology/relatedActivity"/>
    </owl:ObjectProperty>
    


    <!-- http://example.org/virtualhome2kg/ontology/previousEvent -->


    <owl:ObjectProperty rdf:about="http://example.org/virtualhome2kg/ontology/previousEvent">
        <rdfs:subPropertyOf rdf:resource="http://example.org/virtualhome2kg/ontology/relatedEvent"/>
        <rdfs:domain rdf:resource="http://example.org/virtualhome2kg/ontology/Event"/>
        <rdfs:range rdf:resource="http://example.org/virtualhome2kg/ontology/Event"/>
    </owl:ObjectProperty>
    


    <!-- http://example.org/virtualhome2kg/ontology/previousSituation -->


    <owl:ObjectProperty rdf:about="http://example.org/virtualhome2kg/ontology/previousSituation">
        <rdfs:subPropertyOf rdf:resource="http://example.org/virtualhome2kg/ontology/relatedSituation"/>
        <rdfs:domain rdf:resource="http://example.org/virtualhome2kg/ontology/Situation"/>
        <rdfs:range rdf:resource="http://example.org/virtualhome2kg/ontology/Situation"/>
    </owl:ObjectProperty>
    


    <!-- http://example.org/virtualhome2kg/ontology/previousState -->


    <owl:ObjectProperty rdf:about="http://example.org/virtualhome2kg/ontology/previousState">
        <rdfs:subPropertyOf rdf:resource="http://example.org/virtualhome2kg/ontology/relatedState"/>
        <rdfs:domain rdf:resource="http://example.org/virtualhome2kg/ontology/State"/>
        <rdfs:range rdf:resource="http://example.org/virtualhome2kg/ontology/State"/>
    </owl:ObjectProperty>
    


    <!-- http://example.org/virtualhome2kg/ontology/relatedActivity -->


    <owl:ObjectProperty rdf:about="http://example.org/virtualhome2kg/ontology/relatedActivity">
        <rdfs:domain rdf:resource="http://www.owl-ontologies.com/VirtualHome.owl#Activity"/>
        <rdfs:range rdf:resource="http://www.owl-ontologies.com/VirtualHome.owl#Activity"/>
    </owl:ObjectProperty>
    


    <!-- http://example.org/virtualhome2kg/ontology/relatedEvent -->


    <owl:ObjectProperty rdf:about="http://example.org/virtualhome2kg/ontology/relatedEvent">
        <rdfs:domain rdf:resource="http://example.org/virtualhome2kg/ontology/Event"/>
        <rdfs:range rdf:resource="http://example.org/virtualhome2kg/ontology/Event"/>
    </owl:ObjectProperty>
    


    <!-- http://example.org/virtualhome2kg/ontology/relatedShape -->


    <owl:ObjectProperty rdf:about="http://example.org/virtualhome2kg/ontology/relatedShape">
        <rdfs:domain rdf:resource="https://www.web3d.org/specifications/X3dOntology4.0#Shape"/>
        <rdfs:range rdf:resource="https://www.web3d.org/specifications/X3dOntology4.0#Shape"/>
    </owl:ObjectProperty>
    


    <!-- http://example.org/virtualhome2kg/ontology/relatedSituation -->


    <owl:ObjectProperty rdf:about="http://example.org/virtualhome2kg/ontology/relatedSituation">
        <rdfs:domain rdf:resource="http://example.org/virtualhome2kg/ontology/Situation"/>
        <rdfs:range rdf:resource="http://example.org/virtualhome2kg/ontology/Situation"/>
    </owl:ObjectProperty>
    


    <!-- http://example.org/virtualhome2kg/ontology/relatedState -->


    <owl:ObjectProperty rdf:about="http://example.org/virtualhome2kg/ontology/relatedState">
        <rdfs:domain rdf:resource="http://example.org/virtualhome2kg/ontology/State"/>
        <rdfs:range rdf:resource="http://example.org/virtualhome2kg/ontology/State"/>
    </owl:ObjectProperty>
    


    <!-- http://example.org/virtualhome2kg/ontology/situationAfterEvent -->


    <owl:ObjectProperty rdf:about="http://example.org/virtualhome2kg/ontology/situationAfterEvent">
        <rdfs:subPropertyOf rdf:resource="http://example.org/virtualhome2kg/ontology/relatedSituation"/>
        <rdfs:domain rdf:resource="http://example.org/virtualhome2kg/ontology/Event"/>
        <rdfs:range rdf:resource="http://example.org/virtualhome2kg/ontology/Situation"/>
    </owl:ObjectProperty>
    


    <!-- http://example.org/virtualhome2kg/ontology/situationBeforeEvent -->


    <owl:ObjectProperty rdf:about="http://example.org/virtualhome2kg/ontology/situationBeforeEvent">
        <rdfs:subPropertyOf rdf:resource="http://example.org/virtualhome2kg/ontology/relatedSituation"/>
        <rdfs:domain rdf:resource="http://example.org/virtualhome2kg/ontology/Event"/>
        <rdfs:range rdf:resource="http://example.org/virtualhome2kg/ontology/Situation"/>
    </owl:ObjectProperty>
    


    <!-- http://example.org/virtualhome2kg/ontology/state -->


    <owl:ObjectProperty rdf:about="http://example.org/virtualhome2kg/ontology/state">
        <rdfs:domain rdf:resource="http://example.org/virtualhome2kg/ontology/State"/>
        <rdfs:range rdf:resource="http://example.org/virtualhome2kg/ontology/StateType"/>
    </owl:ObjectProperty>
    


    <!-- http://example.org/virtualhome2kg/ontology/targetObject -->


    <owl:ObjectProperty rdf:about="http://example.org/virtualhome2kg/ontology/targetObject">
        <rdfs:subPropertyOf rdf:resource="http://www.owl-ontologies.com/VirtualHome.owl#object"/>
        <rdfs:domain rdf:resource="http://example.org/virtualhome2kg/ontology/Event"/>
        <rdfs:range rdf:resource="http://example.org/virtualhome2kg/ontology/Object"/>
        <rdfs:comment>A target object of an event.
If an agent pours milk into a glass, the value of the value of the targetObject is the glass.</rdfs:comment>
    </owl:ObjectProperty>
    


    <!-- http://example.org/virtualhome2kg/ontology/time -->


    <owl:ObjectProperty rdf:about="http://example.org/virtualhome2kg/ontology/time">
        <rdfs:domain rdf:resource="http://example.org/virtualhome2kg/ontology/Event"/>
        <rdfs:range>
            <owl:Class>
                <owl:unionOf rdf:parseType="Collection">
                    <rdf:Description rdf:about="http://www.w3.org/2006/time#TemporalDuration"/>
                    <rdf:Description rdf:about="http://www.w3.org/2006/time#TemporalEntity"/>
                </owl:unionOf>
            </owl:Class>
        </rdfs:range>
        <skos:closeMatch rdf:resource="http://purl.org/NET/c4dm/event.owl#time"/>
    </owl:ObjectProperty>
    


    <!-- http://example.org/virtualhome2kg/ontology/to -->


    <owl:ObjectProperty rdf:about="http://example.org/virtualhome2kg/ontology/to">
        <rdfs:domain rdf:resource="http://example.org/virtualhome2kg/ontology/Event"/>
        <rdfs:range rdf:resource="http://example.org/virtualhome2kg/ontology/Room"/>
    </owl:ObjectProperty>
    


    <!-- http://example.org/virtualhome2kg/ontology/unit -->


    <owl:ObjectProperty rdf:about="http://example.org/virtualhome2kg/ontology/unit">
        <rdfs:range rdf:resource="http://example.org/virtualhome2kg/ontology/Unit"/>
    </owl:ObjectProperty>
    


    <!-- http://example.org/virtualhome2kg/ontology/virtualHome -->


    <owl:ObjectProperty rdf:about="http://example.org/virtualhome2kg/ontology/virtualHome">
        <rdfs:range rdf:resource="http://example.org/virtualhome2kg/ontology/VirtualHome"/>
    </owl:ObjectProperty>
    


    <!-- http://example.org/virtualhome2kg/ontology/weight -->


    <owl:ObjectProperty rdf:about="http://example.org/virtualhome2kg/ontology/weight"/>
    


    <!-- http://www.owl-ontologies.com/VirtualHome.owl#object -->


    <owl:ObjectProperty rdf:about="http://www.owl-ontologies.com/VirtualHome.owl#object">
        <rdfs:domain rdf:resource="http://example.org/virtualhome2kg/ontology/Event"/>
        <rdfs:range rdf:resource="http://example.org/virtualhome2kg/ontology/Object"/>
    </owl:ObjectProperty>
    


    <!-- http://www.w3.org/2006/time#hasDuration -->


    <owl:ObjectProperty rdf:about="http://www.w3.org/2006/time#hasDuration">
        <rdfs:range rdf:resource="http://www.w3.org/2006/time#Duration"/>
    </owl:ObjectProperty>
    


    <!-- http://www.w3.org/2006/time#unitType -->


    <owl:ObjectProperty rdf:about="http://www.w3.org/2006/time#unitType">
        <rdfs:range rdf:resource="http://www.w3.org/2006/time#TemporalUnit"/>
    </owl:ObjectProperty>
    


    <!-- 
    ///////////////////////////////////////////////////////////////////////////////////////
    //
    // Data properties
    //
    ///////////////////////////////////////////////////////////////////////////////////////
     -->


    


    <!-- http://example.org/virtualhome2kg/ontology/actionNumber -->


    <owl:DatatypeProperty rdf:about="http://example.org/virtualhome2kg/ontology/actionNumber">
        <rdfs:domain rdf:resource="http://example.org/virtualhome2kg/ontology/Action"/>
        <rdfs:range rdf:resource="http://www.w3.org/2001/XMLSchema#int"/>
    </owl:DatatypeProperty>
    


    <!-- http://example.org/virtualhome2kg/ontology/activityNumber -->


    <owl:DatatypeProperty rdf:about="http://example.org/virtualhome2kg/ontology/activityNumber">
        <rdfs:domain rdf:resource="http://www.owl-ontologies.com/VirtualHome.owl#Activity"/>
        <rdfs:range rdf:resource="http://www.w3.org/2001/XMLSchema#int"/>
    </owl:DatatypeProperty>
    


    <!-- http://example.org/virtualhome2kg/ontology/eventNumber -->


    <owl:DatatypeProperty rdf:about="http://example.org/virtualhome2kg/ontology/eventNumber">
        <rdfs:domain rdf:resource="http://example.org/virtualhome2kg/ontology/Event"/>
        <rdfs:range rdf:resource="http://www.w3.org/2001/XMLSchema#int"/>
    </owl:DatatypeProperty>
    


    <!-- http://www.w3.org/1999/02/22-rdf-syntax-ns#first -->


    <owl:DatatypeProperty rdf:about="http://www.w3.org/1999/02/22-rdf-syntax-ns#first"/>
    


    <!-- http://www.w3.org/1999/02/22-rdf-syntax-ns#rest -->


    <owl:DatatypeProperty rdf:about="http://www.w3.org/1999/02/22-rdf-syntax-ns#rest"/>
    


    <!-- http://www.w3.org/1999/02/22-rdf-syntax-ns#value -->


    <owl:DatatypeProperty rdf:about="http://www.w3.org/1999/02/22-rdf-syntax-ns#value"/>
    


    <!-- http://www.w3.org/2006/time#numericDuration -->


    <owl:DatatypeProperty rdf:about="http://www.w3.org/2006/time#numericDuration">
        <rdfs:range rdf:resource="http://www.w3.org/2001/XMLSchema#decimal"/>
    </owl:DatatypeProperty>
    


    <!-- https://www.web3d.org/specifications/X3dOntology4.0#bboxCenter -->


    <owl:DatatypeProperty rdf:about="https://www.web3d.org/specifications/X3dOntology4.0#bboxCenter">
        <rdfs:domain rdf:resource="https://www.web3d.org/specifications/X3dOntology4.0#Shape"/>
        <rdfs:range rdf:resource="https://www.web3d.org/specifications/X3dOntology4.0#SFVec3f"/>
    </owl:DatatypeProperty>
    


    <!-- https://www.web3d.org/specifications/X3dOntology4.0#bboxSize -->


    <owl:DatatypeProperty rdf:about="https://www.web3d.org/specifications/X3dOntology4.0#bboxSize">
        <rdfs:domain rdf:resource="https://www.web3d.org/specifications/X3dOntology4.0#Shape"/>
        <rdfs:range rdf:resource="https://www.web3d.org/specifications/X3dOntology4.0#SFVec3f"/>
    </owl:DatatypeProperty>
    


    <!-- 
    ///////////////////////////////////////////////////////////////////////////////////////
    //
    // Classes
    //
    ///////////////////////////////////////////////////////////////////////////////////////
     -->


    


    <!-- http://example.org/virtualhome2kg/ontology/Action -->


    <owl:Class rdf:about="http://example.org/virtualhome2kg/ontology/Action"/>
    


    <!-- http://example.org/virtualhome2kg/ontology/Attribute -->


    <owl:Class rdf:about="http://example.org/virtualhome2kg/ontology/Attribute"/>
    


    <!-- http://example.org/virtualhome2kg/ontology/Back_Porch -->


    <owl:Class rdf:about="http://example.org/virtualhome2kg/ontology/Back_Porch">
        <rdfs:subClassOf rdf:resource="http://example.org/virtualhome2kg/ontology/Room"/>
    </owl:Class>
    


    <!-- http://example.org/virtualhome2kg/ontology/Backyard -->


    <owl:Class rdf:about="http://example.org/virtualhome2kg/ontology/Backyard">
        <rdfs:subClassOf rdf:resource="http://example.org/virtualhome2kg/ontology/Room"/>
    </owl:Class>
    


    <!-- http://example.org/virtualhome2kg/ontology/Bathroom -->


    <owl:Class rdf:about="http://example.org/virtualhome2kg/ontology/Bathroom">
        <rdfs:subClassOf rdf:resource="http://example.org/virtualhome2kg/ontology/Room"/>
    </owl:Class>
    


    <!-- http://example.org/virtualhome2kg/ontology/Bedroom -->


    <owl:Class rdf:about="http://example.org/virtualhome2kg/ontology/Bedroom">
        <rdfs:subClassOf rdf:resource="http://example.org/virtualhome2kg/ontology/Room"/>
    </owl:Class>
    


    <!-- http://example.org/virtualhome2kg/ontology/Character -->


    <owl:Class rdf:about="http://example.org/virtualhome2kg/ontology/Character">
        <rdfs:subClassOf rdf:resource="http://example.org/virtualhome2kg/ontology/Object"/>
    </owl:Class>
    


    <!-- http://example.org/virtualhome2kg/ontology/Dining_room -->


    <owl:Class rdf:about="http://example.org/virtualhome2kg/ontology/Dining_room">
        <rdfs:subClassOf rdf:resource="http://example.org/virtualhome2kg/ontology/Room"/>
    </owl:Class>
    


    <!-- http://example.org/virtualhome2kg/ontology/EndEvent -->


    <owl:Class rdf:about="http://example.org/virtualhome2kg/ontology/EndEvent">
        <rdfs:subClassOf rdf:resource="http://example.org/virtualhome2kg/ontology/Event"/>
    </owl:Class>
    


    <!-- http://example.org/virtualhome2kg/ontology/Entrance -->


    <owl:Class rdf:about="http://example.org/virtualhome2kg/ontology/Entrance">
        <rdfs:subClassOf rdf:resource="http://example.org/virtualhome2kg/ontology/Room"/>
    </owl:Class>
    


    <!-- http://example.org/virtualhome2kg/ontology/Event -->


    <owl:Class rdf:about="http://example.org/virtualhome2kg/ontology/Event">
        <skos:closeMatch rdf:resource="http://purl.org/NET/c4dm/event.owl#Event"/>
        <skos:closeMatch rdf:resource="http://semanticweb.cs.vu.nl/2009/11/sem/Event"/>
    </owl:Class>
    


    <!-- http://example.org/virtualhome2kg/ontology/Family_Altar -->


    <owl:Class rdf:about="http://example.org/virtualhome2kg/ontology/Family_Altar">
        <rdfs:subClassOf rdf:resource="http://example.org/virtualhome2kg/ontology/Room"/>
    </owl:Class>
    


    <!-- http://example.org/virtualhome2kg/ontology/Home -->


    <owl:Class rdf:about="http://example.org/virtualhome2kg/ontology/Home">
        <rdfs:subClassOf rdf:resource="http://example.org/virtualhome2kg/ontology/Room"/>
    </owl:Class>
    


    <!-- http://example.org/virtualhome2kg/ontology/Home_office -->


    <owl:Class rdf:about="http://example.org/virtualhome2kg/ontology/Home_office">
        <rdfs:subClassOf rdf:resource="http://example.org/virtualhome2kg/ontology/Room"/>
    </owl:Class>
    


    <!-- http://example.org/virtualhome2kg/ontology/Kitchen -->


    <owl:Class rdf:about="http://example.org/virtualhome2kg/ontology/Kitchen">
        <rdfs:subClassOf rdf:resource="http://example.org/virtualhome2kg/ontology/Room"/>
    </owl:Class>
    


    <!-- http://example.org/virtualhome2kg/ontology/Livingroom -->


    <owl:Class rdf:about="http://example.org/virtualhome2kg/ontology/Livingroom">
        <rdfs:subClassOf rdf:resource="http://example.org/virtualhome2kg/ontology/Room"/>
    </owl:Class>
    


    <!-- http://example.org/virtualhome2kg/ontology/Object -->


    <owl:Class rdf:about="http://example.org/virtualhome2kg/ontology/Object"/>
    


    <!-- http://example.org/virtualhome2kg/ontology/Room -->


    <owl:Class rdf:about="http://example.org/virtualhome2kg/ontology/Room">
        <rdfs:subClassOf rdf:resource="http://example.org/virtualhome2kg/ontology/Object"/>
    </owl:Class>
    


    <!-- http://example.org/virtualhome2kg/ontology/Service_Entrance -->


    <owl:Class rdf:about="http://example.org/virtualhome2kg/ontology/Service_Entrance">
        <rdfs:subClassOf rdf:resource="http://example.org/virtualhome2kg/ontology/Room"/>
    </owl:Class>
    


    <!-- http://example.org/virtualhome2kg/ontology/Situation -->


    <owl:Class rdf:about="http://example.org/virtualhome2kg/ontology/Situation">
        <rdfs:comment>The class which describes the situation of the entire home at a certain moment.</rdfs:comment>
    </owl:Class>
    


    <!-- http://example.org/virtualhome2kg/ontology/Stairs -->


    <owl:Class rdf:about="http://example.org/virtualhome2kg/ontology/Stairs">
        <rdfs:subClassOf rdf:resource="http://example.org/virtualhome2kg/ontology/Room"/>
    </owl:Class>
    


    <!-- http://example.org/virtualhome2kg/ontology/StartEvent -->


    <owl:Class rdf:about="http://example.org/virtualhome2kg/ontology/StartEvent">
        <rdfs:subClassOf rdf:resource="http://example.org/virtualhome2kg/ontology/Event"/>
    </owl:Class>
    


    <!-- http://example.org/virtualhome2kg/ontology/State -->


    <owl:Class rdf:about="http://example.org/virtualhome2kg/ontology/State"/>
    


    <!-- http://example.org/virtualhome2kg/ontology/StateType -->


    <owl:Class rdf:about="http://example.org/virtualhome2kg/ontology/StateType"/>
    


    <!-- http://example.org/virtualhome2kg/ontology/Toilet -->


    <owl:Class rdf:about="http://example.org/virtualhome2kg/ontology/Toilet">
        <rdfs:subClassOf rdf:resource="http://example.org/virtualhome2kg/ontology/Room"/>
    </owl:Class>
    


    <!-- http://example.org/virtualhome2kg/ontology/Unit -->


    <owl:Class rdf:about="http://example.org/virtualhome2kg/ontology/Unit"/>
    


    <!-- http://example.org/virtualhome2kg/ontology/VirtualHome -->


    <owl:Class rdf:about="http://example.org/virtualhome2kg/ontology/VirtualHome"/>
    


    <!-- http://plod.info/rdf/Episode -->


    <owl:Class rdf:about="http://plod.info/rdf/Episode"/>
    


    <!-- http://www.owl-ontologies.com/VirtualHome.owl#Activity -->


    <owl:Class rdf:about="http://www.owl-ontologies.com/VirtualHome.owl#Activity"/>
    


    <!-- http://www.owl-ontologies.com/VirtualHome.owl#BedTimeSleep -->


    <owl:Class rdf:about="http://www.owl-ontologies.com/VirtualHome.owl#BedTimeSleep">
        <owl:equivalentClass>
            <owl:Class>
                <owl:unionOf rdf:parseType="Collection">
                    <owl:Restriction>
                        <owl:onProperty rdf:resource="http://example.org/virtualhome2kg/ontology/hasEvent"/>
                        <owl:someValuesFrom>
                            <owl:Restriction>
                                <owl:onProperty rdf:resource="http://example.org/virtualhome2kg/ontology/action"/>
                                <owl:hasValue rdf:resource="http://example.org/virtualhome2kg/ontology/action/sleep"/>
                            </owl:Restriction>
                        </owl:someValuesFrom>
                    </owl:Restriction>
                    <owl:Restriction>
                        <owl:onProperty rdf:resource="http://example.org/virtualhome2kg/ontology/hasEvent"/>
                        <owl:someValuesFrom>
                            <owl:Restriction>
                                <owl:onProperty rdf:resource="http://example.org/virtualhome2kg/ontology/action"/>
                                <owl:hasValue rdf:resource="http://example.org/virtualhome2kg/ontology/action/wakeUp"/>
                            </owl:Restriction>
                        </owl:someValuesFrom>
                    </owl:Restriction>
                </owl:unionOf>
            </owl:Class>
        </owl:equivalentClass>
        <rdfs:subClassOf rdf:resource="http://www.owl-ontologies.com/VirtualHome.owl#Activity"/>
        <rdfs:comment>Class with sequences for getting ready for the bed, or get ready for 
sleep, or even put the kids to sleep
.</rdfs:comment>
    </owl:Class>
    


    <!-- http://www.owl-ontologies.com/VirtualHome.owl#Dance -->


    <owl:Class rdf:about="http://www.owl-ontologies.com/VirtualHome.owl#Dance">
        <rdfs:subClassOf rdf:resource="http://www.owl-ontologies.com/VirtualHome.owl#Leisure"/>
        <rdfs:comment>The class with sequence of actions for dancing.</rdfs:comment>
    </owl:Class>
    


    <!-- http://www.owl-ontologies.com/VirtualHome.owl#Drink -->


    <owl:Class rdf:about="http://www.owl-ontologies.com/VirtualHome.owl#Drink">
        <rdfs:subClassOf rdf:resource="http://www.owl-ontologies.com/VirtualHome.owl#EatingDrinking"/>
        <rdfs:comment>Class that contains sequences where the goal is for the user to drink 
under different circumstances.</rdfs:comment>
    </owl:Class>
    


    <!-- http://www.owl-ontologies.com/VirtualHome.owl#Eat -->


    <owl:Class rdf:about="http://www.owl-ontologies.com/VirtualHome.owl#Eat">
        <rdfs:subClassOf rdf:resource="http://www.owl-ontologies.com/VirtualHome.owl#EatingDrinking"/>
        <rdfs:comment>Class with subclasses, for eating seqeunces under different 
circumstances.</rdfs:comment>
    </owl:Class>
    


    <!-- http://www.owl-ontologies.com/VirtualHome.owl#EatingDrinking -->


    <owl:Class rdf:about="http://www.owl-ontologies.com/VirtualHome.owl#EatingDrinking">
        <owl:equivalentClass>
            <owl:Class>
                <owl:unionOf rdf:parseType="Collection">
                    <owl:Restriction>
                        <owl:onProperty rdf:resource="http://example.org/virtualhome2kg/ontology/hasEvent"/>
                        <owl:someValuesFrom>
                            <owl:Restriction>
                                <owl:onProperty rdf:resource="http://example.org/virtualhome2kg/ontology/action"/>
                                <owl:hasValue rdf:resource="http://example.org/virtualhome2kg/ontology/action/drink"/>
                            </owl:Restriction>
                        </owl:someValuesFrom>
                    </owl:Restriction>
                    <owl:Restriction>
                        <owl:onProperty rdf:resource="http://example.org/virtualhome2kg/ontology/hasEvent"/>
                        <owl:someValuesFrom>
                            <owl:Restriction>
                                <owl:onProperty rdf:resource="http://example.org/virtualhome2kg/ontology/action"/>
                                <owl:hasValue rdf:resource="http://example.org/virtualhome2kg/ontology/action/eat"/>
                            </owl:Restriction>
                        </owl:someValuesFrom>
                    </owl:Restriction>
                </owl:unionOf>
            </owl:Class>
        </owl:equivalentClass>
        <rdfs:subClassOf rdf:resource="http://www.owl-ontologies.com/VirtualHome.owl#Activity"/>
        <rdfs:comment>Class that contains sequences for eating and drinking.</rdfs:comment>
    </owl:Class>
    


    <!-- http://www.owl-ontologies.com/VirtualHome.owl#FoodPreparation -->


    <owl:Class rdf:about="http://www.owl-ontologies.com/VirtualHome.owl#FoodPreparation">
        <rdfs:subClassOf rdf:resource="http://www.owl-ontologies.com/VirtualHome.owl#Activity"/>
        <rdfs:comment>Class for preparing food, or other kitchen based acitivities for eating 
or drinking (prepeare coffee).</rdfs:comment>
    </owl:Class>
    


    <!-- http://www.owl-ontologies.com/VirtualHome.owl#GettingReady -->


    <owl:Class rdf:about="http://www.owl-ontologies.com/VirtualHome.owl#GettingReady">
        <rdfs:subClassOf rdf:resource="http://www.owl-ontologies.com/VirtualHome.owl#Activity"/>
        <rdfs:comment>Class with sequences for getting ready to go to work, or getting ready 
o perform a task outside the home, or even a procedure that needs prior 
preparation.</rdfs:comment>
    </owl:Class>
    


    <!-- http://www.owl-ontologies.com/VirtualHome.owl#HouseArrangement -->


    <owl:Class rdf:about="http://www.owl-ontologies.com/VirtualHome.owl#HouseArrangement">
        <rdfs:subClassOf rdf:resource="http://www.owl-ontologies.com/VirtualHome.owl#Activity"/>
        <rdfs:comment>Superclass that contains sequence for arrangement tasks inside the house. Some of these classes could have been classified as a House Cleaning subclass. We prefer this hierarchy, because the task are more to the category of organizing object inside a domestic environment, rather than cleaning.</rdfs:comment>
    </owl:Class>
    


    <!-- http://www.owl-ontologies.com/VirtualHome.owl#HouseCleaning -->


    <owl:Class rdf:about="http://www.owl-ontologies.com/VirtualHome.owl#HouseCleaning">
        <rdfs:subClassOf rdf:resource="http://www.owl-ontologies.com/VirtualHome.owl#Activity"/>
        <rdfs:comment>The class that contains sequence of actions, with Cleaning tasks.</rdfs:comment>
    </owl:Class>
    


    <!-- http://www.owl-ontologies.com/VirtualHome.owl#HygieneStyling -->


    <owl:Class rdf:about="http://www.owl-ontologies.com/VirtualHome.owl#HygieneStyling">
        <rdfs:subClassOf rdf:resource="http://www.owl-ontologies.com/VirtualHome.owl#Activity"/>
        <rdfs:comment>Class for sequence that are related to Hygiene otr Styling (NOTICE: some 
of this sequences could be conisdered also as cleaning).</rdfs:comment>
    </owl:Class>
    


    <!-- http://www.owl-ontologies.com/VirtualHome.owl#Laugh -->


    <owl:Class rdf:about="http://www.owl-ontologies.com/VirtualHome.owl#Laugh">
        <rdfs:subClassOf rdf:resource="http://www.owl-ontologies.com/VirtualHome.owl#Other"/>
        <rdfs:comment>The class with sequence of actions for laughing.</rdfs:comment>
    </owl:Class>
    


    <!-- http://www.owl-ontologies.com/VirtualHome.owl#Leisure -->


    <owl:Class rdf:about="http://www.owl-ontologies.com/VirtualHome.owl#Leisure">
        <rdfs:subClassOf rdf:resource="http://www.owl-ontologies.com/VirtualHome.owl#Activity"/>
        <rdfs:comment>Class that contains procedures about leisure</rdfs:comment>
    </owl:Class>
    


    <!-- http://www.owl-ontologies.com/VirtualHome.owl#Other -->


    <owl:Class rdf:about="http://www.owl-ontologies.com/VirtualHome.owl#Other">
        <rdfs:subClassOf rdf:resource="http://www.owl-ontologies.com/VirtualHome.owl#Activity"/>
        <rdfs:comment>This class contains instances that are tasks performed inside a domestic 
envronmnet but could not be classified in a specific class.</rdfs:comment>
    </owl:Class>
    


    <!-- http://www.owl-ontologies.com/VirtualHome.owl#PhysicalActivity -->


    <owl:Class rdf:about="http://www.owl-ontologies.com/VirtualHome.owl#PhysicalActivity">
        <rdfs:subClassOf rdf:resource="http://www.owl-ontologies.com/VirtualHome.owl#Activity"/>
        <rdfs:comment>Class with sequences for exercise and different physical activities.</rdfs:comment>
    </owl:Class>
    


    <!-- http://www.owl-ontologies.com/VirtualHome.owl#Play -->


    <owl:Class rdf:about="http://www.owl-ontologies.com/VirtualHome.owl#Play">
        <rdfs:subClassOf rdf:resource="http://www.owl-ontologies.com/VirtualHome.owl#Leisure"/>
        <rdfs:comment>The class with sequence of actions on how to play (physical games).</rdfs:comment>
    </owl:Class>
    


    <!-- http://www.owl-ontologies.com/VirtualHome.owl#Read -->


    <owl:Class rdf:about="http://www.owl-ontologies.com/VirtualHome.owl#Read">
        <rdfs:subClassOf rdf:resource="http://www.owl-ontologies.com/VirtualHome.owl#Other"/>
        <rdfs:comment>The class with sequence of actions for  reading.</rdfs:comment>
    </owl:Class>
    


    <!-- http://www.owl-ontologies.com/VirtualHome.owl#Sew -->


    <owl:Class rdf:about="http://www.owl-ontologies.com/VirtualHome.owl#Sew">
        <rdfs:subClassOf rdf:resource="http://www.owl-ontologies.com/VirtualHome.owl#Other"/>
        <rdfs:comment>The class with sequence of actions for sewing, from inside the house.</rdfs:comment>
    </owl:Class>
    


    <!-- http://www.owl-ontologies.com/VirtualHome.owl#Shave -->


    <owl:Class rdf:about="http://www.owl-ontologies.com/VirtualHome.owl#Shave">
        <rdfs:subClassOf rdf:resource="http://www.owl-ontologies.com/VirtualHome.owl#HygieneStyling"/>
        <rdfs:comment>The class with sequence of actions for shaving your own face.</rdfs:comment>
    </owl:Class>
    


    <!-- http://www.owl-ontologies.com/VirtualHome.owl#Sit -->


    <owl:Class rdf:about="http://www.owl-ontologies.com/VirtualHome.owl#Sit">
        <rdfs:subClassOf rdf:resource="http://www.owl-ontologies.com/VirtualHome.owl#Other"/>
        <rdfs:comment>The class with sequence of actions for sitting.</rdfs:comment>
    </owl:Class>
    


    <!-- http://www.owl-ontologies.com/VirtualHome.owl#SocialInteraction -->


    <owl:Class rdf:about="http://www.owl-ontologies.com/VirtualHome.owl#SocialInteraction">
        <rdfs:subClassOf rdf:resource="http://www.owl-ontologies.com/VirtualHome.owl#Activity"/>
        <rdfs:comment>Class that contains sequences that are related between , human-robot or 
human-human interaction.</rdfs:comment>
    </owl:Class>
    


    <!-- http://www.owl-ontologies.com/VirtualHome.owl#Stretch -->


    <owl:Class rdf:about="http://www.owl-ontologies.com/VirtualHome.owl#Stretch">
        <rdfs:subClassOf rdf:resource="http://www.owl-ontologies.com/VirtualHome.owl#PhysicalActivity"/>
        <rdfs:comment>A class with soft physical activity, or exercise, such as stretch.</rdfs:comment>
    </owl:Class>
    


    <!-- http://www.owl-ontologies.com/VirtualHome.owl#Wait -->


    <owl:Class rdf:about="http://www.owl-ontologies.com/VirtualHome.owl#Wait">
        <rdfs:subClassOf rdf:resource="http://www.owl-ontologies.com/VirtualHome.owl#Other"/>
        <rdfs:comment>The class with sequence of actions for waiting.</rdfs:comment>
    </owl:Class>
    


    <!-- http://www.owl-ontologies.com/VirtualHome.owl#Work -->


    <owl:Class rdf:about="http://www.owl-ontologies.com/VirtualHome.owl#Work">
        <rdfs:subClassOf rdf:resource="http://www.owl-ontologies.com/VirtualHome.owl#Activity"/>
        <rdfs:comment>Class with related activites such as send an email, getting ready for work.</rdfs:comment>
    </owl:Class>
    


    <!-- http://www.owl-ontologies.com/VirtualHome.owl#Write -->


    <owl:Class rdf:about="http://www.owl-ontologies.com/VirtualHome.owl#Write">
        <rdfs:subClassOf rdf:resource="http://www.owl-ontologies.com/VirtualHome.owl#Other"/>
        <rdfs:comment>The class with sequence of actions for writing on a papers or on the computer.</rdfs:comment>
    </owl:Class>
    


    <!-- http://www.owl-ontologies.com/VirtualHome.owl#add_paper_to_printer -->


    <owl:Class rdf:about="http://www.owl-ontologies.com/VirtualHome.owl#add_paper_to_printer">
        <rdfs:subClassOf rdf:resource="http://www.owl-ontologies.com/VirtualHome.owl#Other"/>
        <rdfs:comment>The class with sequence of actions for adding paper to the printer.</rdfs:comment>
    </owl:Class>
    


    <!-- http://www.owl-ontologies.com/VirtualHome.owl#added_meat_to_freezer -->


    <owl:Class rdf:about="http://www.owl-ontologies.com/VirtualHome.owl#added_meat_to_freezer">
        <rdfs:subClassOf rdf:resource="http://www.owl-ontologies.com/VirtualHome.owl#HouseArrangement"/>
        <rdfs:comment>The class with sequence of actions for adding meat into the freezer.</rdfs:comment>
    </owl:Class>
    


    <!-- http://www.owl-ontologies.com/VirtualHome.owl#admire_art -->


    <owl:Class rdf:about="http://www.owl-ontologies.com/VirtualHome.owl#admire_art">
        <rdfs:subClassOf rdf:resource="http://www.owl-ontologies.com/VirtualHome.owl#Other"/>
        <rdfs:comment>The class with sequence of actions for admiring art that exist inside 
your home.</rdfs:comment>
    </owl:Class>
    


    <!-- http://www.owl-ontologies.com/VirtualHome.owl#admire_paintings -->


    <owl:Class rdf:about="http://www.owl-ontologies.com/VirtualHome.owl#admire_paintings">
        <rdfs:subClassOf rdf:resource="http://www.owl-ontologies.com/VirtualHome.owl#Leisure"/>
    </owl:Class>
    


    <!-- http://www.owl-ontologies.com/VirtualHome.owl#annoy_your_dog -->


    <owl:Class rdf:about="http://www.owl-ontologies.com/VirtualHome.owl#annoy_your_dog">
        <rdfs:subClassOf rdf:resource="http://www.owl-ontologies.com/VirtualHome.owl#Other"/>
        <rdfs:comment>The class with sequence of actions for annoying your dog, in any room (play with dog).</rdfs:comment>
    </owl:Class>
    


    <!-- http://www.owl-ontologies.com/VirtualHome.owl#answer_door -->


    <owl:Class rdf:about="http://www.owl-ontologies.com/VirtualHome.owl#answer_door">
        <rdfs:subClassOf rdf:resource="http://www.owl-ontologies.com/VirtualHome.owl#SocialInteraction"/>
        <rdfs:comment>The class with sequence of actions for answering the door (main entrance 
of the house).</rdfs:comment>
    </owl:Class>
    


    <!-- http://www.owl-ontologies.com/VirtualHome.owl#answer_emails -->


    <owl:Class rdf:about="http://www.owl-ontologies.com/VirtualHome.owl#answer_emails">
        <rdfs:subClassOf rdf:resource="http://www.owl-ontologies.com/VirtualHome.owl#Work"/>
        <rdfs:comment>The class with sequence of actions for answering your mails (writing the 
text, not sending the mail).</rdfs:comment>
    </owl:Class>
    


    <!-- http://www.owl-ontologies.com/VirtualHome.owl#answer_phone -->


    <owl:Class rdf:about="http://www.owl-ontologies.com/VirtualHome.owl#answer_phone">
        <rdfs:subClassOf rdf:resource="http://www.owl-ontologies.com/VirtualHome.owl#Other"/>
        <rdfs:comment>The class with sequence of actions for answering the phone, cell phone or phone home.</rdfs:comment>
    </owl:Class>
    


    <!-- http://www.owl-ontologies.com/VirtualHome.owl#apply_lotion -->


    <owl:Class rdf:about="http://www.owl-ontologies.com/VirtualHome.owl#apply_lotion">
        <rdfs:subClassOf rdf:resource="http://www.owl-ontologies.com/VirtualHome.owl#HygieneStyling"/>
        <rdfs:comment>The class with sequence of actions for applying lotion in any part of 
the body.</rdfs:comment>
    </owl:Class>
    


    <!-- http://www.owl-ontologies.com/VirtualHome.owl#arrange_bookshelf -->


    <owl:Class rdf:about="http://www.owl-ontologies.com/VirtualHome.owl#arrange_bookshelf">
        <rdfs:subClassOf rdf:resource="http://www.owl-ontologies.com/VirtualHome.owl#HouseArrangement"/>
        <rdfs:comment>The class with sequence of actions for arranging the bookself.</rdfs:comment>
    </owl:Class>
    


    <!-- http://www.owl-ontologies.com/VirtualHome.owl#arrange_folders -->


    <owl:Class rdf:about="http://www.owl-ontologies.com/VirtualHome.owl#arrange_folders">
        <rdfs:subClassOf rdf:resource="http://www.owl-ontologies.com/VirtualHome.owl#HouseArrangement"/>
        <rdfs:comment>The class with sequence of actions for arranging folders, in any place 
or room.</rdfs:comment>
    </owl:Class>
    


    <!-- http://www.owl-ontologies.com/VirtualHome.owl#arrange_furniture -->


    <owl:Class rdf:about="http://www.owl-ontologies.com/VirtualHome.owl#arrange_furniture">
        <rdfs:subClassOf rdf:resource="http://www.owl-ontologies.com/VirtualHome.owl#HouseArrangement"/>
        <rdfs:comment>The class with sequence of actions for arranging furniture in any room.</rdfs:comment>
    </owl:Class>
    


    <!-- http://www.owl-ontologies.com/VirtualHome.owl#arrange_shoes -->


    <owl:Class rdf:about="http://www.owl-ontologies.com/VirtualHome.owl#arrange_shoes">
        <rdfs:subClassOf rdf:resource="http://www.owl-ontologies.com/VirtualHome.owl#HouseArrangement"/>
        <rdfs:comment>The class with sequence of actions for arranging shoes in any room.</rdfs:comment>
    </owl:Class>
    


    <!-- http://www.owl-ontologies.com/VirtualHome.owl#arrange_sofa -->


    <owl:Class rdf:about="http://www.owl-ontologies.com/VirtualHome.owl#arrange_sofa">
        <rdfs:subClassOf rdf:resource="http://www.owl-ontologies.com/VirtualHome.owl#HouseArrangement"/>
        <rdfs:comment>The class with sequence of actions for arranging sofa, in any room.</rdfs:comment>
    </owl:Class>
    


    <!-- http://www.owl-ontologies.com/VirtualHome.owl#bake -->


    <owl:Class rdf:about="http://www.owl-ontologies.com/VirtualHome.owl#bake">
        <rdfs:subClassOf rdf:resource="http://www.owl-ontologies.com/VirtualHome.owl#FoodPreparation"/>
        <rdfs:comment>The class with sequence of actions for baking something.</rdfs:comment>
    </owl:Class>
    


    <!-- http://www.owl-ontologies.com/VirtualHome.owl#bathe -->


    <owl:Class rdf:about="http://www.owl-ontologies.com/VirtualHome.owl#bathe">
        <rdfs:subClassOf rdf:resource="http://www.owl-ontologies.com/VirtualHome.owl#HygieneStyling"/>
        <rdfs:comment>The class with sequence of actions for taking a bathe.</rdfs:comment>
    </owl:Class>
    


    <!-- http://www.owl-ontologies.com/VirtualHome.owl#be_able_to_talk_to_me_about_tv_show_im_watching -->


    <owl:Class rdf:about="http://www.owl-ontologies.com/VirtualHome.owl#be_able_to_talk_to_me_about_tv_show_im_watching">
        <rdfs:subClassOf rdf:resource="http://www.owl-ontologies.com/VirtualHome.owl#SocialInteraction"/>
        <rdfs:comment>The class with sequence of actions for beeing able to talk to the user 
about TV show I&apos;m watching.</rdfs:comment>
    </owl:Class>
    


    <!-- http://www.owl-ontologies.com/VirtualHome.owl#bed_time -->


    <owl:Class rdf:about="http://www.owl-ontologies.com/VirtualHome.owl#bed_time">
        <rdfs:subClassOf rdf:resource="http://www.owl-ontologies.com/VirtualHome.owl#BedTimeSleep"/>
        <rdfs:comment>The class with sequence of actions for going to bed.</rdfs:comment>
    </owl:Class>
    


    <!-- http://www.owl-ontologies.com/VirtualHome.owl#blow_dry_hair -->


    <owl:Class rdf:about="http://www.owl-ontologies.com/VirtualHome.owl#blow_dry_hair">
        <rdfs:subClassOf rdf:resource="http://www.owl-ontologies.com/VirtualHome.owl#HygieneStyling"/>
        <rdfs:comment>The class with sequence of actions for blowing and drying your hair.</rdfs:comment>
    </owl:Class>
    


    <!-- http://www.owl-ontologies.com/VirtualHome.owl#break_table -->


    <owl:Class rdf:about="http://www.owl-ontologies.com/VirtualHome.owl#break_table">
        <rdfs:subClassOf rdf:resource="http://www.owl-ontologies.com/VirtualHome.owl#Other"/>
        <rdfs:comment>The class with sequence of actions for breaking a table, in any room.</rdfs:comment>
    </owl:Class>
    


    <!-- http://www.owl-ontologies.com/VirtualHome.owl#breakfast -->


    <owl:Class rdf:about="http://www.owl-ontologies.com/VirtualHome.owl#breakfast">
        <rdfs:subClassOf rdf:resource="http://www.owl-ontologies.com/VirtualHome.owl#FoodPreparation"/>
        <rdfs:comment>The class with sequence of actions for breakfast.</rdfs:comment>
    </owl:Class>
    


    <!-- http://www.owl-ontologies.com/VirtualHome.owl#brew_coffee -->


    <owl:Class rdf:about="http://www.owl-ontologies.com/VirtualHome.owl#brew_coffee">
        <rdfs:subClassOf rdf:resource="http://www.owl-ontologies.com/VirtualHome.owl#FoodPreparation"/>
        <rdfs:comment>The class with sequence of actions for brewing coffee in any room.</rdfs:comment>
    </owl:Class>
    


    <!-- http://www.owl-ontologies.com/VirtualHome.owl#bring_dirty_plate_to_sink -->


    <owl:Class rdf:about="http://www.owl-ontologies.com/VirtualHome.owl#bring_dirty_plate_to_sink">
        <rdfs:subClassOf rdf:resource="http://www.owl-ontologies.com/VirtualHome.owl#HouseArrangement"/>
        <rdfs:comment>The class with sequence of actions for bringing your dirty plate in the 
sink.</rdfs:comment>
    </owl:Class>
    


    <!-- http://www.owl-ontologies.com/VirtualHome.owl#bring_food -->


    <owl:Class rdf:about="http://www.owl-ontologies.com/VirtualHome.owl#bring_food">
        <rdfs:subClassOf rdf:resource="http://www.owl-ontologies.com/VirtualHome.owl#Other"/>
        <rdfs:comment>The class with sequence of actions for bringing food, to home from any place.</rdfs:comment>
    </owl:Class>
    


    <!-- http://www.owl-ontologies.com/VirtualHome.owl#bring_leftovers_in_kitchen -->


    <owl:Class rdf:about="http://www.owl-ontologies.com/VirtualHome.owl#bring_leftovers_in_kitchen">
        <rdfs:subClassOf rdf:resource="http://www.owl-ontologies.com/VirtualHome.owl#HouseArrangement"/>
        <rdfs:comment>The class with sequence of actions for bringing leftovers in kitchen, 
from any room.</rdfs:comment>
    </owl:Class>
    


    <!-- http://www.owl-ontologies.com/VirtualHome.owl#bring_me_red_cookbook -->


    <owl:Class rdf:about="http://www.owl-ontologies.com/VirtualHome.owl#bring_me_red_cookbook">
        <rdfs:subClassOf rdf:resource="http://www.owl-ontologies.com/VirtualHome.owl#Other"/>
        <rdfs:comment>The class with sequence of actions for bringing the user the red 
cookbook.</rdfs:comment>
    </owl:Class>
    


    <!-- http://www.owl-ontologies.com/VirtualHome.owl#broom -->


    <owl:Class rdf:about="http://www.owl-ontologies.com/VirtualHome.owl#broom">
        <rdfs:subClassOf rdf:resource="http://www.owl-ontologies.com/VirtualHome.owl#HygieneStyling"/>
        <rdfs:comment>The class with sequence of actions for broomin, every room in the house.</rdfs:comment>
    </owl:Class>
    


    <!-- http://www.owl-ontologies.com/VirtualHome.owl#browse_computer -->


    <owl:Class rdf:about="http://www.owl-ontologies.com/VirtualHome.owl#browse_computer">
        <rdfs:subClassOf rdf:resource="http://www.owl-ontologies.com/VirtualHome.owl#Leisure"/>
        <rdfs:comment>The class with sequence of actions for browsing the computer.</rdfs:comment>
    </owl:Class>
    


    <!-- http://www.owl-ontologies.com/VirtualHome.owl#browse_internet -->


    <owl:Class rdf:about="http://www.owl-ontologies.com/VirtualHome.owl#browse_internet">
        <rdfs:subClassOf rdf:resource="http://www.owl-ontologies.com/VirtualHome.owl#Leisure"/>
        <rdfs:subClassOf rdf:resource="http://www.owl-ontologies.com/VirtualHome.owl#Work"/>
        <rdfs:comment>The class which contains sequences for browsing the internet.</rdfs:comment>
    </owl:Class>
    


    <!-- http://www.owl-ontologies.com/VirtualHome.owl#brush_hair -->


    <owl:Class rdf:about="http://www.owl-ontologies.com/VirtualHome.owl#brush_hair">
        <rdfs:subClassOf rdf:resource="http://www.owl-ontologies.com/VirtualHome.owl#HygieneStyling"/>
        <rdfs:comment>The class with sequence of actions for brushing your hair.</rdfs:comment>
    </owl:Class>
    


    <!-- http://www.owl-ontologies.com/VirtualHome.owl#brush_teeth -->


    <owl:Class rdf:about="http://www.owl-ontologies.com/VirtualHome.owl#brush_teeth">
        <rdfs:subClassOf rdf:resource="http://www.owl-ontologies.com/VirtualHome.owl#HygieneStyling"/>
        <rdfs:comment>The class with sequence of actions for brushing your teeth.</rdfs:comment>
    </owl:Class>
    


    <!-- http://www.owl-ontologies.com/VirtualHome.owl#build_lego_house -->


    <owl:Class rdf:about="http://www.owl-ontologies.com/VirtualHome.owl#build_lego_house">
        <rdfs:subClassOf rdf:resource="http://www.owl-ontologies.com/VirtualHome.owl#Other"/>
        <rdfs:comment>The class with sequence of actions for building a lego house, in any 
room.</rdfs:comment>
    </owl:Class>
    


    <!-- http://www.owl-ontologies.com/VirtualHome.owl#call_client -->


    <owl:Class rdf:about="http://www.owl-ontologies.com/VirtualHome.owl#call_client">
        <rdfs:subClassOf rdf:resource="http://www.owl-ontologies.com/VirtualHome.owl#SocialInteraction"/>
        <rdfs:comment>The class with sequence of actions for calling client, either form cell 
phone or home phone.</rdfs:comment>
    </owl:Class>
    


    <!-- http://www.owl-ontologies.com/VirtualHome.owl#call_family_member_with_skype_application -->


    <owl:Class rdf:about="http://www.owl-ontologies.com/VirtualHome.owl#call_family_member_with_skype_application">
        <rdfs:subClassOf rdf:resource="http://www.owl-ontologies.com/VirtualHome.owl#SocialInteraction"/>
        <rdfs:comment>The class with sequence of actions for calling family member with skype 
application.</rdfs:comment>
    </owl:Class>
    


    <!-- http://www.owl-ontologies.com/VirtualHome.owl#call_mother -->


    <owl:Class rdf:about="http://www.owl-ontologies.com/VirtualHome.owl#call_mother">
        <rdfs:subClassOf rdf:resource="http://www.owl-ontologies.com/VirtualHome.owl#SocialInteraction"/>
        <rdfs:comment>The class with sequence of actions for calling your mother.</rdfs:comment>
    </owl:Class>
    


    <!-- http://www.owl-ontologies.com/VirtualHome.owl#card -->


    <owl:Class rdf:about="http://www.owl-ontologies.com/VirtualHome.owl#card">
        <rdfs:subClassOf rdf:resource="http://www.owl-ontologies.com/VirtualHome.owl#Other"/>
        <rdfs:comment>The class with sequence of actions for carding.</rdfs:comment>
    </owl:Class>
    


    <!-- http://www.owl-ontologies.com/VirtualHome.owl#care_for_houseplants -->


    <owl:Class rdf:about="http://www.owl-ontologies.com/VirtualHome.owl#care_for_houseplants">
        <rdfs:subClassOf rdf:resource="http://www.owl-ontologies.com/VirtualHome.owl#HouseArrangement"/>
        <rdfs:comment>The class with sequence of actions for for carring for house plants.</rdfs:comment>
    </owl:Class>
    


    <!-- http://www.owl-ontologies.com/VirtualHome.owl#carry_box -->


    <owl:Class rdf:about="http://www.owl-ontologies.com/VirtualHome.owl#carry_box">
        <rdfs:subClassOf rdf:resource="http://www.owl-ontologies.com/VirtualHome.owl#HouseArrangement"/>
    </owl:Class>
    


    <!-- http://www.owl-ontologies.com/VirtualHome.owl#carry_groceries_to_kitchen -->


    <owl:Class rdf:about="http://www.owl-ontologies.com/VirtualHome.owl#carry_groceries_to_kitchen">
        <rdfs:subClassOf rdf:resource="http://www.owl-ontologies.com/VirtualHome.owl#Other"/>
        <rdfs:comment>The class with sequence of actions for carrying groceries to kitchen.</rdfs:comment>
    </owl:Class>
    


    <!-- http://www.owl-ontologies.com/VirtualHome.owl#celebrate -->


    <owl:Class rdf:about="http://www.owl-ontologies.com/VirtualHome.owl#celebrate">
        <rdfs:subClassOf rdf:resource="http://www.owl-ontologies.com/VirtualHome.owl#Other"/>
        <rdfs:comment>The class with sequence of actions for celebrating, in any occasion.</rdfs:comment>
    </owl:Class>
    


    <!-- http://www.owl-ontologies.com/VirtualHome.owl#celebrate_birthday_with_nice_meal -->


    <owl:Class rdf:about="http://www.owl-ontologies.com/VirtualHome.owl#celebrate_birthday_with_nice_meal">
        <rdfs:subClassOf rdf:resource="http://www.owl-ontologies.com/VirtualHome.owl#Other"/>
        <rdfs:comment>The class with sequence of actions for celebrating birthday with a nice 
meal, in any room.</rdfs:comment>
    </owl:Class>
    


    <!-- http://www.owl-ontologies.com/VirtualHome.owl#change_bedding -->


    <owl:Class rdf:about="http://www.owl-ontologies.com/VirtualHome.owl#change_bedding">
        <rdfs:subClassOf rdf:resource="http://www.owl-ontologies.com/VirtualHome.owl#HouseArrangement"/>
        <rdfs:comment>The class with sequence of actions for changing the bedding, in any bed 
in the house.</rdfs:comment>
    </owl:Class>
    


    <!-- http://www.owl-ontologies.com/VirtualHome.owl#change_clothes -->


    <owl:Class rdf:about="http://www.owl-ontologies.com/VirtualHome.owl#change_clothes">
        <rdfs:subClassOf rdf:resource="http://www.owl-ontologies.com/VirtualHome.owl#HygieneStyling"/>
        <rdfs:comment>The class with sequence of actions for changing your own clothes.</rdfs:comment>
    </owl:Class>
    


    <!-- http://www.owl-ontologies.com/VirtualHome.owl#change_curtains -->


    <owl:Class rdf:about="http://www.owl-ontologies.com/VirtualHome.owl#change_curtains">
        <rdfs:subClassOf rdf:resource="http://www.owl-ontologies.com/VirtualHome.owl#HouseArrangement"/>
        <rdfs:comment>The class with sequence of actions for changing curtains, in any room.</rdfs:comment>
    </owl:Class>
    


    <!-- http://www.owl-ontologies.com/VirtualHome.owl#change_light -->


    <owl:Class rdf:about="http://www.owl-ontologies.com/VirtualHome.owl#change_light">
        <rdfs:subClassOf rdf:resource="http://www.owl-ontologies.com/VirtualHome.owl#HouseArrangement"/>
        <rdfs:comment>The class with sequence of actions for changing lights in any room.</rdfs:comment>
    </owl:Class>
    


    <!-- http://www.owl-ontologies.com/VirtualHome.owl#change_lightbulb -->


    <owl:Class rdf:about="http://www.owl-ontologies.com/VirtualHome.owl#change_lightbulb">
        <rdfs:subClassOf rdf:resource="http://www.owl-ontologies.com/VirtualHome.owl#HouseArrangement"/>
        <rdfs:comment>The class with sequence of actions for changing any lightbulb, inside the house.</rdfs:comment>
    </owl:Class>
    


    <!-- http://www.owl-ontologies.com/VirtualHome.owl#change_sheets_and_pillow_cases -->


    <owl:Class rdf:about="http://www.owl-ontologies.com/VirtualHome.owl#change_sheets_and_pillow_cases">
        <rdfs:subClassOf rdf:resource="http://www.owl-ontologies.com/VirtualHome.owl#HouseArrangement"/>
        <rdfs:comment>The class with sequence of actions for changing sheets and pillow cases, for any bed in the house.</rdfs:comment>
    </owl:Class>
    


    <!-- http://www.owl-ontologies.com/VirtualHome.owl#change_sheets_on_bed -->


    <owl:Class rdf:about="http://www.owl-ontologies.com/VirtualHome.owl#change_sheets_on_bed">
        <rdfs:subClassOf rdf:resource="http://www.owl-ontologies.com/VirtualHome.owl#HouseArrangement"/>
        <rdfs:comment>The class with sequence of actions for changing sheets on bed.</rdfs:comment>
    </owl:Class>
    


    <!-- http://www.owl-ontologies.com/VirtualHome.owl#change_shower_curtain -->


    <owl:Class rdf:about="http://www.owl-ontologies.com/VirtualHome.owl#change_shower_curtain">
        <rdfs:subClassOf rdf:resource="http://www.owl-ontologies.com/VirtualHome.owl#HouseArrangement"/>
        <rdfs:comment>The class with sequence of actions for changing the curtain from a shower.</rdfs:comment>
    </owl:Class>
    


    <!-- http://www.owl-ontologies.com/VirtualHome.owl#change_toilet_paper_roll -->


    <owl:Class rdf:about="http://www.owl-ontologies.com/VirtualHome.owl#change_toilet_paper_roll">
        <rdfs:subClassOf rdf:resource="http://www.owl-ontologies.com/VirtualHome.owl#HouseArrangement"/>
        <rdfs:comment>The class with sequence of actions for changing toilet paper roll.</rdfs:comment>
    </owl:Class>
    


    <!-- http://www.owl-ontologies.com/VirtualHome.owl#change_toothbrush -->


    <owl:Class rdf:about="http://www.owl-ontologies.com/VirtualHome.owl#change_toothbrush">
        <rdfs:subClassOf rdf:resource="http://www.owl-ontologies.com/VirtualHome.owl#HouseArrangement"/>
        <rdfs:comment>The class with sequence of actions for changing the toothbrush, in any 
room.</rdfs:comment>
    </owl:Class>
    


    <!-- http://www.owl-ontologies.com/VirtualHome.owl#change_tv_channel -->


    <owl:Class rdf:about="http://www.owl-ontologies.com/VirtualHome.owl#change_tv_channel">
        <rdfs:subClassOf rdf:resource="http://www.owl-ontologies.com/VirtualHome.owl#Other"/>
        <rdfs:comment>The class with sequence of actions for changing the tv channel.</rdfs:comment>
    </owl:Class>
    


    <!-- http://www.owl-ontologies.com/VirtualHome.owl#change_tv_channels -->


    <owl:Class rdf:about="http://www.owl-ontologies.com/VirtualHome.owl#change_tv_channels">
        <rdfs:subClassOf rdf:resource="http://www.owl-ontologies.com/VirtualHome.owl#Leisure"/>
        <rdfs:comment>The class with sequence of actions for changing TV channels.</rdfs:comment>
    </owl:Class>
    


    <!-- http://www.owl-ontologies.com/VirtualHome.owl#check_appearance_in_mirror -->


    <owl:Class rdf:about="http://www.owl-ontologies.com/VirtualHome.owl#check_appearance_in_mirror">
        <rdfs:subClassOf rdf:resource="http://www.owl-ontologies.com/VirtualHome.owl#HygieneStyling"/>
        <rdfs:comment>The class with sequence of actions for checking appearance in mirror.</rdfs:comment>
    </owl:Class>
    


    <!-- http://www.owl-ontologies.com/VirtualHome.owl#check_email -->


    <owl:Class rdf:about="http://www.owl-ontologies.com/VirtualHome.owl#check_email">
        <rdfs:subClassOf rdf:resource="http://www.owl-ontologies.com/VirtualHome.owl#Work"/>
        <rdfs:comment>The class with sequence of actions for checking your mail after you have 
opened it.</rdfs:comment>
    </owl:Class>
    


    <!-- http://www.owl-ontologies.com/VirtualHome.owl#check_homework -->


    <owl:Class rdf:about="http://www.owl-ontologies.com/VirtualHome.owl#check_homework">
        <rdfs:subClassOf rdf:resource="http://www.owl-ontologies.com/VirtualHome.owl#Work"/>
        <rdfs:comment>The class with sequence of actions for checking homework (either you own 
or anothers person).</rdfs:comment>
    </owl:Class>
    


    <!-- http://www.owl-ontologies.com/VirtualHome.owl#check_self_in_mirror -->


    <owl:Class rdf:about="http://www.owl-ontologies.com/VirtualHome.owl#check_self_in_mirror">
        <rdfs:subClassOf rdf:resource="http://www.owl-ontologies.com/VirtualHome.owl#HygieneStyling"/>
        <rdfs:comment>The class with sequence of actions for checking your self in the mirror.</rdfs:comment>
    </owl:Class>
    


    <!-- http://www.owl-ontologies.com/VirtualHome.owl#chop_vegetables -->


    <owl:Class rdf:about="http://www.owl-ontologies.com/VirtualHome.owl#chop_vegetables">
        <rdfs:subClassOf rdf:resource="http://www.owl-ontologies.com/VirtualHome.owl#FoodPreparation"/>
        <rdfs:comment>Class with sequences on how to cut-chop vegetables in order to prepare dinner, salad, or other kind of food.</rdfs:comment>
    </owl:Class>
    


    <!-- http://www.owl-ontologies.com/VirtualHome.owl#clean -->


    <owl:Class rdf:about="http://www.owl-ontologies.com/VirtualHome.owl#clean">
        <rdfs:subClassOf rdf:resource="http://www.owl-ontologies.com/VirtualHome.owl#HouseCleaning"/>
        <rdfs:comment>Class with general sequences for cleaning, such as clean lamp, bathroom, 
welcome mat.</rdfs:comment>
    </owl:Class>
    


    <!-- http://www.owl-ontologies.com/VirtualHome.owl#clean_bathroom -->


    <owl:Class rdf:about="http://www.owl-ontologies.com/VirtualHome.owl#clean_bathroom">
        <rdfs:subClassOf rdf:resource="http://www.owl-ontologies.com/VirtualHome.owl#HouseCleaning"/>
        <rdfs:comment>The class with sequence of actions for cleaning the bathroom, the whole 
room.</rdfs:comment>
    </owl:Class>
    


    <!-- http://www.owl-ontologies.com/VirtualHome.owl#clean_desk -->


    <owl:Class rdf:about="http://www.owl-ontologies.com/VirtualHome.owl#clean_desk">
        <rdfs:subClassOf rdf:resource="http://www.owl-ontologies.com/VirtualHome.owl#HouseCleaning"/>
    </owl:Class>
    


    <!-- http://www.owl-ontologies.com/VirtualHome.owl#clean_dishes -->


    <owl:Class rdf:about="http://www.owl-ontologies.com/VirtualHome.owl#clean_dishes">
        <rdfs:subClassOf rdf:resource="http://www.owl-ontologies.com/VirtualHome.owl#HouseArrangement"/>
        <rdfs:comment>The class with sequence of actions for cleaning the dishes.</rdfs:comment>
    </owl:Class>
    


    <!-- http://www.owl-ontologies.com/VirtualHome.owl#clean_eggs_from_our_chickens -->


    <owl:Class rdf:about="http://www.owl-ontologies.com/VirtualHome.owl#clean_eggs_from_our_chickens">
        <rdfs:subClassOf rdf:resource="http://www.owl-ontologies.com/VirtualHome.owl#Other"/>
        <rdfs:comment>The class with sequence of actions for cleaning eggs that were produced 
by our chickens.</rdfs:comment>
    </owl:Class>
    


    <!-- http://www.owl-ontologies.com/VirtualHome.owl#clean_floor -->


    <owl:Class rdf:about="http://www.owl-ontologies.com/VirtualHome.owl#clean_floor">
        <rdfs:subClassOf rdf:resource="http://www.owl-ontologies.com/VirtualHome.owl#HouseCleaning"/>
        <rdfs:comment>Class with sequences on how to clean the floor.</rdfs:comment>
    </owl:Class>
    


    <!-- http://www.owl-ontologies.com/VirtualHome.owl#clean_fridge -->


    <owl:Class rdf:about="http://www.owl-ontologies.com/VirtualHome.owl#clean_fridge">
        <rdfs:subClassOf rdf:resource="http://www.owl-ontologies.com/VirtualHome.owl#HouseCleaning"/>
        <rdfs:comment>The class with sequence of actions clean the fridge form the inside and 
the outside.</rdfs:comment>
    </owl:Class>
    


    <!-- http://www.owl-ontologies.com/VirtualHome.owl#clean_glasses -->


    <owl:Class rdf:about="http://www.owl-ontologies.com/VirtualHome.owl#clean_glasses">
        <rdfs:subClassOf rdf:resource="http://www.owl-ontologies.com/VirtualHome.owl#HouseArrangement"/>
        <rdfs:comment>The class with sequence of actions for cleaning watching glasses.</rdfs:comment>
    </owl:Class>
    


    <!-- http://www.owl-ontologies.com/VirtualHome.owl#clean_kitchen -->


    <owl:Class rdf:about="http://www.owl-ontologies.com/VirtualHome.owl#clean_kitchen">
        <rdfs:subClassOf rdf:resource="http://www.owl-ontologies.com/VirtualHome.owl#HouseCleaning"/>
        <rdfs:comment>The class with sequence of actions the procedure of cleaning all the 
kitchen.</rdfs:comment>
    </owl:Class>
    


    <!-- http://www.owl-ontologies.com/VirtualHome.owl#clean_large_jacuzzi_tub -->


    <owl:Class rdf:about="http://www.owl-ontologies.com/VirtualHome.owl#clean_large_jacuzzi_tub">
        <rdfs:subClassOf rdf:resource="http://www.owl-ontologies.com/VirtualHome.owl#HouseCleaning"/>
        <rdfs:comment>The class with sequence of actions for cleaning up a large jacuzzi tab.</rdfs:comment>
    </owl:Class>
    


    <!-- http://www.owl-ontologies.com/VirtualHome.owl#clean_mirror -->


    <owl:Class rdf:about="http://www.owl-ontologies.com/VirtualHome.owl#clean_mirror">
        <rdfs:subClassOf rdf:resource="http://www.owl-ontologies.com/VirtualHome.owl#HouseCleaning"/>
        <rdfs:comment>The class with sequence of actions on how to clean a mirror, no matter 
in which room is in.</rdfs:comment>
    </owl:Class>
    


    <!-- http://www.owl-ontologies.com/VirtualHome.owl#clean_room -->


    <owl:Class rdf:about="http://www.owl-ontologies.com/VirtualHome.owl#clean_room">
        <rdfs:subClassOf rdf:resource="http://www.owl-ontologies.com/VirtualHome.owl#HouseCleaning"/>
        <rdfs:comment>The class with sequence of actions on how to clean a room.</rdfs:comment>
    </owl:Class>
    


    <!-- http://www.owl-ontologies.com/VirtualHome.owl#clean_screen -->


    <owl:Class rdf:about="http://www.owl-ontologies.com/VirtualHome.owl#clean_screen">
        <rdfs:subClassOf rdf:resource="http://www.owl-ontologies.com/VirtualHome.owl#HouseCleaning"/>
        <rdfs:comment>The class with sequence of actions for cleaning the screen of the TV, of a computer, or other objects.</rdfs:comment>
    </owl:Class>
    


    <!-- http://www.owl-ontologies.com/VirtualHome.owl#clean_sink -->


    <owl:Class rdf:about="http://www.owl-ontologies.com/VirtualHome.owl#clean_sink">
        <rdfs:subClassOf rdf:resource="http://www.owl-ontologies.com/VirtualHome.owl#HouseCleaning"/>
        <rdfs:comment>Class with sequences for cleaning only the sink, not the surounding, or 
the whole room.</rdfs:comment>
    </owl:Class>
    


    <!-- http://www.owl-ontologies.com/VirtualHome.owl#clean_toilet -->


    <owl:Class rdf:about="http://www.owl-ontologies.com/VirtualHome.owl#clean_toilet">
        <rdfs:subClassOf rdf:resource="http://www.owl-ontologies.com/VirtualHome.owl#HouseCleaning"/>
        <rdfs:comment>Class with sequences on how to clean the toilet specifically, not the 
whole bathroom.</rdfs:comment>
    </owl:Class>
    


    <!-- http://www.owl-ontologies.com/VirtualHome.owl#clear_table -->


    <owl:Class rdf:about="http://www.owl-ontologies.com/VirtualHome.owl#clear_table">
        <rdfs:subClassOf rdf:resource="http://www.owl-ontologies.com/VirtualHome.owl#HouseArrangement"/>
        <rdfs:comment>The class with sequence of actions for clearing the table after eating 
or claering it because it is dirty.</rdfs:comment>
    </owl:Class>
    


    <!-- http://www.owl-ontologies.com/VirtualHome.owl#close_curtains -->


    <owl:Class rdf:about="http://www.owl-ontologies.com/VirtualHome.owl#close_curtains">
        <rdfs:subClassOf rdf:resource="http://www.owl-ontologies.com/VirtualHome.owl#Other"/>
        <rdfs:comment>The class with sequence of actions for clossing the curtains, in any room.</rdfs:comment>
    </owl:Class>
    


    <!-- http://www.owl-ontologies.com/VirtualHome.owl#close_door -->


    <owl:Class rdf:about="http://www.owl-ontologies.com/VirtualHome.owl#close_door">
        <rdfs:subClassOf rdf:resource="http://www.owl-ontologies.com/VirtualHome.owl#Other"/>
        <rdfs:comment>The class with sequence of actions for closing the door from any room.</rdfs:comment>
    </owl:Class>
    


    <!-- http://www.owl-ontologies.com/VirtualHome.owl#close_dresser_drawer -->


    <owl:Class rdf:about="http://www.owl-ontologies.com/VirtualHome.owl#close_dresser_drawer">
        <rdfs:subClassOf rdf:resource="http://www.owl-ontologies.com/VirtualHome.owl#Other"/>
        <rdfs:comment>The class with sequence of actions for closing dresser drawer, in any 
room.</rdfs:comment>
    </owl:Class>
    


    <!-- http://www.owl-ontologies.com/VirtualHome.owl#close_shower_curtain -->


    <owl:Class rdf:about="http://www.owl-ontologies.com/VirtualHome.owl#close_shower_curtain">
        <rdfs:subClassOf rdf:resource="http://www.owl-ontologies.com/VirtualHome.owl#HouseArrangement"/>
        <rdfs:comment>The class with sequence of actions for closing shower curtain.</rdfs:comment>
    </owl:Class>
    


    <!-- http://www.owl-ontologies.com/VirtualHome.owl#collect_napkin_rings -->


    <owl:Class rdf:about="http://www.owl-ontologies.com/VirtualHome.owl#collect_napkin_rings">
        <rdfs:subClassOf rdf:resource="http://www.owl-ontologies.com/VirtualHome.owl#HouseArrangement"/>
        <rdfs:comment>The class with sequence of actions for collecting napkin rings.</rdfs:comment>
    </owl:Class>
    


    <!-- http://www.owl-ontologies.com/VirtualHome.owl#color -->


    <owl:Class rdf:about="http://www.owl-ontologies.com/VirtualHome.owl#color">
        <rdfs:subClassOf rdf:resource="http://www.owl-ontologies.com/VirtualHome.owl#Other"/>
        <rdfs:comment>The class with sequence of actions for coloring (painting, or painting 
house, etc.).</rdfs:comment>
    </owl:Class>
    


    <!-- http://www.owl-ontologies.com/VirtualHome.owl#comb_hair -->


    <owl:Class rdf:about="http://www.owl-ontologies.com/VirtualHome.owl#comb_hair">
        <rdfs:subClassOf rdf:resource="http://www.owl-ontologies.com/VirtualHome.owl#HygieneStyling"/>
        <rdfs:comment>The class with sequence of actions for combing cutting your hair.</rdfs:comment>
    </owl:Class>
    


    <!-- http://www.owl-ontologies.com/VirtualHome.owl#come_home -->


    <owl:Class rdf:about="http://www.owl-ontologies.com/VirtualHome.owl#come_home">
        <rdfs:subClassOf rdf:resource="http://www.owl-ontologies.com/VirtualHome.owl#Other"/>
        <rdfs:comment>The class with sequence of actions for comming home, from wokr, or 
grocery store, etc.</rdfs:comment>
    </owl:Class>
    


    <!-- http://www.owl-ontologies.com/VirtualHome.owl#come_in_and_leave_home -->


    <owl:Class rdf:about="http://www.owl-ontologies.com/VirtualHome.owl#come_in_and_leave_home">
        <rdfs:subClassOf rdf:resource="http://www.owl-ontologies.com/VirtualHome.owl#Other"/>
        <rdfs:comment>The class with sequence of actions for comming in the house to do 
something, and then get out again.</rdfs:comment>
    </owl:Class>
    


    <!-- http://www.owl-ontologies.com/VirtualHome.owl#complete_homework -->


    <owl:Class rdf:about="http://www.owl-ontologies.com/VirtualHome.owl#complete_homework">
        <rdfs:subClassOf rdf:resource="http://www.owl-ontologies.com/VirtualHome.owl#Work"/>
        <rdfs:comment>The class with sequence of actions for completing your homework.</rdfs:comment>
    </owl:Class>
    


    <!-- http://www.owl-ontologies.com/VirtualHome.owl#complete_school_work -->


    <owl:Class rdf:about="http://www.owl-ontologies.com/VirtualHome.owl#complete_school_work">
        <rdfs:subClassOf rdf:resource="http://www.owl-ontologies.com/VirtualHome.owl#Work"/>
        <rdfs:comment>The class with sequence of actions for completing your school work, this 
is not only homework, could also be getting ready for school.</rdfs:comment>
    </owl:Class>
    


    <!-- http://www.owl-ontologies.com/VirtualHome.owl#complete_surveys_on_amazon_turk -->


    <owl:Class rdf:about="http://www.owl-ontologies.com/VirtualHome.owl#complete_surveys_on_amazon_turk">
        <rdfs:subClassOf rdf:resource="http://www.owl-ontologies.com/VirtualHome.owl#Work"/>
        <rdfs:comment>The class with sequence of actions for completing youe amazon turk 
surveys.</rdfs:comment>
    </owl:Class>
    


    <!-- http://www.owl-ontologies.com/VirtualHome.owl#compute -->


    <owl:Class rdf:about="http://www.owl-ontologies.com/VirtualHome.owl#compute">
        <rdfs:subClassOf rdf:resource="http://www.owl-ontologies.com/VirtualHome.owl#Other"/>
        <rdfs:comment>The class with sequence of actions for computing anything.</rdfs:comment>
    </owl:Class>
    


    <!-- http://www.owl-ontologies.com/VirtualHome.owl#computer_work -->


    <owl:Class rdf:about="http://www.owl-ontologies.com/VirtualHome.owl#computer_work">
        <rdfs:subClassOf rdf:resource="http://www.owl-ontologies.com/VirtualHome.owl#Work"/>
        <rdfs:comment>The class with sequence of actions to do computer work.</rdfs:comment>
    </owl:Class>
    


    <!-- http://www.owl-ontologies.com/VirtualHome.owl#cook_some_food -->


    <owl:Class rdf:about="http://www.owl-ontologies.com/VirtualHome.owl#cook_some_food">
        <rdfs:subClassOf rdf:resource="http://www.owl-ontologies.com/VirtualHome.owl#FoodPreparation"/>
        <rdfs:comment>Class with sequences on how to cook some food prepare the place, the 
order of the ingredience.</rdfs:comment>
    </owl:Class>
    


    <!-- http://www.owl-ontologies.com/VirtualHome.owl#curled_hair -->


    <owl:Class rdf:about="http://www.owl-ontologies.com/VirtualHome.owl#curled_hair">
        <rdfs:subClassOf rdf:resource="http://www.owl-ontologies.com/VirtualHome.owl#HygieneStyling"/>
        <rdfs:comment>The class with sequence of actions for making your hair into curle.</rdfs:comment>
    </owl:Class>
    


    <!-- http://www.owl-ontologies.com/VirtualHome.owl#cut_bread -->


    <owl:Class rdf:about="http://www.owl-ontologies.com/VirtualHome.owl#cut_bread">
        <rdfs:subClassOf rdf:resource="http://www.owl-ontologies.com/VirtualHome.owl#FoodPreparation"/>
        <rdfs:comment>The class with sequence of actions for cutting bread.</rdfs:comment>
    </owl:Class>
    


    <!-- http://www.owl-ontologies.com/VirtualHome.owl#cut_steak -->


    <owl:Class rdf:about="http://www.owl-ontologies.com/VirtualHome.owl#cut_steak">
        <rdfs:subClassOf rdf:resource="http://www.owl-ontologies.com/VirtualHome.owl#FoodPreparation"/>
        <rdfs:comment>The class with sequence of actions for cutting the steak.</rdfs:comment>
    </owl:Class>
    


    <!-- http://www.owl-ontologies.com/VirtualHome.owl#cut_toenails -->


    <owl:Class rdf:about="http://www.owl-ontologies.com/VirtualHome.owl#cut_toenails">
        <rdfs:subClassOf rdf:resource="http://www.owl-ontologies.com/VirtualHome.owl#HygieneStyling"/>
        <rdfs:comment>The class with sequence of actions for cutting our toenails.</rdfs:comment>
    </owl:Class>
    


    <!-- http://www.owl-ontologies.com/VirtualHome.owl#cut_your_hair -->


    <owl:Class rdf:about="http://www.owl-ontologies.com/VirtualHome.owl#cut_your_hair">
        <rdfs:subClassOf rdf:resource="http://www.owl-ontologies.com/VirtualHome.owl#HygieneStyling"/>
        <rdfs:comment>The class with sequence of actions for cutting you hair.</rdfs:comment>
    </owl:Class>
    


    <!-- http://www.owl-ontologies.com/VirtualHome.owl#cutting -->


    <owl:Class rdf:about="http://www.owl-ontologies.com/VirtualHome.owl#cutting">
        <rdfs:subClassOf rdf:resource="http://www.owl-ontologies.com/VirtualHome.owl#Other"/>
        <rdfs:comment>The class with sequence of actions for cutting any object, in any room.</rdfs:comment>
    </owl:Class>
    


    <!-- http://www.owl-ontologies.com/VirtualHome.owl#dance_for_table_as_we_eat -->


    <owl:Class rdf:about="http://www.owl-ontologies.com/VirtualHome.owl#dance_for_table_as_we_eat">
        <rdfs:subClassOf rdf:resource="http://www.owl-ontologies.com/VirtualHome.owl#EatingDrinking"/>
        <rdfs:comment>The class with sequence of actions for dancing for amusement at the 
table as the persons eat.</rdfs:comment>
    </owl:Class>
    


    <!-- http://www.owl-ontologies.com/VirtualHome.owl#dance_with_kids -->


    <owl:Class rdf:about="http://www.owl-ontologies.com/VirtualHome.owl#dance_with_kids">
        <rdfs:subClassOf rdf:resource="http://www.owl-ontologies.com/VirtualHome.owl#SocialInteraction"/>
        <rdfs:comment>The class with sequence of actions for dancing with kids.</rdfs:comment>
    </owl:Class>
    


    <!-- http://www.owl-ontologies.com/VirtualHome.owl#de-wrinkle_sheet -->


    <owl:Class rdf:about="http://www.owl-ontologies.com/VirtualHome.owl#de-wrinkle_sheet">
        <rdfs:subClassOf rdf:resource="http://www.owl-ontologies.com/VirtualHome.owl#HouseCleaning"/>
        <rdfs:comment>The class with sequence of actions for de-wrinkling sheets.</rdfs:comment>
    </owl:Class>
    


    <!-- http://www.owl-ontologies.com/VirtualHome.owl#de_wrinkle_sheet -->


    <owl:Class rdf:about="http://www.owl-ontologies.com/VirtualHome.owl#de_wrinkle_sheet">
        <rdfs:subClassOf rdf:resource="http://www.owl-ontologies.com/VirtualHome.owl#Other"/>
        <rdfs:comment>The class with sequence of actions for de-wrinkling the sheet, in any 
room.</rdfs:comment>
    </owl:Class>
    


    <!-- http://www.owl-ontologies.com/VirtualHome.owl#decorate -->


    <owl:Class rdf:about="http://www.owl-ontologies.com/VirtualHome.owl#decorate">
        <rdfs:subClassOf rdf:resource="http://www.owl-ontologies.com/VirtualHome.owl#HouseArrangement"/>
        <rdfs:comment>The class with sequence of actions for decoratng any item inside the 
house that can be decorated.</rdfs:comment>
    </owl:Class>
    


    <!-- http://www.owl-ontologies.com/VirtualHome.owl#decorate_it -->


    <owl:Class rdf:about="http://www.owl-ontologies.com/VirtualHome.owl#decorate_it">
        <rdfs:subClassOf rdf:resource="http://www.owl-ontologies.com/VirtualHome.owl#HouseArrangement"/>
        <rdfs:comment>The class with sequence of actions for decorating something, after 
getting the token &amp;quot;decorate it&amp;quot;.</rdfs:comment>
    </owl:Class>
    


    <!-- http://www.owl-ontologies.com/VirtualHome.owl#deficate -->


    <owl:Class rdf:about="http://www.owl-ontologies.com/VirtualHome.owl#deficate">
        <rdfs:subClassOf rdf:resource="http://www.owl-ontologies.com/VirtualHome.owl#HygieneStyling"/>
        <rdfs:comment>The class with sequence of actions for deficating.</rdfs:comment>
    </owl:Class>
    


    <!-- http://www.owl-ontologies.com/VirtualHome.owl#defrost_chicken -->


    <owl:Class rdf:about="http://www.owl-ontologies.com/VirtualHome.owl#defrost_chicken">
        <rdfs:subClassOf rdf:resource="http://www.owl-ontologies.com/VirtualHome.owl#FoodPreparation"/>
        <rdfs:comment>The class with sequence of actions for defrosting chicken.</rdfs:comment>
    </owl:Class>
    


    <!-- http://www.owl-ontologies.com/VirtualHome.owl#designing_crafts_with_family -->


    <owl:Class rdf:about="http://www.owl-ontologies.com/VirtualHome.owl#designing_crafts_with_family">
        <rdfs:subClassOf rdf:resource="http://www.owl-ontologies.com/VirtualHome.owl#Other"/>
        <rdfs:comment>The class with sequence of actions for designing crafts with your family.</rdfs:comment>
    </owl:Class>
    


    <!-- http://www.owl-ontologies.com/VirtualHome.owl#dining -->


    <owl:Class rdf:about="http://www.owl-ontologies.com/VirtualHome.owl#dining">
        <rdfs:subClassOf rdf:resource="http://www.owl-ontologies.com/VirtualHome.owl#EatingDrinking"/>
        <rdfs:comment>The class with sequence of actions for dining.</rdfs:comment>
    </owl:Class>
    


    <!-- http://www.owl-ontologies.com/VirtualHome.owl#do_an_art_project -->


    <owl:Class rdf:about="http://www.owl-ontologies.com/VirtualHome.owl#do_an_art_project">
        <rdfs:subClassOf rdf:resource="http://www.owl-ontologies.com/VirtualHome.owl#Other"/>
        <rdfs:comment>&lt;p style=&quot;margin-top: 0&quot;&gt;
      The class with sequence of actions for doing an art project, in any room.
    &lt;/p&gt;</rdfs:comment>
    </owl:Class>
    


    <!-- http://www.owl-ontologies.com/VirtualHome.owl#do_dishes -->


    <owl:Class rdf:about="http://www.owl-ontologies.com/VirtualHome.owl#do_dishes">
        <rdfs:subClassOf rdf:resource="http://www.owl-ontologies.com/VirtualHome.owl#HouseArrangement"/>
        <rdfs:comment>The class with sequence of actions for doing the dishes, either clean 
them or put them in the cabinet</rdfs:comment>
    </owl:Class>
    


    <!-- http://www.owl-ontologies.com/VirtualHome.owl#do_facial -->


    <owl:Class rdf:about="http://www.owl-ontologies.com/VirtualHome.owl#do_facial">
        <rdfs:subClassOf rdf:resource="http://www.owl-ontologies.com/VirtualHome.owl#HygieneStyling"/>
        <rdfs:comment>The class with sequence of actions for doing up a facial.</rdfs:comment>
    </owl:Class>
    


    <!-- http://www.owl-ontologies.com/VirtualHome.owl#do_free-style_dance_routine -->


    <owl:Class rdf:about="http://www.owl-ontologies.com/VirtualHome.owl#do_free-style_dance_routine">
        <rdfs:subClassOf rdf:resource="http://www.owl-ontologies.com/VirtualHome.owl#Other"/>
        <rdfs:comment>The class with sequence of actions for doing free style dance routine, 
in any room.</rdfs:comment>
    </owl:Class>
    


    <!-- http://www.owl-ontologies.com/VirtualHome.owl#do_homework -->


    <owl:Class rdf:about="http://www.owl-ontologies.com/VirtualHome.owl#do_homework">
        <rdfs:subClassOf rdf:resource="http://www.owl-ontologies.com/VirtualHome.owl#Work"/>
        <rdfs:comment>The class with sequence of actions for writing down your homework (or 
perform other task that will help you finish your homework).</rdfs:comment>
    </owl:Class>
    


    <!-- http://www.owl-ontologies.com/VirtualHome.owl#do_laundry -->


    <owl:Class rdf:about="http://www.owl-ontologies.com/VirtualHome.owl#do_laundry">
        <rdfs:subClassOf rdf:resource="http://www.owl-ontologies.com/VirtualHome.owl#HouseArrangement"/>
        <rdfs:comment>The class with sequence of actions for doing the laundry in any room available.</rdfs:comment>
    </owl:Class>
    


    <!-- http://www.owl-ontologies.com/VirtualHome.owl#do_nails -->


    <owl:Class rdf:about="http://www.owl-ontologies.com/VirtualHome.owl#do_nails">
        <rdfs:subClassOf rdf:resource="http://www.owl-ontologies.com/VirtualHome.owl#HygieneStyling"/>
        <rdfs:comment>The class with sequence of actions for doing your nails, hands and feet.</rdfs:comment>
    </owl:Class>
    


    <!-- http://www.owl-ontologies.com/VirtualHome.owl#do_taxes -->


    <owl:Class rdf:about="http://www.owl-ontologies.com/VirtualHome.owl#do_taxes">
        <rdfs:subClassOf rdf:resource="http://www.owl-ontologies.com/VirtualHome.owl#Work"/>
        <rdfs:comment>The class with sequence of actions for doing taxes.</rdfs:comment>
    </owl:Class>
    


    <!-- http://www.owl-ontologies.com/VirtualHome.owl#do_work -->


    <owl:Class rdf:about="http://www.owl-ontologies.com/VirtualHome.owl#do_work">
        <rdfs:subClassOf rdf:resource="http://www.owl-ontologies.com/VirtualHome.owl#Work"/>
        <rdfs:comment>The class with sequence of actions for doing work.</rdfs:comment>
    </owl:Class>
    


    <!-- http://www.owl-ontologies.com/VirtualHome.owl#do_work_on_computer -->


    <owl:Class rdf:about="http://www.owl-ontologies.com/VirtualHome.owl#do_work_on_computer">
        <rdfs:subClassOf rdf:resource="http://www.owl-ontologies.com/VirtualHome.owl#Work"/>
        <rdfs:comment>The class with sequence of actions for doing some on the compute, either 
on iths hardware or on the computer itself.</rdfs:comment>
    </owl:Class>
    


    <!-- http://www.owl-ontologies.com/VirtualHome.owl#do_yoga -->


    <owl:Class rdf:about="http://www.owl-ontologies.com/VirtualHome.owl#do_yoga">
        <rdfs:subClassOf rdf:resource="http://www.owl-ontologies.com/VirtualHome.owl#PhysicalActivity"/>
        <rdfs:comment>The class with sequence of actions for doing yoga, in any room.</rdfs:comment>
    </owl:Class>
    


    <!-- http://www.owl-ontologies.com/VirtualHome.owl#draft_home -->


    <owl:Class rdf:about="http://www.owl-ontologies.com/VirtualHome.owl#draft_home">
        <rdfs:subClassOf rdf:resource="http://www.owl-ontologies.com/VirtualHome.owl#Other"/>
        <rdfs:comment>The class with sequence of actions for drafting a home, in any room.</rdfs:comment>
    </owl:Class>
    


    <!-- http://www.owl-ontologies.com/VirtualHome.owl#draw_picture -->


    <owl:Class rdf:about="http://www.owl-ontologies.com/VirtualHome.owl#draw_picture">
        <rdfs:subClassOf rdf:resource="http://www.owl-ontologies.com/VirtualHome.owl#Other"/>
        <rdfs:comment>The class with sequence of actions for drawing any picture, either on 
paper or computer.</rdfs:comment>
    </owl:Class>
    


    <!-- http://www.owl-ontologies.com/VirtualHome.owl#dress_up_and_pretend -->


    <owl:Class rdf:about="http://www.owl-ontologies.com/VirtualHome.owl#dress_up_and_pretend">
        <rdfs:subClassOf rdf:resource="http://www.owl-ontologies.com/VirtualHome.owl#HygieneStyling"/>
        <rdfs:comment>&lt;p style=&quot;margin-top: 0&quot;&gt;
      The class with sequence of actions for dressing up and pretending.
    &lt;/p&gt;</rdfs:comment>
    </owl:Class>
    


    <!-- http://www.owl-ontologies.com/VirtualHome.owl#drink -->


    <owl:Class rdf:about="http://www.owl-ontologies.com/VirtualHome.owl#drink">
        <rdfs:subClassOf rdf:resource="http://www.owl-ontologies.com/VirtualHome.owl#EatingDrinking"/>
    </owl:Class>
    


    <!-- http://www.owl-ontologies.com/VirtualHome.owl#dry_hair -->


    <owl:Class rdf:about="http://www.owl-ontologies.com/VirtualHome.owl#dry_hair">
        <rdfs:subClassOf rdf:resource="http://www.owl-ontologies.com/VirtualHome.owl#HygieneStyling"/>
        <rdfs:comment>The class with sequence of actions for drying your hair.</rdfs:comment>
    </owl:Class>
    


    <!-- http://www.owl-ontologies.com/VirtualHome.owl#dry_soap_bottles -->


    <owl:Class rdf:about="http://www.owl-ontologies.com/VirtualHome.owl#dry_soap_bottles">
        <rdfs:subClassOf rdf:resource="http://www.owl-ontologies.com/VirtualHome.owl#Other"/>
        <rdfs:comment>The class with sequence of actions for drying soap bottles, in any room.</rdfs:comment>
    </owl:Class>
    


    <!-- http://www.owl-ontologies.com/VirtualHome.owl#dust -->


    <owl:Class rdf:about="http://www.owl-ontologies.com/VirtualHome.owl#dust">
        <rdfs:subClassOf rdf:resource="http://www.owl-ontologies.com/VirtualHome.owl#HouseCleaning"/>
        <rdfs:comment>Class with sequences about how to dust, different objects.</rdfs:comment>
    </owl:Class>
    


    <!-- http://www.owl-ontologies.com/VirtualHome.owl#eat_breakfast -->


    <owl:Class rdf:about="http://www.owl-ontologies.com/VirtualHome.owl#eat_breakfast">
        <rdfs:subClassOf rdf:resource="http://www.owl-ontologies.com/VirtualHome.owl#FoodPreparation"/>
        <rdfs:comment>The class with sequence of actions for eating breakfast in any room.</rdfs:comment>
    </owl:Class>
    


    <!-- http://www.owl-ontologies.com/VirtualHome.owl#eat_breaksfast -->


    <owl:Class rdf:about="http://www.owl-ontologies.com/VirtualHome.owl#eat_breaksfast">
        <rdfs:subClassOf rdf:resource="http://www.owl-ontologies.com/VirtualHome.owl#EatingDrinking"/>
        <rdfs:comment>The class with sequence of actions for eating breakfast only.</rdfs:comment>
    </owl:Class>
    


    <!-- http://www.owl-ontologies.com/VirtualHome.owl#eat_cereal -->


    <owl:Class rdf:about="http://www.owl-ontologies.com/VirtualHome.owl#eat_cereal">
        <rdfs:subClassOf rdf:resource="http://www.owl-ontologies.com/VirtualHome.owl#EatingDrinking"/>
        <rdfs:comment>The class with sequence of actions for eating cereals.</rdfs:comment>
    </owl:Class>
    


    <!-- http://www.owl-ontologies.com/VirtualHome.owl#eat_cheese -->


    <owl:Class rdf:about="http://www.owl-ontologies.com/VirtualHome.owl#eat_cheese">
        <rdfs:subClassOf rdf:resource="http://www.owl-ontologies.com/VirtualHome.owl#EatingDrinking"/>
        <rdfs:comment>The class with sequence of actions for eating cheese.</rdfs:comment>
    </owl:Class>
    


    <!-- http://www.owl-ontologies.com/VirtualHome.owl#eat_dessert -->


    <owl:Class rdf:about="http://www.owl-ontologies.com/VirtualHome.owl#eat_dessert">
        <rdfs:subClassOf rdf:resource="http://www.owl-ontologies.com/VirtualHome.owl#EatingDrinking"/>
        <rdfs:comment>The class with sequence of actions for eating dessert in any room.</rdfs:comment>
    </owl:Class>
    


    <!-- http://www.owl-ontologies.com/VirtualHome.owl#eat_dinner -->


    <owl:Class rdf:about="http://www.owl-ontologies.com/VirtualHome.owl#eat_dinner">
        <rdfs:subClassOf rdf:resource="http://www.owl-ontologies.com/VirtualHome.owl#EatingDrinking"/>
        <rdfs:comment>The class with sequence of actions for eating dinner only.</rdfs:comment>
    </owl:Class>
    


    <!-- http://www.owl-ontologies.com/VirtualHome.owl#eat_donuts -->


    <owl:Class rdf:about="http://www.owl-ontologies.com/VirtualHome.owl#eat_donuts">
        <rdfs:subClassOf rdf:resource="http://www.owl-ontologies.com/VirtualHome.owl#EatingDrinking"/>
        <rdfs:comment>The class with sequence of actions for eating donuts.</rdfs:comment>
    </owl:Class>
    


    <!-- http://www.owl-ontologies.com/VirtualHome.owl#eat_family_meals -->


    <owl:Class rdf:about="http://www.owl-ontologies.com/VirtualHome.owl#eat_family_meals">
        <rdfs:subClassOf rdf:resource="http://www.owl-ontologies.com/VirtualHome.owl#EatingDrinking"/>
        <rdfs:comment>The class with sequence of actions for eating meals with your family.</rdfs:comment>
    </owl:Class>
    


    <!-- http://www.owl-ontologies.com/VirtualHome.owl#eat_ice_cream -->


    <owl:Class rdf:about="http://www.owl-ontologies.com/VirtualHome.owl#eat_ice_cream">
        <rdfs:subClassOf rdf:resource="http://www.owl-ontologies.com/VirtualHome.owl#EatingDrinking"/>
        <rdfs:comment>The class with sequence of actions for eating ice cream in any room.</rdfs:comment>
    </owl:Class>
    


    <!-- http://www.owl-ontologies.com/VirtualHome.owl#eat_meals -->


    <owl:Class rdf:about="http://www.owl-ontologies.com/VirtualHome.owl#eat_meals">
        <rdfs:subClassOf rdf:resource="http://www.owl-ontologies.com/VirtualHome.owl#EatingDrinking"/>
        <rdfs:comment>The class with sequence of actions for eating meals.</rdfs:comment>
    </owl:Class>
    


    <!-- http://www.owl-ontologies.com/VirtualHome.owl#eat_on_fancy_china -->


    <owl:Class rdf:about="http://www.owl-ontologies.com/VirtualHome.owl#eat_on_fancy_china">
        <rdfs:subClassOf rdf:resource="http://www.owl-ontologies.com/VirtualHome.owl#EatingDrinking"/>
        <rdfs:comment>The class with sequence of actions for eating at fancy china.</rdfs:comment>
    </owl:Class>
    


    <!-- http://www.owl-ontologies.com/VirtualHome.owl#eat_snacks_and_drink_tea -->


    <owl:Class rdf:about="http://www.owl-ontologies.com/VirtualHome.owl#eat_snacks_and_drink_tea">
        <rdfs:subClassOf rdf:resource="http://www.owl-ontologies.com/VirtualHome.owl#EatingDrinking"/>
        <rdfs:comment>The class with sequence of actions for eating snacks and drinking tea.</rdfs:comment>
    </owl:Class>
    


    <!-- http://www.owl-ontologies.com/VirtualHome.owl#eat_while_watching_tv -->


    <owl:Class rdf:about="http://www.owl-ontologies.com/VirtualHome.owl#eat_while_watching_tv">
        <rdfs:subClassOf rdf:resource="http://www.owl-ontologies.com/VirtualHome.owl#EatingDrinking"/>
        <rdfs:subClassOf rdf:resource="http://www.owl-ontologies.com/VirtualHome.owl#Leisure"/>
        <rdfs:comment>The class with sequence of actions for eating something while watching 
TV.</rdfs:comment>
    </owl:Class>
    


    <!-- http://www.owl-ontologies.com/VirtualHome.owl#empty_dishwasher_and_fill_dishwasher -->


    <owl:Class rdf:about="http://www.owl-ontologies.com/VirtualHome.owl#empty_dishwasher_and_fill_dishwasher">
        <rdfs:subClassOf rdf:resource="http://www.owl-ontologies.com/VirtualHome.owl#HouseArrangement"/>
        <rdfs:comment>The class with sequence of actions for emptying dishwasher and fill 
dishwasher, in any room.</rdfs:comment>
    </owl:Class>
    


    <!-- http://www.owl-ontologies.com/VirtualHome.owl#enjoy_view_out_window -->


    <owl:Class rdf:about="http://www.owl-ontologies.com/VirtualHome.owl#enjoy_view_out_window">
        <rdfs:subClassOf rdf:resource="http://www.owl-ontologies.com/VirtualHome.owl#Other"/>
        <rdfs:comment>The class with sequence of actions for enjoying the view out of the 
window, in any room.</rdfs:comment>
    </owl:Class>
    


    <!-- http://www.owl-ontologies.com/VirtualHome.owl#enter_home -->


    <owl:Class rdf:about="http://www.owl-ontologies.com/VirtualHome.owl#enter_home">
        <rdfs:subClassOf rdf:resource="http://www.owl-ontologies.com/VirtualHome.owl#Other"/>
        <rdfs:comment>The class with sequence of actions for entering home.</rdfs:comment>
    </owl:Class>
    


    <!-- http://www.owl-ontologies.com/VirtualHome.owl#entertain -->


    <owl:Class rdf:about="http://www.owl-ontologies.com/VirtualHome.owl#entertain">
        <rdfs:subClassOf rdf:resource="http://www.owl-ontologies.com/VirtualHome.owl#SocialInteraction"/>
        <rdfs:comment>A class with sequences for entertaining your self with activities that 
have to do with other persons.</rdfs:comment>
    </owl:Class>
    


    <!-- http://www.owl-ontologies.com/VirtualHome.owl#exercise -->


    <owl:Class rdf:about="http://www.owl-ontologies.com/VirtualHome.owl#exercise">
        <rdfs:subClassOf rdf:resource="http://www.owl-ontologies.com/VirtualHome.owl#PhysicalActivity"/>
        <rdfs:comment>The class with sequence of actions for exercising.</rdfs:comment>
    </owl:Class>
    


    <!-- http://www.owl-ontologies.com/VirtualHome.owl#face_washing -->


    <owl:Class rdf:about="http://www.owl-ontologies.com/VirtualHome.owl#face_washing">
        <rdfs:subClassOf rdf:resource="http://www.owl-ontologies.com/VirtualHome.owl#HygieneStyling"/>
        <rdfs:comment>The class with sequence of actions for washing your face.</rdfs:comment>
    </owl:Class>
    


    <!-- http://www.owl-ontologies.com/VirtualHome.owl#family_meetings -->


    <owl:Class rdf:about="http://www.owl-ontologies.com/VirtualHome.owl#family_meetings">
        <rdfs:subClassOf rdf:resource="http://www.owl-ontologies.com/VirtualHome.owl#SocialInteraction"/>
        <rdfs:comment>The class with sequence of actions for family meetings.</rdfs:comment>
    </owl:Class>
    


    <!-- http://www.owl-ontologies.com/VirtualHome.owl#fan_magazines_on_coffee_table -->


    <owl:Class rdf:about="http://www.owl-ontologies.com/VirtualHome.owl#fan_magazines_on_coffee_table">
        <rdfs:subClassOf rdf:resource="http://www.owl-ontologies.com/VirtualHome.owl#Other"/>
        <rdfs:comment>The class with sequence of actions for fanning magazines on coffee table.</rdfs:comment>
    </owl:Class>
    


    <!-- http://www.owl-ontologies.com/VirtualHome.owl#fax_forms_to_doctor -->


    <owl:Class rdf:about="http://www.owl-ontologies.com/VirtualHome.owl#fax_forms_to_doctor">
        <rdfs:subClassOf rdf:resource="http://www.owl-ontologies.com/VirtualHome.owl#Work"/>
        <rdfs:comment>The class with sequence of actions to fax forms to a doctor only.</rdfs:comment>
    </owl:Class>
    


    <!-- http://www.owl-ontologies.com/VirtualHome.owl#feed_daughter -->


    <owl:Class rdf:about="http://www.owl-ontologies.com/VirtualHome.owl#feed_daughter">
        <rdfs:subClassOf rdf:resource="http://www.owl-ontologies.com/VirtualHome.owl#Other"/>
        <rdfs:comment>The class with sequence of actions for feeding your daughter.</rdfs:comment>
    </owl:Class>
    


    <!-- http://www.owl-ontologies.com/VirtualHome.owl#feed_dog -->


    <owl:Class rdf:about="http://www.owl-ontologies.com/VirtualHome.owl#feed_dog">
        <rdfs:subClassOf rdf:resource="http://www.owl-ontologies.com/VirtualHome.owl#Other"/>
        <rdfs:comment>The class with sequence of actions for feeding the dog.</rdfs:comment>
    </owl:Class>
    


    <!-- http://www.owl-ontologies.com/VirtualHome.owl#feed_me -->


    <owl:Class rdf:about="http://www.owl-ontologies.com/VirtualHome.owl#feed_me">
        <rdfs:subClassOf rdf:resource="http://www.owl-ontologies.com/VirtualHome.owl#Other"/>
        <rdfs:comment>The class with sequence of actions for feeding the user.</rdfs:comment>
    </owl:Class>
    


    <!-- http://www.owl-ontologies.com/VirtualHome.owl#file_documents -->


    <owl:Class rdf:about="http://www.owl-ontologies.com/VirtualHome.owl#file_documents">
        <rdfs:subClassOf rdf:resource="http://www.owl-ontologies.com/VirtualHome.owl#Work"/>
        <rdfs:comment>Class with sequences about how to file the documents.</rdfs:comment>
    </owl:Class>
    


    <!-- http://www.owl-ontologies.com/VirtualHome.owl#file_expense_reports -->


    <owl:Class rdf:about="http://www.owl-ontologies.com/VirtualHome.owl#file_expense_reports">
        <rdfs:subClassOf rdf:resource="http://www.owl-ontologies.com/VirtualHome.owl#Work"/>
        <rdfs:comment>The class with sequence of actions for performing file expense reports.</rdfs:comment>
    </owl:Class>
    


    <!-- http://www.owl-ontologies.com/VirtualHome.owl#find_dictionary -->


    <owl:Class rdf:about="http://www.owl-ontologies.com/VirtualHome.owl#find_dictionary">
        <rdfs:subClassOf rdf:resource="http://www.owl-ontologies.com/VirtualHome.owl#Other"/>
        <rdfs:comment>The class with sequence of actions for finding the dictionary, in any room search.</rdfs:comment>
    </owl:Class>
    


    <!-- http://www.owl-ontologies.com/VirtualHome.owl#find_some_food -->


    <owl:Class rdf:about="http://www.owl-ontologies.com/VirtualHome.owl#find_some_food">
        <rdfs:subClassOf rdf:resource="http://www.owl-ontologies.com/VirtualHome.owl#FoodPreparation"/>
    </owl:Class>
    


    <!-- http://www.owl-ontologies.com/VirtualHome.owl#fix_bowl_of_cereal -->


    <owl:Class rdf:about="http://www.owl-ontologies.com/VirtualHome.owl#fix_bowl_of_cereal">
        <rdfs:subClassOf rdf:resource="http://www.owl-ontologies.com/VirtualHome.owl#FoodPreparation"/>
        <rdfs:comment>The class with sequence of actions for fixing bowls of cereals (re 
arrange it if it has spilled, or make it look beautiful).</rdfs:comment>
    </owl:Class>
    


    <!-- http://www.owl-ontologies.com/VirtualHome.owl#fix_broken_toys -->


    <owl:Class rdf:about="http://www.owl-ontologies.com/VirtualHome.owl#fix_broken_toys">
        <rdfs:subClassOf rdf:resource="http://www.owl-ontologies.com/VirtualHome.owl#Other"/>
        <rdfs:comment>The class with sequence of actions for fixing broken toys, any toys in 
any room.</rdfs:comment>
    </owl:Class>
    


    <!-- http://www.owl-ontologies.com/VirtualHome.owl#fix_sandwhich -->


    <owl:Class rdf:about="http://www.owl-ontologies.com/VirtualHome.owl#fix_sandwhich">
        <rdfs:subClassOf rdf:resource="http://www.owl-ontologies.com/VirtualHome.owl#FoodPreparation"/>
        <rdfs:comment>The class with sequence of actions for fixing sandwhich (make it look 
beautifull, or if it has spilled what it has inside re arragne it).</rdfs:comment>
    </owl:Class>
    


    <!-- http://www.owl-ontologies.com/VirtualHome.owl#fix_sandwich -->


    <owl:Class rdf:about="http://www.owl-ontologies.com/VirtualHome.owl#fix_sandwich">
        <rdfs:subClassOf rdf:resource="http://www.owl-ontologies.com/VirtualHome.owl#FoodPreparation"/>
        <rdfs:comment>The class with sequence of actions for fixing a sandwhich.</rdfs:comment>
    </owl:Class>
    


    <!-- http://www.owl-ontologies.com/VirtualHome.owl#fix_snack -->


    <owl:Class rdf:about="http://www.owl-ontologies.com/VirtualHome.owl#fix_snack">
        <rdfs:subClassOf rdf:resource="http://www.owl-ontologies.com/VirtualHome.owl#FoodPreparation"/>
        <rdfs:comment>The class with sequence of actions for fixing a snack (make it look 
beautiful, or re arrange it if ti has beedn torn apart).</rdfs:comment>
    </owl:Class>
    


    <!-- http://www.owl-ontologies.com/VirtualHome.owl#fluff_pillow -->


    <owl:Class rdf:about="http://www.owl-ontologies.com/VirtualHome.owl#fluff_pillow">
        <rdfs:subClassOf rdf:resource="http://www.owl-ontologies.com/VirtualHome.owl#HouseArrangement"/>
        <rdfs:comment>The class with sequence of actions for fluffing a pillow, in any room.</rdfs:comment>
    </owl:Class>
    


    <!-- http://www.owl-ontologies.com/VirtualHome.owl#fluff_pillows -->


    <owl:Class rdf:about="http://www.owl-ontologies.com/VirtualHome.owl#fluff_pillows">
        <rdfs:subClassOf rdf:resource="http://www.owl-ontologies.com/VirtualHome.owl#HouseCleaning"/>
        <rdfs:comment>The class with sequence of actions for fluffing the pillows.</rdfs:comment>
    </owl:Class>
    


    <!-- http://www.owl-ontologies.com/VirtualHome.owl#flush_toilet -->


    <owl:Class rdf:about="http://www.owl-ontologies.com/VirtualHome.owl#flush_toilet">
        <rdfs:subClassOf rdf:resource="http://www.owl-ontologies.com/VirtualHome.owl#HouseCleaning"/>
        <rdfs:comment>The class with sequence of actions to flush down the toilet.</rdfs:comment>
    </owl:Class>
    


    <!-- http://www.owl-ontologies.com/VirtualHome.owl#fold_laundry -->


    <owl:Class rdf:about="http://www.owl-ontologies.com/VirtualHome.owl#fold_laundry">
        <rdfs:subClassOf rdf:resource="http://www.owl-ontologies.com/VirtualHome.owl#HouseArrangement"/>
        <rdfs:comment>Class with sequences about how to fold the different laundry objects 
(i.e. clothes, or objects that could be considered laundry).</rdfs:comment>
    </owl:Class>
    


    <!-- http://www.owl-ontologies.com/VirtualHome.owl#gaze_out_window -->


    <owl:Class rdf:about="http://www.owl-ontologies.com/VirtualHome.owl#gaze_out_window">
        <rdfs:subClassOf rdf:resource="http://www.owl-ontologies.com/VirtualHome.owl#Other"/>
        <rdfs:comment>The class with sequence of actions for gazing out the window.</rdfs:comment>
    </owl:Class>
    


    <!-- http://www.owl-ontologies.com/VirtualHome.owl#get_dressed -->


    <owl:Class rdf:about="http://www.owl-ontologies.com/VirtualHome.owl#get_dressed">
        <rdfs:subClassOf rdf:resource="http://www.owl-ontologies.com/VirtualHome.owl#HygieneStyling"/>
        <rdfs:comment>Class with sequences about how to get dressed for getting out, or for 
getting to work.</rdfs:comment>
    </owl:Class>
    


    <!-- http://www.owl-ontologies.com/VirtualHome.owl#get_drink -->


    <owl:Class rdf:about="http://www.owl-ontologies.com/VirtualHome.owl#get_drink">
        <rdfs:subClassOf rdf:resource="http://www.owl-ontologies.com/VirtualHome.owl#Other"/>
        <rdfs:comment>The class with sequence of actions for getting a drink, in any room.</rdfs:comment>
    </owl:Class>
    


    <!-- http://www.owl-ontologies.com/VirtualHome.owl#get_glass_of_milk -->


    <owl:Class rdf:about="http://www.owl-ontologies.com/VirtualHome.owl#get_glass_of_milk">
        <rdfs:subClassOf rdf:resource="http://www.owl-ontologies.com/VirtualHome.owl#Other"/>
        <rdfs:comment>The class with sequence of actions for getting a glass of milk, from any 
room the milk is in.</rdfs:comment>
    </owl:Class>
    


    <!-- http://www.owl-ontologies.com/VirtualHome.owl#get_glass_of_water -->


    <owl:Class rdf:about="http://www.owl-ontologies.com/VirtualHome.owl#get_glass_of_water">
        <rdfs:subClassOf rdf:resource="http://www.owl-ontologies.com/VirtualHome.owl#Other"/>
        <rdfs:comment>The class with sequence of actions for getting glass of water, from any 
room that can get water.</rdfs:comment>
    </owl:Class>
    


    <!-- http://www.owl-ontologies.com/VirtualHome.owl#get_in_way_of_guests_trying_to_leave -->


    <owl:Class rdf:about="http://www.owl-ontologies.com/VirtualHome.owl#get_in_way_of_guests_trying_to_leave">
        <rdfs:subClassOf rdf:resource="http://www.owl-ontologies.com/VirtualHome.owl#Other"/>
        <rdfs:comment>The class with sequence of actions for getting in way of guests.</rdfs:comment>
    </owl:Class>
    


    <!-- http://www.owl-ontologies.com/VirtualHome.owl#get_mail_ready -->


    <owl:Class rdf:about="http://www.owl-ontologies.com/VirtualHome.owl#get_mail_ready">
        <rdfs:subClassOf rdf:resource="http://www.owl-ontologies.com/VirtualHome.owl#Work"/>
        <rdfs:comment>The class with sequence of actions for getting an email ready to be send.</rdfs:comment>
    </owl:Class>
    


    <!-- http://www.owl-ontologies.com/VirtualHome.owl#get_out_dish -->


    <owl:Class rdf:about="http://www.owl-ontologies.com/VirtualHome.owl#get_out_dish">
        <rdfs:subClassOf rdf:resource="http://www.owl-ontologies.com/VirtualHome.owl#Other"/>
        <rdfs:comment>The class with sequence of actions for getting a dish out, for serving 
in any room.</rdfs:comment>
    </owl:Class>
    


    <!-- http://www.owl-ontologies.com/VirtualHome.owl#get_ready_for_bed -->


    <owl:Class rdf:about="http://www.owl-ontologies.com/VirtualHome.owl#get_ready_for_bed">
        <rdfs:subClassOf rdf:resource="http://www.owl-ontologies.com/VirtualHome.owl#BedTimeSleep"/>
        <rdfs:comment>\The class with sequence of actions for getting ready for going to bed.</rdfs:comment>
    </owl:Class>
    


    <!-- http://www.owl-ontologies.com/VirtualHome.owl#get_ready_for_day -->


    <owl:Class rdf:about="http://www.owl-ontologies.com/VirtualHome.owl#get_ready_for_day">
        <rdfs:subClassOf rdf:resource="http://www.owl-ontologies.com/VirtualHome.owl#GettingReady"/>
        <rdfs:comment>The class with sequence of actions for getting ready for the day.</rdfs:comment>
    </owl:Class>
    


    <!-- http://www.owl-ontologies.com/VirtualHome.owl#get_ready_for_school -->


    <owl:Class rdf:about="http://www.owl-ontologies.com/VirtualHome.owl#get_ready_for_school">
        <rdfs:subClassOf rdf:resource="http://www.owl-ontologies.com/VirtualHome.owl#GettingReady"/>
        <rdfs:comment>The class with sequence of actions for getting ready for school.</rdfs:comment>
    </owl:Class>
    


    <!-- http://www.owl-ontologies.com/VirtualHome.owl#get_ready_for_work -->


    <owl:Class rdf:about="http://www.owl-ontologies.com/VirtualHome.owl#get_ready_for_work">
        <rdfs:subClassOf rdf:resource="http://www.owl-ontologies.com/VirtualHome.owl#GettingReady"/>
        <rdfs:comment>The class with sequence of actions for gettinf ready to go to work.</rdfs:comment>
    </owl:Class>
    


    <!-- http://www.owl-ontologies.com/VirtualHome.owl#get_ready_to_leave -->


    <owl:Class rdf:about="http://www.owl-ontologies.com/VirtualHome.owl#get_ready_to_leave">
        <rdfs:subClassOf rdf:resource="http://www.owl-ontologies.com/VirtualHome.owl#GettingReady"/>
        <rdfs:comment>The class with sequence of actions for getting ready to leave the house.</rdfs:comment>
    </owl:Class>
    


    <!-- http://www.owl-ontologies.com/VirtualHome.owl#get_some_water -->


    <owl:Class rdf:about="http://www.owl-ontologies.com/VirtualHome.owl#get_some_water">
        <rdfs:subClassOf rdf:resource="http://www.owl-ontologies.com/VirtualHome.owl#Other"/>
        <rdfs:comment>The class with sequence of actions for getting some water.</rdfs:comment>
    </owl:Class>
    


    <!-- http://www.owl-ontologies.com/VirtualHome.owl#get_something_to_drink -->


    <owl:Class rdf:about="http://www.owl-ontologies.com/VirtualHome.owl#get_something_to_drink">
        <rdfs:subClassOf rdf:resource="http://www.owl-ontologies.com/VirtualHome.owl#EatingDrinking"/>
        <rdfs:comment>The class with sequence of actions for getting something to drink.</rdfs:comment>
    </owl:Class>
    


    <!-- http://www.owl-ontologies.com/VirtualHome.owl#get_toilet_paper -->


    <owl:Class rdf:about="http://www.owl-ontologies.com/VirtualHome.owl#get_toilet_paper">
        <rdfs:subClassOf rdf:resource="http://www.owl-ontologies.com/VirtualHome.owl#Other"/>
        <rdfs:comment>The class with sequence of actions for getting toilet paper from any 
room and put it in the toilet.</rdfs:comment>
    </owl:Class>
    


    <!-- http://www.owl-ontologies.com/VirtualHome.owl#getting__dresses -->


    <owl:Class rdf:about="http://www.owl-ontologies.com/VirtualHome.owl#getting__dresses">
        <rdfs:subClassOf rdf:resource="http://www.owl-ontologies.com/VirtualHome.owl#Other"/>
        <rdfs:comment>The class with sequence of actions for getting dresses.</rdfs:comment>
    </owl:Class>
    


    <!-- http://www.owl-ontologies.com/VirtualHome.owl#getting_dressed -->


    <owl:Class rdf:about="http://www.owl-ontologies.com/VirtualHome.owl#getting_dressed">
        <rdfs:subClassOf rdf:resource="http://www.owl-ontologies.com/VirtualHome.owl#HygieneStyling"/>
        <rdfs:comment>The class with sequence of actions for getting dressed.</rdfs:comment>
    </owl:Class>
    


    <!-- http://www.owl-ontologies.com/VirtualHome.owl#getting_in_way_of_guest_trying_to_leave -->


    <owl:Class rdf:about="http://www.owl-ontologies.com/VirtualHome.owl#getting_in_way_of_guest_trying_to_leave">
        <rdfs:subClassOf rdf:resource="http://www.owl-ontologies.com/VirtualHome.owl#SocialInteraction"/>
        <rdfs:comment>The class with sequence of actions for getting in way of guest trying to 
leave.</rdfs:comment>
    </owl:Class>
    


    <!-- http://www.owl-ontologies.com/VirtualHome.owl#give_children_bath -->


    <owl:Class rdf:about="http://www.owl-ontologies.com/VirtualHome.owl#give_children_bath">
        <rdfs:subClassOf rdf:resource="http://www.owl-ontologies.com/VirtualHome.owl#HygieneStyling"/>
        <rdfs:subClassOf rdf:resource="http://www.owl-ontologies.com/VirtualHome.owl#SocialInteraction"/>
        <rdfs:comment>The class with sequence of actions for giving the children a bath.</rdfs:comment>
        <rdfs:comment>The class with sequence of actions for giving your children a bath.</rdfs:comment>
    </owl:Class>
    


    <!-- http://www.owl-ontologies.com/VirtualHome.owl#give_me_bath -->


    <owl:Class rdf:about="http://www.owl-ontologies.com/VirtualHome.owl#give_me_bath">
        <rdfs:subClassOf rdf:resource="http://www.owl-ontologies.com/VirtualHome.owl#HygieneStyling"/>
        <rdfs:comment>The class with sequence of actions for giving a bath to the user.</rdfs:comment>
    </owl:Class>
    


    <!-- http://www.owl-ontologies.com/VirtualHome.owl#give_milk_to_cat -->


    <owl:Class rdf:about="http://www.owl-ontologies.com/VirtualHome.owl#give_milk_to_cat">
        <rdfs:subClassOf rdf:resource="http://www.owl-ontologies.com/VirtualHome.owl#Other"/>
        <rdfs:comment>The class with sequence of actions for giving milk to the cat, inside 
the house, but in any room.</rdfs:comment>
    </owl:Class>
    


    <!-- http://www.owl-ontologies.com/VirtualHome.owl#give_your_child_bath -->


    <owl:Class rdf:about="http://www.owl-ontologies.com/VirtualHome.owl#give_your_child_bath">
        <rdfs:subClassOf rdf:resource="http://www.owl-ontologies.com/VirtualHome.owl#HygieneStyling"/>
        <rdfs:comment>The class with sequence of actions for giving you child bath.</rdfs:comment>
    </owl:Class>
    


    <!-- http://www.owl-ontologies.com/VirtualHome.owl#go_pee -->


    <owl:Class rdf:about="http://www.owl-ontologies.com/VirtualHome.owl#go_pee">
        <rdfs:subClassOf rdf:resource="http://www.owl-ontologies.com/VirtualHome.owl#HygieneStyling"/>
        <rdfs:comment>The class with sequence of actions for going to pee.</rdfs:comment>
    </owl:Class>
    


    <!-- http://www.owl-ontologies.com/VirtualHome.owl#go_to_bathroom -->


    <owl:Class rdf:about="http://www.owl-ontologies.com/VirtualHome.owl#go_to_bathroom">
        <rdfs:subClassOf rdf:resource="http://www.owl-ontologies.com/VirtualHome.owl#HygieneStyling"/>
        <rdfs:comment>The class with sequence of actions for going to the bathroom.</rdfs:comment>
    </owl:Class>
    


    <!-- http://www.owl-ontologies.com/VirtualHome.owl#go_to_bed -->


    <owl:Class rdf:about="http://www.owl-ontologies.com/VirtualHome.owl#go_to_bed">
        <rdfs:subClassOf rdf:resource="http://www.owl-ontologies.com/VirtualHome.owl#BedTimeSleep"/>
        <rdfs:comment>The class with sequence of actions for going to bed.</rdfs:comment>
    </owl:Class>
    


    <!-- http://www.owl-ontologies.com/VirtualHome.owl#go_to_sleep -->


    <owl:Class rdf:about="http://www.owl-ontologies.com/VirtualHome.owl#go_to_sleep">
        <rdfs:subClassOf rdf:resource="http://www.owl-ontologies.com/VirtualHome.owl#BedTimeSleep"/>
        <rdfs:comment>A class with sequences on how to go to sleep, or get ready to go to 
sleep.</rdfs:comment>
    </owl:Class>
    


    <!-- http://www.owl-ontologies.com/VirtualHome.owl#go_to_toilet -->


    <owl:Class rdf:about="http://www.owl-ontologies.com/VirtualHome.owl#go_to_toilet">
        <rdfs:subClassOf rdf:resource="http://www.owl-ontologies.com/VirtualHome.owl#HygieneStyling"/>
        <rdfs:comment>Class with seqeunces on how to go to toilet.</rdfs:comment>
    </owl:Class>
    


    <!-- http://www.owl-ontologies.com/VirtualHome.owl#grab_some_juice -->


    <owl:Class rdf:about="http://www.owl-ontologies.com/VirtualHome.owl#grab_some_juice">
        <rdfs:subClassOf rdf:resource="http://www.owl-ontologies.com/VirtualHome.owl#Other"/>
        <rdfs:comment>The class with sequence of actions for grabing some juice, from the 
fridge or elsewhere.</rdfs:comment>
    </owl:Class>
    


    <!-- http://www.owl-ontologies.com/VirtualHome.owl#grab_things -->


    <owl:Class rdf:about="http://www.owl-ontologies.com/VirtualHome.owl#grab_things">
        <rdfs:subClassOf rdf:resource="http://www.owl-ontologies.com/VirtualHome.owl#Other"/>
        <rdfs:comment>The class with sequence of actions for grabing things, any object.</rdfs:comment>
    </owl:Class>
    


    <!-- http://www.owl-ontologies.com/VirtualHome.owl#grading_papers -->


    <owl:Class rdf:about="http://www.owl-ontologies.com/VirtualHome.owl#grading_papers">
        <rdfs:subClassOf rdf:resource="http://www.owl-ontologies.com/VirtualHome.owl#Work"/>
        <rdfs:comment>The class with sequence of actions for grading some papers (usually for 
school).</rdfs:comment>
    </owl:Class>
    


    <!-- http://www.owl-ontologies.com/VirtualHome.owl#greet_guests -->


    <owl:Class rdf:about="http://www.owl-ontologies.com/VirtualHome.owl#greet_guests">
        <rdfs:subClassOf rdf:resource="http://www.owl-ontologies.com/VirtualHome.owl#SocialInteraction"/>
        <rdfs:comment>A class with sequences for greeting guest that have come to your home for visit</rdfs:comment>
    </owl:Class>
    


    <!-- http://www.owl-ontologies.com/VirtualHome.owl#greet_people -->


    <owl:Class rdf:about="http://www.owl-ontologies.com/VirtualHome.owl#greet_people">
        <rdfs:subClassOf rdf:resource="http://www.owl-ontologies.com/VirtualHome.owl#SocialInteraction"/>
        <rdfs:comment>The class with sequence of actions for greeting people in any room or outside the house.</rdfs:comment>
    </owl:Class>
    


    <!-- http://www.owl-ontologies.com/VirtualHome.owl#hair -->


    <owl:Class rdf:about="http://www.owl-ontologies.com/VirtualHome.owl#hair">
        <rdfs:subClassOf rdf:resource="http://www.owl-ontologies.com/VirtualHome.owl#Other"/>
        <rdfs:comment>The class with sequence of actions for hairing.</rdfs:comment>
    </owl:Class>
    


    <!-- http://www.owl-ontologies.com/VirtualHome.owl#hair_dressing -->


    <owl:Class rdf:about="http://www.owl-ontologies.com/VirtualHome.owl#hair_dressing">
        <rdfs:subClassOf rdf:resource="http://www.owl-ontologies.com/VirtualHome.owl#HygieneStyling"/>
        <rdfs:comment>The class with sequence of actions for hair dressing.</rdfs:comment>
    </owl:Class>
    


    <!-- http://www.owl-ontologies.com/VirtualHome.owl#hand_washing -->


    <owl:Class rdf:about="http://www.owl-ontologies.com/VirtualHome.owl#hand_washing">
        <rdfs:subClassOf rdf:resource="http://www.owl-ontologies.com/VirtualHome.owl#HygieneStyling"/>
        <rdfs:comment>The class with sequence of actions for hand washing, in any room.</rdfs:comment>
    </owl:Class>
    


    <!-- http://www.owl-ontologies.com/VirtualHome.owl#hang_car_keys -->


    <owl:Class rdf:about="http://www.owl-ontologies.com/VirtualHome.owl#hang_car_keys">
        <rdfs:subClassOf rdf:resource="http://www.owl-ontologies.com/VirtualHome.owl#Other"/>
        <rdfs:comment>The class with sequence of actions for hanging car keys, in any place 
that can be hanged.</rdfs:comment>
    </owl:Class>
    


    <!-- http://www.owl-ontologies.com/VirtualHome.owl#hang_keys -->


    <owl:Class rdf:about="http://www.owl-ontologies.com/VirtualHome.owl#hang_keys">
        <rdfs:subClassOf rdf:resource="http://www.owl-ontologies.com/VirtualHome.owl#Other"/>
        <rdfs:comment>The class with sequence of actions for hanging up keys in any room.</rdfs:comment>
    </owl:Class>
    


    <!-- http://www.owl-ontologies.com/VirtualHome.owl#hang_out -->


    <owl:Class rdf:about="http://www.owl-ontologies.com/VirtualHome.owl#hang_out">
        <rdfs:subClassOf rdf:resource="http://www.owl-ontologies.com/VirtualHome.owl#Other"/>
        <rdfs:comment>The class with sequence of actions for hanging out, speending free time in house.</rdfs:comment>
    </owl:Class>
    


    <!-- http://www.owl-ontologies.com/VirtualHome.owl#hang_pictures -->


    <owl:Class rdf:about="http://www.owl-ontologies.com/VirtualHome.owl#hang_pictures">
        <rdfs:subClassOf rdf:resource="http://www.owl-ontologies.com/VirtualHome.owl#HouseArrangement"/>
        <rdfs:comment>The class with sequence of actions for hanging out a picture in any room.</rdfs:comment>
    </owl:Class>
    


    <!-- http://www.owl-ontologies.com/VirtualHome.owl#hang_up_car_keys -->


    <owl:Class rdf:about="http://www.owl-ontologies.com/VirtualHome.owl#hang_up_car_keys">
        <rdfs:subClassOf rdf:resource="http://www.owl-ontologies.com/VirtualHome.owl#Other"/>
        <rdfs:comment>The class with sequence of actions for hanging up your car keys, in 
every room.</rdfs:comment>
    </owl:Class>
    


    <!-- http://www.owl-ontologies.com/VirtualHome.owl#hang_up_jacket -->


    <owl:Class rdf:about="http://www.owl-ontologies.com/VirtualHome.owl#hang_up_jacket">
        <rdfs:subClassOf rdf:resource="http://www.owl-ontologies.com/VirtualHome.owl#Other"/>
        <rdfs:comment>A class with sequences on how to hang up your jacket
.</rdfs:comment>
    </owl:Class>
    


    <!-- http://www.owl-ontologies.com/VirtualHome.owl#hang_up_poster -->


    <owl:Class rdf:about="http://www.owl-ontologies.com/VirtualHome.owl#hang_up_poster">
        <rdfs:subClassOf rdf:resource="http://www.owl-ontologies.com/VirtualHome.owl#HouseArrangement"/>
        <rdfs:comment>The class with sequence of actions for hanging up the poster in any room.</rdfs:comment>
    </owl:Class>
    


    <!-- http://www.owl-ontologies.com/VirtualHome.owl#hang_with_friend -->


    <owl:Class rdf:about="http://www.owl-ontologies.com/VirtualHome.owl#hang_with_friend">
        <rdfs:subClassOf rdf:resource="http://www.owl-ontologies.com/VirtualHome.owl#SocialInteraction"/>
        <rdfs:comment>The class with sequence of actions for hanging with your friend inside 
the house.</rdfs:comment>
    </owl:Class>
    


    <!-- http://www.owl-ontologies.com/VirtualHome.owl#hang_with_friends -->


    <owl:Class rdf:about="http://www.owl-ontologies.com/VirtualHome.owl#hang_with_friends">
        <rdfs:subClassOf rdf:resource="http://www.owl-ontologies.com/VirtualHome.owl#Other"/>
        <rdfs:comment>The class with sequence of actions for hanging with friends.</rdfs:comment>
    </owl:Class>
    


    <!-- http://www.owl-ontologies.com/VirtualHome.owl#have_conversation_with_boyfriend -->


    <owl:Class rdf:about="http://www.owl-ontologies.com/VirtualHome.owl#have_conversation_with_boyfriend">
        <rdfs:subClassOf rdf:resource="http://www.owl-ontologies.com/VirtualHome.owl#SocialInteraction"/>
        <rdfs:comment>The class with sequence of actions for having conversation with your 
boyfriend.</rdfs:comment>
    </owl:Class>
    


    <!-- http://www.owl-ontologies.com/VirtualHome.owl#have_dinner -->


    <owl:Class rdf:about="http://www.owl-ontologies.com/VirtualHome.owl#have_dinner">
        <rdfs:subClassOf rdf:resource="http://www.owl-ontologies.com/VirtualHome.owl#EatingDrinking"/>
        <rdfs:comment>The class with sequence of actions for having dinner.</rdfs:comment>
    </owl:Class>
    


    <!-- http://www.owl-ontologies.com/VirtualHome.owl#have_ice_coffee -->


    <owl:Class rdf:about="http://www.owl-ontologies.com/VirtualHome.owl#have_ice_coffee">
        <rdfs:subClassOf rdf:resource="http://www.owl-ontologies.com/VirtualHome.owl#EatingDrinking"/>
        <rdfs:comment>The class with sequence of actions for drinking ice coffee in any room.</rdfs:comment>
    </owl:Class>
    


    <!-- http://www.owl-ontologies.com/VirtualHome.owl#have_party -->


    <owl:Class rdf:about="http://www.owl-ontologies.com/VirtualHome.owl#have_party">
        <rdfs:subClassOf rdf:resource="http://www.owl-ontologies.com/VirtualHome.owl#SocialInteraction"/>
        <rdfs:comment>The class with sequence of actions for having a party inside the house.</rdfs:comment>
    </owl:Class>
    


    <!-- http://www.owl-ontologies.com/VirtualHome.owl#have_quality_family_time -->


    <owl:Class rdf:about="http://www.owl-ontologies.com/VirtualHome.owl#have_quality_family_time">
        <rdfs:subClassOf rdf:resource="http://www.owl-ontologies.com/VirtualHome.owl#SocialInteraction"/>
        <rdfs:comment>The class with sequence of actions for having qualtiy family time, no matter the members if the family.</rdfs:comment>
    </owl:Class>
    


    <!-- http://www.owl-ontologies.com/VirtualHome.owl#have_snack -->


    <owl:Class rdf:about="http://www.owl-ontologies.com/VirtualHome.owl#have_snack">
        <rdfs:subClassOf rdf:resource="http://www.owl-ontologies.com/VirtualHome.owl#EatingDrinking"/>
        <rdfs:comment>The class with sequence of actions for having a snack at any time of the 
day.</rdfs:comment>
    </owl:Class>
    


    <!-- http://www.owl-ontologies.com/VirtualHome.owl#have_tea_party -->


    <owl:Class rdf:about="http://www.owl-ontologies.com/VirtualHome.owl#have_tea_party">
        <rdfs:subClassOf rdf:resource="http://www.owl-ontologies.com/VirtualHome.owl#SocialInteraction"/>
        <rdfs:comment>The class with sequence of actions for having a tea party.</rdfs:comment>
    </owl:Class>
    


    <!-- http://www.owl-ontologies.com/VirtualHome.owl#help_kids_with_homework -->


    <owl:Class rdf:about="http://www.owl-ontologies.com/VirtualHome.owl#help_kids_with_homework">
        <rdfs:subClassOf rdf:resource="http://www.owl-ontologies.com/VirtualHome.owl#SocialInteraction"/>
        <rdfs:comment>The class with sequence of actions for helping kids with their homework.</rdfs:comment>
    </owl:Class>
    


    <!-- http://www.owl-ontologies.com/VirtualHome.owl#help_organize_files -->


    <owl:Class rdf:about="http://www.owl-ontologies.com/VirtualHome.owl#help_organize_files">
        <rdfs:subClassOf rdf:resource="http://www.owl-ontologies.com/VirtualHome.owl#Other"/>
        <rdfs:comment>The class with sequence of actions for helping organize the files, in 
any order.</rdfs:comment>
    </owl:Class>
    


    <!-- http://www.owl-ontologies.com/VirtualHome.owl#help_with_quiz_shows -->


    <owl:Class rdf:about="http://www.owl-ontologies.com/VirtualHome.owl#help_with_quiz_shows">
        <rdfs:subClassOf rdf:resource="http://www.owl-ontologies.com/VirtualHome.owl#Other"/>
        <rdfs:comment>The class with sequence of actions for helping with quiz shows, any 
person.</rdfs:comment>
    </owl:Class>
    


    <!-- http://www.owl-ontologies.com/VirtualHome.owl#hide -->


    <owl:Class rdf:about="http://www.owl-ontologies.com/VirtualHome.owl#hide">
        <rdfs:subClassOf rdf:resource="http://www.owl-ontologies.com/VirtualHome.owl#Other"/>
        <rdfs:comment>The class with sequence of actions for hiding in any room.</rdfs:comment>
    </owl:Class>
    


    <!-- http://www.owl-ontologies.com/VirtualHome.owl#hold_coats_and_umbrellas -->


    <owl:Class rdf:about="http://www.owl-ontologies.com/VirtualHome.owl#hold_coats_and_umbrellas">
        <rdfs:subClassOf rdf:resource="http://www.owl-ontologies.com/VirtualHome.owl#HouseArrangement"/>
        <rdfs:comment>The class with sequence of actions for holding your coat (or coats) and 
an umbrella.</rdfs:comment>
    </owl:Class>
    


    <!-- http://www.owl-ontologies.com/VirtualHome.owl#homework -->


    <owl:Class rdf:about="http://www.owl-ontologies.com/VirtualHome.owl#homework">
        <rdfs:subClassOf rdf:resource="http://www.owl-ontologies.com/VirtualHome.owl#Work"/>
        <rdfs:comment>The class with sequence of actions for actions for getting ready for homework.</rdfs:comment>
    </owl:Class>
    


    <!-- http://www.owl-ontologies.com/VirtualHome.owl#ignore_people -->


    <owl:Class rdf:about="http://www.owl-ontologies.com/VirtualHome.owl#ignore_people">
        <rdfs:subClassOf rdf:resource="http://www.owl-ontologies.com/VirtualHome.owl#SocialInteraction"/>
        <rdfs:comment>The class with sequence of actions for ignoring the people inside the room.</rdfs:comment>
    </owl:Class>
    


    <!-- http://www.owl-ontologies.com/VirtualHome.owl#in_living_room_i_eat_dinner -->


    <owl:Class rdf:about="http://www.owl-ontologies.com/VirtualHome.owl#in_living_room_i_eat_dinner">
        <rdfs:subClassOf rdf:resource="http://www.owl-ontologies.com/VirtualHome.owl#Leisure"/>
        <rdfs:comment>The class with sequence of actions for eating dinner in living room.</rdfs:comment>
    </owl:Class>
    


    <!-- http://www.owl-ontologies.com/VirtualHome.owl#iron_shirt -->


    <owl:Class rdf:about="http://www.owl-ontologies.com/VirtualHome.owl#iron_shirt">
        <rdfs:subClassOf rdf:resource="http://www.owl-ontologies.com/VirtualHome.owl#HouseArrangement"/>
        <rdfs:comment>The class with sequence of actions for ironing a shirt in any place or 
room.</rdfs:comment>
    </owl:Class>
    


    <!-- http://www.owl-ontologies.com/VirtualHome.owl#juggling -->


    <owl:Class rdf:about="http://www.owl-ontologies.com/VirtualHome.owl#juggling">
        <rdfs:subClassOf rdf:resource="http://www.owl-ontologies.com/VirtualHome.owl#Leisure"/>
        <rdfs:comment>The class with sequence of actions for juggling (whatever object can 
fly).</rdfs:comment>
    </owl:Class>
    


    <!-- http://www.owl-ontologies.com/VirtualHome.owl#keep_an_eye_on_stove_as_something_is_cooking -->


    <owl:Class rdf:about="http://www.owl-ontologies.com/VirtualHome.owl#keep_an_eye_on_stove_as_something_is_cooking">
        <rdfs:subClassOf rdf:resource="http://www.owl-ontologies.com/VirtualHome.owl#FoodPreparation"/>
        <rdfs:comment>The class with sequence of actions for keeping an eye on stove as 
somehting is cooking.</rdfs:comment>
    </owl:Class>
    


    <!-- http://www.owl-ontologies.com/VirtualHome.owl#keep_cats_inside_while_door_is_open -->


    <owl:Class rdf:about="http://www.owl-ontologies.com/VirtualHome.owl#keep_cats_inside_while_door_is_open">
        <rdfs:subClassOf rdf:resource="http://www.owl-ontologies.com/VirtualHome.owl#Other"/>
        <rdfs:comment>The class with sequence of actions for trying to keep cats inside while 
door is open.</rdfs:comment>
    </owl:Class>
    


    <!-- http://www.owl-ontologies.com/VirtualHome.owl#keep_cats_out_of_room -->


    <owl:Class rdf:about="http://www.owl-ontologies.com/VirtualHome.owl#keep_cats_out_of_room">
        <rdfs:subClassOf rdf:resource="http://www.owl-ontologies.com/VirtualHome.owl#SocialInteraction"/>
        <rdfs:comment>The class with sequence of actions for keepin the cats out of room
, any room.</rdfs:comment>
    </owl:Class>
    


    <!-- http://www.owl-ontologies.com/VirtualHome.owl#lay_down_on_floor_and_say_im_rug -->


    <owl:Class rdf:about="http://www.owl-ontologies.com/VirtualHome.owl#lay_down_on_floor_and_say_im_rug">
        <rdfs:subClassOf rdf:resource="http://www.owl-ontologies.com/VirtualHome.owl#Other"/>
        <rdfs:comment>The class with sequence of actions for laying down on floor in any room 
and say, I am rug.</rdfs:comment>
    </owl:Class>
    


    <!-- http://www.owl-ontologies.com/VirtualHome.owl#lay_tablecloth -->


    <owl:Class rdf:about="http://www.owl-ontologies.com/VirtualHome.owl#lay_tablecloth">
        <rdfs:subClassOf rdf:resource="http://www.owl-ontologies.com/VirtualHome.owl#HouseArrangement"/>
        <rdfs:comment>The class with sequence of actions for laying the tablecoth on the 
table, in any room.</rdfs:comment>
    </owl:Class>
    


    <!-- http://www.owl-ontologies.com/VirtualHome.owl#leave_home -->


    <owl:Class rdf:about="http://www.owl-ontologies.com/VirtualHome.owl#leave_home">
        <rdfs:subClassOf rdf:resource="http://www.owl-ontologies.com/VirtualHome.owl#Other"/>
        <rdfs:comment>The class with sequence of actions for leaving home.</rdfs:comment>
    </owl:Class>
    


    <!-- http://www.owl-ontologies.com/VirtualHome.owl#let_baby_learn_how_to_walk -->


    <owl:Class rdf:about="http://www.owl-ontologies.com/VirtualHome.owl#let_baby_learn_how_to_walk">
        <rdfs:subClassOf rdf:resource="http://www.owl-ontologies.com/VirtualHome.owl#Other"/>
        <rdfs:comment>The class with sequence of actions for letting the baby learn how to walk.</rdfs:comment>
    </owl:Class>
    


    <!-- http://www.owl-ontologies.com/VirtualHome.owl#let_bay_learn_how_to_walk -->


    <owl:Class rdf:about="http://www.owl-ontologies.com/VirtualHome.owl#let_bay_learn_how_to_walk">
        <rdfs:subClassOf rdf:resource="http://www.owl-ontologies.com/VirtualHome.owl#SocialInteraction"/>
        <rdfs:comment>The class with sequence of actions for letting your child or baby to 
learn how to walk.</rdfs:comment>
    </owl:Class>
    


    <!-- http://www.owl-ontologies.com/VirtualHome.owl#light_candle -->


    <owl:Class rdf:about="http://www.owl-ontologies.com/VirtualHome.owl#light_candle">
        <rdfs:subClassOf rdf:resource="http://www.owl-ontologies.com/VirtualHome.owl#Other"/>
        <rdfs:comment>The class with sequence of actions for lighting up a candle in any room.</rdfs:comment>
    </owl:Class>
    


    <!-- http://www.owl-ontologies.com/VirtualHome.owl#light_candles -->


    <owl:Class rdf:about="http://www.owl-ontologies.com/VirtualHome.owl#light_candles">
        <rdfs:subClassOf rdf:resource="http://www.owl-ontologies.com/VirtualHome.owl#HouseArrangement"/>
        <rdfs:comment>The class with sequence of actions for lighting up the candles.</rdfs:comment>
    </owl:Class>
    


    <!-- http://www.owl-ontologies.com/VirtualHome.owl#listen_to_music -->


    <owl:Class rdf:about="http://www.owl-ontologies.com/VirtualHome.owl#listen_to_music">
        <rdfs:subClassOf rdf:resource="http://www.owl-ontologies.com/VirtualHome.owl#Leisure"/>
        <rdfs:comment>The class which contains sequences for listening to music.</rdfs:comment>
    </owl:Class>
    


    <!-- http://www.owl-ontologies.com/VirtualHome.owl#load_dishwasher -->


    <owl:Class rdf:about="http://www.owl-ontologies.com/VirtualHome.owl#load_dishwasher">
        <rdfs:subClassOf rdf:resource="http://www.owl-ontologies.com/VirtualHome.owl#HouseArrangement"/>
        <rdfs:comment>The class with sequence of actions for laoding up the dishwasher
.</rdfs:comment>
    </owl:Class>
    


    <!-- http://www.owl-ontologies.com/VirtualHome.owl#lock_door -->


    <owl:Class rdf:about="http://www.owl-ontologies.com/VirtualHome.owl#lock_door">
        <rdfs:subClassOf rdf:resource="http://www.owl-ontologies.com/VirtualHome.owl#Other"/>
        <rdfs:comment>The class with sequence of actions for locking the door in any room.</rdfs:comment>
    </owl:Class>
    


    <!-- http://www.owl-ontologies.com/VirtualHome.owl#look_at_mirror -->


    <owl:Class rdf:about="http://www.owl-ontologies.com/VirtualHome.owl#look_at_mirror">
        <rdfs:subClassOf rdf:resource="http://www.owl-ontologies.com/VirtualHome.owl#Other"/>
        <rdfs:comment>The class with sequence of actions for looking at the mirror in any room.</rdfs:comment>
    </owl:Class>
    


    <!-- http://www.owl-ontologies.com/VirtualHome.owl#look_at_painting -->


    <owl:Class rdf:about="http://www.owl-ontologies.com/VirtualHome.owl#look_at_painting">
        <rdfs:subClassOf rdf:resource="http://www.owl-ontologies.com/VirtualHome.owl#Other"/>
        <rdfs:comment>The class with sequence of actions for looki g at painting in any room.</rdfs:comment>
    </owl:Class>
    


    <!-- http://www.owl-ontologies.com/VirtualHome.owl#look_in_refrigerator -->


    <owl:Class rdf:about="http://www.owl-ontologies.com/VirtualHome.owl#look_in_refrigerator">
        <rdfs:subClassOf rdf:resource="http://www.owl-ontologies.com/VirtualHome.owl#Other"/>
        <rdfs:comment>The class with sequence of actions for looking in refrigerator for any 
reason.</rdfs:comment>
    </owl:Class>
    


    <!-- http://www.owl-ontologies.com/VirtualHome.owl#look_out_window -->


    <owl:Class rdf:about="http://www.owl-ontologies.com/VirtualHome.owl#look_out_window">
        <rdfs:subClassOf rdf:resource="http://www.owl-ontologies.com/VirtualHome.owl#Other"/>
        <rdfs:comment>The class with sequence of actions for looking out the window, in any 
room.</rdfs:comment>
    </owl:Class>
    


    <!-- http://www.owl-ontologies.com/VirtualHome.owl#mail_signed_letter_to_customer -->


    <owl:Class rdf:about="http://www.owl-ontologies.com/VirtualHome.owl#mail_signed_letter_to_customer">
        <rdfs:subClassOf rdf:resource="http://www.owl-ontologies.com/VirtualHome.owl#Work"/>
        <rdfs:comment>The class with sequence of actions read-send a mail that contains a 
signed letter for the customer.</rdfs:comment>
    </owl:Class>
    


    <!-- http://www.owl-ontologies.com/VirtualHome.owl#make__cookies -->


    <owl:Class rdf:about="http://www.owl-ontologies.com/VirtualHome.owl#make__cookies">
        <rdfs:subClassOf rdf:resource="http://www.owl-ontologies.com/VirtualHome.owl#FoodPreparation"/>
        <rdfs:comment>The class with sequence of actions for making cookies in any room.</rdfs:comment>
    </owl:Class>
    


    <!-- http://www.owl-ontologies.com/VirtualHome.owl#make_banana_bread -->


    <owl:Class rdf:about="http://www.owl-ontologies.com/VirtualHome.owl#make_banana_bread">
        <rdfs:subClassOf rdf:resource="http://www.owl-ontologies.com/VirtualHome.owl#FoodPreparation"/>
        <rdfs:comment>The class with sequence of actions for making a bread that contains 
banana.</rdfs:comment>
    </owl:Class>
    


    <!-- http://www.owl-ontologies.com/VirtualHome.owl#make_bed -->


    <owl:Class rdf:about="http://www.owl-ontologies.com/VirtualHome.owl#make_bed">
        <rdfs:subClassOf rdf:resource="http://www.owl-ontologies.com/VirtualHome.owl#HouseArrangement"/>
        <rdfs:comment>Class with sequences about how to make you own bed, under different 
circumstances.</rdfs:comment>
    </owl:Class>
    


    <!-- http://www.owl-ontologies.com/VirtualHome.owl#make_cereal -->


    <owl:Class rdf:about="http://www.owl-ontologies.com/VirtualHome.owl#make_cereal">
        <rdfs:subClassOf rdf:resource="http://www.owl-ontologies.com/VirtualHome.owl#FoodPreparation"/>
        <rdfs:comment>The class with sequence of actions for making cereals.</rdfs:comment>
    </owl:Class>
    


    <!-- http://www.owl-ontologies.com/VirtualHome.owl#make_childs_bed -->


    <owl:Class rdf:about="http://www.owl-ontologies.com/VirtualHome.owl#make_childs_bed">
        <rdfs:subClassOf rdf:resource="http://www.owl-ontologies.com/VirtualHome.owl#HouseArrangement"/>
        <rdfs:comment>The class with sequence of actions for making the childs bed in any room.</rdfs:comment>
    </owl:Class>
    


    <!-- http://www.owl-ontologies.com/VirtualHome.owl#make_coffee -->


    <owl:Class rdf:about="http://www.owl-ontologies.com/VirtualHome.owl#make_coffee">
        <rdfs:subClassOf rdf:resource="http://www.owl-ontologies.com/VirtualHome.owl#FoodPreparation"/>
        <rdfs:comment>Class with sequences on how to make coffee with different methods, and different steps.</rdfs:comment>
    </owl:Class>
    


    <!-- http://www.owl-ontologies.com/VirtualHome.owl#make_drink -->


    <owl:Class rdf:about="http://www.owl-ontologies.com/VirtualHome.owl#make_drink">
        <rdfs:subClassOf rdf:resource="http://www.owl-ontologies.com/VirtualHome.owl#FoodPreparation"/>
        <rdfs:comment>The class with sequence of actions for making a drink.</rdfs:comment>
    </owl:Class>
    


    <!-- http://www.owl-ontologies.com/VirtualHome.owl#make_eggs -->


    <owl:Class rdf:about="http://www.owl-ontologies.com/VirtualHome.owl#make_eggs">
        <rdfs:subClassOf rdf:resource="http://www.owl-ontologies.com/VirtualHome.owl#FoodPreparation"/>
        <rdfs:comment>The class with sequence of actions for making eggs.</rdfs:comment>
    </owl:Class>
    


    <!-- http://www.owl-ontologies.com/VirtualHome.owl#make_ice_in_ice_trays_for_freezer -->


    <owl:Class rdf:about="http://www.owl-ontologies.com/VirtualHome.owl#make_ice_in_ice_trays_for_freezer">
        <rdfs:subClassOf rdf:resource="http://www.owl-ontologies.com/VirtualHome.owl#FoodPreparation"/>
        <rdfs:comment>The class with sequence of actions for making ice in ice trays fo 
freezer.</rdfs:comment>
    </owl:Class>
    


    <!-- http://www.owl-ontologies.com/VirtualHome.owl#make_iced_coffee -->


    <owl:Class rdf:about="http://www.owl-ontologies.com/VirtualHome.owl#make_iced_coffee">
        <rdfs:subClassOf rdf:resource="http://www.owl-ontologies.com/VirtualHome.owl#FoodPreparation"/>
        <rdfs:comment>The class with sequence of actions for making iced coffee only.</rdfs:comment>
    </owl:Class>
    


    <!-- http://www.owl-ontologies.com/VirtualHome.owl#make_jello -->


    <owl:Class rdf:about="http://www.owl-ontologies.com/VirtualHome.owl#make_jello">
        <rdfs:subClassOf rdf:resource="http://www.owl-ontologies.com/VirtualHome.owl#FoodPreparation"/>
        <rdfs:comment>The class with sequence of actions for making jello.</rdfs:comment>
    </owl:Class>
    


    <!-- http://www.owl-ontologies.com/VirtualHome.owl#make_kids_bed -->


    <owl:Class rdf:about="http://www.owl-ontologies.com/VirtualHome.owl#make_kids_bed">
        <rdfs:subClassOf rdf:resource="http://www.owl-ontologies.com/VirtualHome.owl#HouseArrangement"/>
        <rdfs:comment>The class with sequence of actions for making the kids bed, in any room.</rdfs:comment>
    </owl:Class>
    


    <!-- http://www.owl-ontologies.com/VirtualHome.owl#make_peanut_butter_sandwhich -->


    <owl:Class rdf:about="http://www.owl-ontologies.com/VirtualHome.owl#make_peanut_butter_sandwhich">
        <rdfs:subClassOf rdf:resource="http://www.owl-ontologies.com/VirtualHome.owl#FoodPreparation"/>
        <rdfs:comment>The class with sequence of actions for making peanut butter sandwhich.</rdfs:comment>
    </owl:Class>
    


    <!-- http://www.owl-ontologies.com/VirtualHome.owl#make_peanut_butter_sandwich -->


    <owl:Class rdf:about="http://www.owl-ontologies.com/VirtualHome.owl#make_peanut_butter_sandwich">
        <rdfs:subClassOf rdf:resource="http://www.owl-ontologies.com/VirtualHome.owl#FoodPreparation"/>
        <rdfs:comment>The class with sequence of actions for making peanut butter sandwhich.</rdfs:comment>
    </owl:Class>
    


    <!-- http://www.owl-ontologies.com/VirtualHome.owl#make_phone_call -->


    <owl:Class rdf:about="http://www.owl-ontologies.com/VirtualHome.owl#make_phone_call">
        <rdfs:subClassOf rdf:resource="http://www.owl-ontologies.com/VirtualHome.owl#SocialInteraction"/>
        <rdfs:comment>The class with sequence of actions for making a phone call, form cell phone or home phone.</rdfs:comment>
    </owl:Class>
    


    <!-- http://www.owl-ontologies.com/VirtualHome.owl#make_place_cards -->


    <owl:Class rdf:about="http://www.owl-ontologies.com/VirtualHome.owl#make_place_cards">
        <rdfs:subClassOf rdf:resource="http://www.owl-ontologies.com/VirtualHome.owl#Other"/>
        <rdfs:comment>The class with sequence of actions for making place cards.</rdfs:comment>
    </owl:Class>
    


    <!-- http://www.owl-ontologies.com/VirtualHome.owl#make_popcorn -->


    <owl:Class rdf:about="http://www.owl-ontologies.com/VirtualHome.owl#make_popcorn">
        <rdfs:subClassOf rdf:resource="http://www.owl-ontologies.com/VirtualHome.owl#FoodPreparation"/>
        <rdfs:comment>The class with sequence of actions for making popcorn, in what ever mean 
can cook popcorn.</rdfs:comment>
    </owl:Class>
    


    <!-- http://www.owl-ontologies.com/VirtualHome.owl#make_sandwich -->


    <owl:Class rdf:about="http://www.owl-ontologies.com/VirtualHome.owl#make_sandwich">
        <rdfs:subClassOf rdf:resource="http://www.owl-ontologies.com/VirtualHome.owl#FoodPreparation"/>
        <rdfs:comment>The class with sequence of actions for making sandwich.</rdfs:comment>
    </owl:Class>
    


    <!-- http://www.owl-ontologies.com/VirtualHome.owl#make_sandwitch -->


    <owl:Class rdf:about="http://www.owl-ontologies.com/VirtualHome.owl#make_sandwitch">
        <rdfs:subClassOf rdf:resource="http://www.owl-ontologies.com/VirtualHome.owl#FoodPreparation"/>
        <rdfs:comment>The class with sequence of actions for making a sandwitch.</rdfs:comment>
    </owl:Class>
    


    <!-- http://www.owl-ontologies.com/VirtualHome.owl#make_several_copies_on_printer -->


    <owl:Class rdf:about="http://www.owl-ontologies.com/VirtualHome.owl#make_several_copies_on_printer">
        <rdfs:subClassOf rdf:resource="http://www.owl-ontologies.com/VirtualHome.owl#Work"/>
        <rdfs:comment>The class with sequence of actions to make several copies on the 
printer, the file does not matter in this case.</rdfs:comment>
    </owl:Class>
    


    <!-- http://www.owl-ontologies.com/VirtualHome.owl#make_tea -->


    <owl:Class rdf:about="http://www.owl-ontologies.com/VirtualHome.owl#make_tea">
        <rdfs:subClassOf rdf:resource="http://www.owl-ontologies.com/VirtualHome.owl#FoodPreparation"/>
        <rdfs:comment>The class with sequence of actions for making tea.</rdfs:comment>
    </owl:Class>
    


    <!-- http://www.owl-ontologies.com/VirtualHome.owl#make_toast -->


    <owl:Class rdf:about="http://www.owl-ontologies.com/VirtualHome.owl#make_toast">
        <rdfs:subClassOf rdf:resource="http://www.owl-ontologies.com/VirtualHome.owl#FoodPreparation"/>
        <rdfs:comment>The class with sequence of actions for making your own toast, or for 
someone else.</rdfs:comment>
    </owl:Class>
    


    <!-- http://www.owl-ontologies.com/VirtualHome.owl#make_tomato_sauce -->


    <owl:Class rdf:about="http://www.owl-ontologies.com/VirtualHome.owl#make_tomato_sauce">
        <rdfs:subClassOf rdf:resource="http://www.owl-ontologies.com/VirtualHome.owl#FoodPreparation"/>
        <rdfs:comment>The class with sequence of actions for making tomatoes sauce, in any 
room.</rdfs:comment>
    </owl:Class>
    


    <!-- http://www.owl-ontologies.com/VirtualHome.owl#make_tutu -->


    <owl:Class rdf:about="http://www.owl-ontologies.com/VirtualHome.owl#make_tutu">
        <rdfs:subClassOf rdf:resource="http://www.owl-ontologies.com/VirtualHome.owl#Other"/>
        <rdfs:comment>The class with sequence of actions for making tutu, inside the house.</rdfs:comment>
    </owl:Class>
    


    <!-- http://www.owl-ontologies.com/VirtualHome.owl#make_up_bed_for_guest_on_couch -->


    <owl:Class rdf:about="http://www.owl-ontologies.com/VirtualHome.owl#make_up_bed_for_guest_on_couch">
        <rdfs:subClassOf rdf:resource="http://www.owl-ontologies.com/VirtualHome.owl#HouseArrangement"/>
        <rdfs:comment>The class with sequence of actions for making up bed for guest on couch, 
wherever the couch is in the house.</rdfs:comment>
    </owl:Class>
    


    <!-- http://www.owl-ontologies.com/VirtualHome.owl#manage_documents -->


    <owl:Class rdf:about="http://www.owl-ontologies.com/VirtualHome.owl#manage_documents">
        <rdfs:subClassOf rdf:resource="http://www.owl-ontologies.com/VirtualHome.owl#Work"/>
        <rdfs:comment>The class with sequence of actions on how to manage your documents.</rdfs:comment>
    </owl:Class>
    


    <!-- http://www.owl-ontologies.com/VirtualHome.owl#manage_emails -->


    <owl:Class rdf:about="http://www.owl-ontologies.com/VirtualHome.owl#manage_emails">
        <rdfs:subClassOf rdf:resource="http://www.owl-ontologies.com/VirtualHome.owl#Work"/>
        <rdfs:comment>The class with sequence of actions for managing your emails (sorting, or 
merging the different files with emails).</rdfs:comment>
    </owl:Class>
    


    <!-- http://www.owl-ontologies.com/VirtualHome.owl#massage -->


    <owl:Class rdf:about="http://www.owl-ontologies.com/VirtualHome.owl#massage">
        <rdfs:subClassOf rdf:resource="http://www.owl-ontologies.com/VirtualHome.owl#SocialInteraction"/>
        <rdfs:comment>The class with sequence of actions for doing massage in any room.</rdfs:comment>
    </owl:Class>
    


    <!-- http://www.owl-ontologies.com/VirtualHome.owl#meeting -->


    <owl:Class rdf:about="http://www.owl-ontologies.com/VirtualHome.owl#meeting">
        <rdfs:subClassOf rdf:resource="http://www.owl-ontologies.com/VirtualHome.owl#SocialInteraction"/>
        <rdfs:comment>The class with sequence of actions for meeting , no matter the purpose 
of meeting.</rdfs:comment>
    </owl:Class>
    


    <!-- http://www.owl-ontologies.com/VirtualHome.owl#mop -->


    <owl:Class rdf:about="http://www.owl-ontologies.com/VirtualHome.owl#mop">
        <rdfs:subClassOf rdf:resource="http://www.owl-ontologies.com/VirtualHome.owl#HouseCleaning"/>
        <rdfs:comment>The class with sequence of actions taking up the mop and cleaning.</rdfs:comment>
    </owl:Class>
    


    <!-- http://www.owl-ontologies.com/VirtualHome.owl#mop_floor -->


    <owl:Class rdf:about="http://www.owl-ontologies.com/VirtualHome.owl#mop_floor">
        <rdfs:subClassOf rdf:resource="http://www.owl-ontologies.com/VirtualHome.owl#HouseCleaning"/>
        <rdfs:comment>The class with sequence of actions for mopping the floor.</rdfs:comment>
    </owl:Class>
    


    <!-- http://www.owl-ontologies.com/VirtualHome.owl#movie -->


    <owl:Class rdf:about="http://www.owl-ontologies.com/VirtualHome.owl#movie">
        <rdfs:subClassOf rdf:resource="http://www.owl-ontologies.com/VirtualHome.owl#Leisure"/>
        <rdfs:comment>The class with sequence of actions for watching a movie, either at TV or 
your Laptop.</rdfs:comment>
    </owl:Class>
    


    <!-- http://www.owl-ontologies.com/VirtualHome.owl#oil_dining_room -->


    <owl:Class rdf:about="http://www.owl-ontologies.com/VirtualHome.owl#oil_dining_room">
        <rdfs:subClassOf rdf:resource="http://www.owl-ontologies.com/VirtualHome.owl#HouseCleaning"/>
        <rdfs:comment>The class with sequence of actions for oiling dining room.</rdfs:comment>
    </owl:Class>
    


    <!-- http://www.owl-ontologies.com/VirtualHome.owl#open_bathroom_window -->


    <owl:Class rdf:about="http://www.owl-ontologies.com/VirtualHome.owl#open_bathroom_window">
        <rdfs:subClassOf rdf:resource="http://www.owl-ontologies.com/VirtualHome.owl#Other"/>
        <rdfs:comment>The class with sequence of actions for opening bathroom window.</rdfs:comment>
    </owl:Class>
    


    <!-- http://www.owl-ontologies.com/VirtualHome.owl#open_curtains -->


    <owl:Class rdf:about="http://www.owl-ontologies.com/VirtualHome.owl#open_curtains">
        <rdfs:subClassOf rdf:resource="http://www.owl-ontologies.com/VirtualHome.owl#Other"/>
        <rdfs:comment>The class with sequence of actions for opening up the curtains, from any 
room inside the house.</rdfs:comment>
    </owl:Class>
    


    <!-- http://www.owl-ontologies.com/VirtualHome.owl#open_door -->


    <owl:Class rdf:about="http://www.owl-ontologies.com/VirtualHome.owl#open_door">
        <rdfs:subClassOf rdf:resource="http://www.owl-ontologies.com/VirtualHome.owl#Other"/>
        <rdfs:comment>The class with sequence of actions for opening the door, either from the 
main entrance or door of a room.</rdfs:comment>
    </owl:Class>
    


    <!-- http://www.owl-ontologies.com/VirtualHome.owl#open_door_and_great_guests -->


    <owl:Class rdf:about="http://www.owl-ontologies.com/VirtualHome.owl#open_door_and_great_guests">
        <rdfs:subClassOf rdf:resource="http://www.owl-ontologies.com/VirtualHome.owl#SocialInteraction"/>
        <rdfs:comment>The class with sequence of actions for opening the door and greeting guests.</rdfs:comment>
    </owl:Class>
    


    <!-- http://www.owl-ontologies.com/VirtualHome.owl#open_front_door -->


    <owl:Class rdf:about="http://www.owl-ontologies.com/VirtualHome.owl#open_front_door">
        <rdfs:subClassOf rdf:resource="http://www.owl-ontologies.com/VirtualHome.owl#Other"/>
        <rdfs:comment>The class with sequence of actions for opening front door (main entrance 
door).</rdfs:comment>
    </owl:Class>
    


    <!-- http://www.owl-ontologies.com/VirtualHome.owl#open_window -->


    <owl:Class rdf:about="http://www.owl-ontologies.com/VirtualHome.owl#open_window">
        <rdfs:subClassOf rdf:resource="http://www.owl-ontologies.com/VirtualHome.owl#Other"/>
        <rdfs:comment>The class with sequence of actions for opening a window in any room.</rdfs:comment>
    </owl:Class>
    


    <!-- http://www.owl-ontologies.com/VirtualHome.owl#order_office_suplies -->


    <owl:Class rdf:about="http://www.owl-ontologies.com/VirtualHome.owl#order_office_suplies">
        <rdfs:subClassOf rdf:resource="http://www.owl-ontologies.com/VirtualHome.owl#Work"/>
        <rdfs:comment>The class with sequence of actions for ordering office suplies, such as 
papers, writing material, and more.</rdfs:comment>
    </owl:Class>
    


    <!-- http://www.owl-ontologies.com/VirtualHome.owl#organise_paperwork -->


    <owl:Class rdf:about="http://www.owl-ontologies.com/VirtualHome.owl#organise_paperwork">
        <rdfs:subClassOf rdf:resource="http://www.owl-ontologies.com/VirtualHome.owl#Work"/>
        <rdfs:comment>The class with sequence of actions for organizing paperwork.</rdfs:comment>
    </owl:Class>
    


    <!-- http://www.owl-ontologies.com/VirtualHome.owl#organize -->


    <owl:Class rdf:about="http://www.owl-ontologies.com/VirtualHome.owl#organize">
        <rdfs:subClassOf rdf:resource="http://www.owl-ontologies.com/VirtualHome.owl#Other"/>
        <rdfs:comment>The class with sequence of actions for organizing your work, your 
clothes, etc.</rdfs:comment>
    </owl:Class>
    


    <!-- http://www.owl-ontologies.com/VirtualHome.owl#organize_cabinet -->


    <owl:Class rdf:about="http://www.owl-ontologies.com/VirtualHome.owl#organize_cabinet">
        <rdfs:subClassOf rdf:resource="http://www.owl-ontologies.com/VirtualHome.owl#HouseArrangement"/>
        <rdfs:comment>The class with sequence of actions for organizing the objects insde the 
cabinet.</rdfs:comment>
    </owl:Class>
    


    <!-- http://www.owl-ontologies.com/VirtualHome.owl#organize_closet -->


    <owl:Class rdf:about="http://www.owl-ontologies.com/VirtualHome.owl#organize_closet">
        <rdfs:subClassOf rdf:resource="http://www.owl-ontologies.com/VirtualHome.owl#HouseCleaning"/>
        <rdfs:comment>The class with sequence of actions for organizing the closet.</rdfs:comment>
    </owl:Class>
    


    <!-- http://www.owl-ontologies.com/VirtualHome.owl#organize_desk -->


    <owl:Class rdf:about="http://www.owl-ontologies.com/VirtualHome.owl#organize_desk">
        <rdfs:subClassOf rdf:resource="http://www.owl-ontologies.com/VirtualHome.owl#HouseArrangement"/>
        <rdfs:comment>The class with sequence of actions for organizing the desk place, 
sorting items, pick up items.</rdfs:comment>
    </owl:Class>
    


    <!-- http://www.owl-ontologies.com/VirtualHome.owl#organize_files -->


    <owl:Class rdf:about="http://www.owl-ontologies.com/VirtualHome.owl#organize_files">
        <rdfs:subClassOf rdf:resource="http://www.owl-ontologies.com/VirtualHome.owl#Other"/>
        <rdfs:comment>The class with sequence of actions for organizing files, in anu order desired.</rdfs:comment>
    </owl:Class>
    


    <!-- http://www.owl-ontologies.com/VirtualHome.owl#organize_panrty -->


    <owl:Class rdf:about="http://www.owl-ontologies.com/VirtualHome.owl#organize_panrty">
        <rdfs:subClassOf rdf:resource="http://www.owl-ontologies.com/VirtualHome.owl#HouseArrangement"/>
        <rdfs:comment>The class with sequence of actions for organizing party, by using your 
phone or computer.</rdfs:comment>
    </owl:Class>
    


    <!-- http://www.owl-ontologies.com/VirtualHome.owl#organize_paperwork -->


    <owl:Class rdf:about="http://www.owl-ontologies.com/VirtualHome.owl#organize_paperwork">
        <rdfs:subClassOf rdf:resource="http://www.owl-ontologies.com/VirtualHome.owl#Work"/>
        <rdfs:comment>The class with sequence of actions for organizing your paper work.</rdfs:comment>
    </owl:Class>
    


    <!-- http://www.owl-ontologies.com/VirtualHome.owl#pack_lunch -->


    <owl:Class rdf:about="http://www.owl-ontologies.com/VirtualHome.owl#pack_lunch">
        <rdfs:subClassOf rdf:resource="http://www.owl-ontologies.com/VirtualHome.owl#Other"/>
        <rdfs:comment>The class with sequence of actions for packing up lunch, and go anywhere.</rdfs:comment>
    </owl:Class>
    


    <!-- http://www.owl-ontologies.com/VirtualHome.owl#paint_ceiling -->


    <owl:Class rdf:about="http://www.owl-ontologies.com/VirtualHome.owl#paint_ceiling">
        <rdfs:subClassOf rdf:resource="http://www.owl-ontologies.com/VirtualHome.owl#HouseArrangement"/>
        <rdfs:comment>The class with sequence of actions for painting the ceiling only.</rdfs:comment>
    </owl:Class>
    


    <!-- http://www.owl-ontologies.com/VirtualHome.owl#paint_nails -->


    <owl:Class rdf:about="http://www.owl-ontologies.com/VirtualHome.owl#paint_nails">
        <rdfs:subClassOf rdf:resource="http://www.owl-ontologies.com/VirtualHome.owl#HygieneStyling"/>
        <rdfs:comment>The class with sequence of actions for painting your own nails.</rdfs:comment>
    </owl:Class>
    


    <!-- http://www.owl-ontologies.com/VirtualHome.owl#pay_bills -->


    <owl:Class rdf:about="http://www.owl-ontologies.com/VirtualHome.owl#pay_bills">
        <rdfs:subClassOf rdf:resource="http://www.owl-ontologies.com/VirtualHome.owl#Work"/>
        <rdfs:comment>Class that contains sequences about how to pay bills.</rdfs:comment>
    </owl:Class>
    


    <!-- http://www.owl-ontologies.com/VirtualHome.owl#pee -->


    <owl:Class rdf:about="http://www.owl-ontologies.com/VirtualHome.owl#pee">
        <rdfs:subClassOf rdf:resource="http://www.owl-ontologies.com/VirtualHome.owl#HygieneStyling"/>
        <rdfs:comment>The class with sequence of actions for peeing.</rdfs:comment>
    </owl:Class>
    


    <!-- http://www.owl-ontologies.com/VirtualHome.owl#peel_kiwi -->


    <owl:Class rdf:about="http://www.owl-ontologies.com/VirtualHome.owl#peel_kiwi">
        <rdfs:subClassOf rdf:resource="http://www.owl-ontologies.com/VirtualHome.owl#FoodPreparation"/>
        <rdfs:comment>The class with sequence of actions for pelling the kiwi fruit.</rdfs:comment>
    </owl:Class>
    


    <!-- http://www.owl-ontologies.com/VirtualHome.owl#peel_potatoes -->


    <owl:Class rdf:about="http://www.owl-ontologies.com/VirtualHome.owl#peel_potatoes">
        <rdfs:subClassOf rdf:resource="http://www.owl-ontologies.com/VirtualHome.owl#FoodPreparation"/>
        <rdfs:comment>The class with sequence of actions for peeling potatoes in any room.</rdfs:comment>
    </owl:Class>
    


    <!-- http://www.owl-ontologies.com/VirtualHome.owl#pet_cat -->


    <owl:Class rdf:about="http://www.owl-ontologies.com/VirtualHome.owl#pet_cat">
        <rdfs:subClassOf rdf:resource="http://www.owl-ontologies.com/VirtualHome.owl#SocialInteraction"/>
        <rdfs:comment>A class with sequeces on how to pet your cat..</rdfs:comment>
    </owl:Class>
    


    <!-- http://www.owl-ontologies.com/VirtualHome.owl#pet_dog -->


    <owl:Class rdf:about="http://www.owl-ontologies.com/VirtualHome.owl#pet_dog">
        <rdfs:subClassOf rdf:resource="http://www.owl-ontologies.com/VirtualHome.owl#Other"/>
        <rdfs:comment>The class with sequence of actions for petting your dog.</rdfs:comment>
    </owl:Class>
    


    <!-- http://www.owl-ontologies.com/VirtualHome.owl#physical_therapy -->


    <owl:Class rdf:about="http://www.owl-ontologies.com/VirtualHome.owl#physical_therapy">
        <rdfs:subClassOf rdf:resource="http://www.owl-ontologies.com/VirtualHome.owl#PhysicalActivity"/>
        <rdfs:comment>The class with sequence of actions for doing physical therapy.</rdfs:comment>
    </owl:Class>
    


    <!-- http://www.owl-ontologies.com/VirtualHome.owl#pick_toys -->


    <owl:Class rdf:about="http://www.owl-ontologies.com/VirtualHome.owl#pick_toys">
        <rdfs:subClassOf rdf:resource="http://www.owl-ontologies.com/VirtualHome.owl#HouseArrangement"/>
        <rdfs:comment>The class with sequence of actions for picking up toys that were thrown 
away.</rdfs:comment>
    </owl:Class>
    


    <!-- http://www.owl-ontologies.com/VirtualHome.owl#pick_up -->


    <owl:Class rdf:about="http://www.owl-ontologies.com/VirtualHome.owl#pick_up">
        <rdfs:subClassOf rdf:resource="http://www.owl-ontologies.com/VirtualHome.owl#Other"/>
        <rdfs:comment>The class with sequence of actions for picking up any object, in any 
room.</rdfs:comment>
    </owl:Class>
    


    <!-- http://www.owl-ontologies.com/VirtualHome.owl#pick_up_all_trash -->


    <owl:Class rdf:about="http://www.owl-ontologies.com/VirtualHome.owl#pick_up_all_trash">
        <rdfs:subClassOf rdf:resource="http://www.owl-ontologies.com/VirtualHome.owl#Other"/>
        <rdfs:comment>The class with sequence of actions for picking up all trash from the 
floor, or any other place.</rdfs:comment>
    </owl:Class>
    


    <!-- http://www.owl-ontologies.com/VirtualHome.owl#pick_up_cat_hair -->


    <owl:Class rdf:about="http://www.owl-ontologies.com/VirtualHome.owl#pick_up_cat_hair">
        <rdfs:subClassOf rdf:resource="http://www.owl-ontologies.com/VirtualHome.owl#HouseCleaning"/>
        <rdfs:comment>The class with sequence of actions picking up the cat hair from the various furniture and the floor.</rdfs:comment>
    </owl:Class>
    


    <!-- http://www.owl-ontologies.com/VirtualHome.owl#pick_up_dIshes -->


    <owl:Class rdf:about="http://www.owl-ontologies.com/VirtualHome.owl#pick_up_dIshes">
        <rdfs:subClassOf rdf:resource="http://www.owl-ontologies.com/VirtualHome.owl#HouseArrangement"/>
        <rdfs:comment>The class with sequence of actions for picking up the dishes, from any room.</rdfs:comment>
    </owl:Class>
    


    <!-- http://www.owl-ontologies.com/VirtualHome.owl#pick_up_dirty_dishes -->


    <owl:Class rdf:about="http://www.owl-ontologies.com/VirtualHome.owl#pick_up_dirty_dishes">
        <rdfs:subClassOf rdf:resource="http://www.owl-ontologies.com/VirtualHome.owl#HouseArrangement"/>
        <rdfs:comment>The class with sequence of actions for picking up dirty dishes, in any 
room.</rdfs:comment>
    </owl:Class>
    


    <!-- http://www.owl-ontologies.com/VirtualHome.owl#pick_up_dishes -->


    <owl:Class rdf:about="http://www.owl-ontologies.com/VirtualHome.owl#pick_up_dishes">
        <rdfs:subClassOf rdf:resource="http://www.owl-ontologies.com/VirtualHome.owl#Other"/>
        <rdfs:comment>The class with sequence of actions for picking up the dishes.</rdfs:comment>
    </owl:Class>
    


    <!-- http://www.owl-ontologies.com/VirtualHome.owl#pick_up_obvious_trash -->


    <owl:Class rdf:about="http://www.owl-ontologies.com/VirtualHome.owl#pick_up_obvious_trash">
        <rdfs:subClassOf rdf:resource="http://www.owl-ontologies.com/VirtualHome.owl#Other"/>
        <rdfs:comment>The class with sequence of actions for picking up objects that are 
obiously trash.</rdfs:comment>
    </owl:Class>
    


    <!-- http://www.owl-ontologies.com/VirtualHome.owl#pick_up_phone -->


    <owl:Class rdf:about="http://www.owl-ontologies.com/VirtualHome.owl#pick_up_phone">
        <rdfs:subClassOf rdf:resource="http://www.owl-ontologies.com/VirtualHome.owl#Other"/>
        <rdfs:comment>A class with sequences on how to answer the phone, from different rooms, 
and in different scenaria sucks as holding something in hands, etc.</rdfs:comment>
    </owl:Class>
    


    <!-- http://www.owl-ontologies.com/VirtualHome.owl#pick_up_spare_change_on_dresser -->


    <owl:Class rdf:about="http://www.owl-ontologies.com/VirtualHome.owl#pick_up_spare_change_on_dresser">
        <rdfs:subClassOf rdf:resource="http://www.owl-ontologies.com/VirtualHome.owl#Other"/>
        <rdfs:comment>The class with sequence of actions for picking up sparse change on dresser, in any room.</rdfs:comment>
    </owl:Class>
    


    <!-- http://www.owl-ontologies.com/VirtualHome.owl#pick_up_toys -->


    <owl:Class rdf:about="http://www.owl-ontologies.com/VirtualHome.owl#pick_up_toys">
        <rdfs:subClassOf rdf:resource="http://www.owl-ontologies.com/VirtualHome.owl#Other"/>
        <rdfs:comment>A class with sequences on to pick up the toys left behind by other 
individuals.</rdfs:comment>
    </owl:Class>
    


    <!-- http://www.owl-ontologies.com/VirtualHome.owl#place_bathmat -->


    <owl:Class rdf:about="http://www.owl-ontologies.com/VirtualHome.owl#place_bathmat">
        <rdfs:subClassOf rdf:resource="http://www.owl-ontologies.com/VirtualHome.owl#HouseArrangement"/>
        <rdfs:comment>The class with sequence of actions for placing bathmat in the bathroom.</rdfs:comment>
    </owl:Class>
    


    <!-- http://www.owl-ontologies.com/VirtualHome.owl#place_centerpiece -->


    <owl:Class rdf:about="http://www.owl-ontologies.com/VirtualHome.owl#place_centerpiece">
        <rdfs:subClassOf rdf:resource="http://www.owl-ontologies.com/VirtualHome.owl#HouseArrangement"/>
        <rdfs:comment>The class with sequence of actions for placing centerpiece.</rdfs:comment>
    </owl:Class>
    


    <!-- http://www.owl-ontologies.com/VirtualHome.owl#place_table -->


    <owl:Class rdf:about="http://www.owl-ontologies.com/VirtualHome.owl#place_table">
        <rdfs:subClassOf rdf:resource="http://www.owl-ontologies.com/VirtualHome.owl#HouseArrangement"/>
        <rdfs:comment>The class with sequence of actions for placing the table in any room.</rdfs:comment>
    </owl:Class>
    


    <!-- http://www.owl-ontologies.com/VirtualHome.owl#play_fetch_with_dog -->


    <owl:Class rdf:about="http://www.owl-ontologies.com/VirtualHome.owl#play_fetch_with_dog">
        <rdfs:subClassOf rdf:resource="http://www.owl-ontologies.com/VirtualHome.owl#SocialInteraction"/>
        <rdfs:comment>The class with sequence of actions for playing fetch with a dog.</rdfs:comment>
    </owl:Class>
    


    <!-- http://www.owl-ontologies.com/VirtualHome.owl#play_games -->


    <owl:Class rdf:about="http://www.owl-ontologies.com/VirtualHome.owl#play_games">
        <rdfs:subClassOf rdf:resource="http://www.owl-ontologies.com/VirtualHome.owl#Leisure"/>
        <rdfs:comment>The sequence of actions about how to paly games.</rdfs:comment>
    </owl:Class>
    


    <!-- http://www.owl-ontologies.com/VirtualHome.owl#play_guitar -->


    <owl:Class rdf:about="http://www.owl-ontologies.com/VirtualHome.owl#play_guitar">
        <rdfs:subClassOf rdf:resource="http://www.owl-ontologies.com/VirtualHome.owl#Leisure"/>
        <rdfs:comment>The class with sequence of actions for playing with the guitar (electric 
or normal).</rdfs:comment>
    </owl:Class>
    


    <!-- http://www.owl-ontologies.com/VirtualHome.owl#play_musical_chairs -->


    <owl:Class rdf:about="http://www.owl-ontologies.com/VirtualHome.owl#play_musical_chairs">
        <rdfs:subClassOf rdf:resource="http://www.owl-ontologies.com/VirtualHome.owl#Leisure"/>
        <rdfs:comment>The class with sequence of actions for playing musical chairs, (with no respect to the environment).</rdfs:comment>
    </owl:Class>
    


    <!-- http://www.owl-ontologies.com/VirtualHome.owl#play_on_laptop -->


    <owl:Class rdf:about="http://www.owl-ontologies.com/VirtualHome.owl#play_on_laptop">
        <rdfs:subClassOf rdf:resource="http://www.owl-ontologies.com/VirtualHome.owl#Leisure"/>
        <rdfs:comment>The class with sequence of actions for palying games or have fyn while at your computer.</rdfs:comment>
    </owl:Class>
    


    <!-- http://www.owl-ontologies.com/VirtualHome.owl#play_piano -->


    <owl:Class rdf:about="http://www.owl-ontologies.com/VirtualHome.owl#play_piano">
        <rdfs:subClassOf rdf:resource="http://www.owl-ontologies.com/VirtualHome.owl#Leisure"/>
        <rdfs:comment>The class with sequence of actions for playing your piano.</rdfs:comment>
    </owl:Class>
    


    <!-- http://www.owl-ontologies.com/VirtualHome.owl#play_with_barbies -->


    <owl:Class rdf:about="http://www.owl-ontologies.com/VirtualHome.owl#play_with_barbies">
        <rdfs:subClassOf rdf:resource="http://www.owl-ontologies.com/VirtualHome.owl#Leisure"/>
        <rdfs:comment>&lt;p style=&quot;margin-top: 0&quot;&gt;
      The class with sequence of actions for palying with barbie dolls.
    &lt;/p&gt;</rdfs:comment>
    </owl:Class>
    


    <!-- http://www.owl-ontologies.com/VirtualHome.owl#play_with_toys -->


    <owl:Class rdf:about="http://www.owl-ontologies.com/VirtualHome.owl#play_with_toys">
        <rdfs:subClassOf rdf:resource="http://www.owl-ontologies.com/VirtualHome.owl#Other"/>
        <rdfs:comment>The class with sequence of actions for playing with toys, in any room.</rdfs:comment>
    </owl:Class>
    


    <!-- http://www.owl-ontologies.com/VirtualHome.owl#playing_video_game -->


    <owl:Class rdf:about="http://www.owl-ontologies.com/VirtualHome.owl#playing_video_game">
        <rdfs:subClassOf rdf:resource="http://www.owl-ontologies.com/VirtualHome.owl#Leisure"/>
        <rdfs:comment>The class with sequence of actions either at a console or at the 
computer.</rdfs:comment>
    </owl:Class>
    


    <!-- http://www.owl-ontologies.com/VirtualHome.owl#playtime_lunch_with_dolls -->


    <owl:Class rdf:about="http://www.owl-ontologies.com/VirtualHome.owl#playtime_lunch_with_dolls">
        <rdfs:subClassOf rdf:resource="http://www.owl-ontologies.com/VirtualHome.owl#Leisure"/>
        <rdfs:comment>The class with sequence of actions for playing with dolls while eating 
your lunch.</rdfs:comment>
    </owl:Class>
    


    <!-- http://www.owl-ontologies.com/VirtualHome.owl#plug_in_nightlight -->


    <owl:Class rdf:about="http://www.owl-ontologies.com/VirtualHome.owl#plug_in_nightlight">
        <rdfs:subClassOf rdf:resource="http://www.owl-ontologies.com/VirtualHome.owl#Other"/>
        <rdfs:comment>The class with sequence of actions for pluging in the nightlight, in any room.</rdfs:comment>
    </owl:Class>
    


    <!-- http://www.owl-ontologies.com/VirtualHome.owl#polish_table -->


    <owl:Class rdf:about="http://www.owl-ontologies.com/VirtualHome.owl#polish_table">
        <rdfs:subClassOf rdf:resource="http://www.owl-ontologies.com/VirtualHome.owl#HouseCleaning"/>
        <rdfs:comment>The class with sequence of actions to polish a table.</rdfs:comment>
    </owl:Class>
    


    <!-- http://www.owl-ontologies.com/VirtualHome.owl#polish_teas_pot -->


    <owl:Class rdf:about="http://www.owl-ontologies.com/VirtualHome.owl#polish_teas_pot">
        <rdfs:subClassOf rdf:resource="http://www.owl-ontologies.com/VirtualHome.owl#HouseArrangement"/>
        <rdfs:comment>The class with sequence of actions for polishing tea pots
.</rdfs:comment>
    </owl:Class>
    


    <!-- http://www.owl-ontologies.com/VirtualHome.owl#polish_your_shoes -->


    <owl:Class rdf:about="http://www.owl-ontologies.com/VirtualHome.owl#polish_your_shoes">
        <rdfs:subClassOf rdf:resource="http://www.owl-ontologies.com/VirtualHome.owl#HouseArrangement"/>
        <rdfs:comment>The class with sequence of actions for polishing your own shoes.</rdfs:comment>
    </owl:Class>
    


    <!-- http://www.owl-ontologies.com/VirtualHome.owl#polishing_floor -->


    <owl:Class rdf:about="http://www.owl-ontologies.com/VirtualHome.owl#polishing_floor">
        <rdfs:subClassOf rdf:resource="http://www.owl-ontologies.com/VirtualHome.owl#HouseCleaning"/>
        <rdfs:comment>The class with sequence of actions for polishing the floor.</rdfs:comment>
    </owl:Class>
    


    <!-- http://www.owl-ontologies.com/VirtualHome.owl#pop_zit -->


    <owl:Class rdf:about="http://www.owl-ontologies.com/VirtualHome.owl#pop_zit">
        <rdfs:subClassOf rdf:resource="http://www.owl-ontologies.com/VirtualHome.owl#Other"/>
        <rdfs:comment>The class with sequence of actions for poping out zits.</rdfs:comment>
    </owl:Class>
    


    <!-- http://www.owl-ontologies.com/VirtualHome.owl#pour_cup_of_coffee -->


    <owl:Class rdf:about="http://www.owl-ontologies.com/VirtualHome.owl#pour_cup_of_coffee">
        <rdfs:subClassOf rdf:resource="http://www.owl-ontologies.com/VirtualHome.owl#Other"/>
        <rdfs:comment>The class with sequence of actions for pouring cup of coffee.</rdfs:comment>
    </owl:Class>
    


    <!-- http://www.owl-ontologies.com/VirtualHome.owl#practice_own_singing -->


    <owl:Class rdf:about="http://www.owl-ontologies.com/VirtualHome.owl#practice_own_singing">
        <rdfs:subClassOf rdf:resource="http://www.owl-ontologies.com/VirtualHome.owl#Leisure"/>
        <rdfs:comment>The class with sequence of actions for practicing your own singing.</rdfs:comment>
    </owl:Class>
    


    <!-- http://www.owl-ontologies.com/VirtualHome.owl#practice_violin -->


    <owl:Class rdf:about="http://www.owl-ontologies.com/VirtualHome.owl#practice_violin">
        <rdfs:subClassOf rdf:resource="http://www.owl-ontologies.com/VirtualHome.owl#Leisure"/>
        <rdfs:comment>The class with sequence of actions for practicing your violin.</rdfs:comment>
    </owl:Class>
    


    <!-- http://www.owl-ontologies.com/VirtualHome.owl#praying -->


    <owl:Class rdf:about="http://www.owl-ontologies.com/VirtualHome.owl#praying">
        <rdfs:subClassOf rdf:resource="http://www.owl-ontologies.com/VirtualHome.owl#Other"/>
        <rdfs:comment>The class with sequence of actions for praying in any room.</rdfs:comment>
    </owl:Class>
    


    <!-- http://www.owl-ontologies.com/VirtualHome.owl#prepare_breakfast -->


    <owl:Class rdf:about="http://www.owl-ontologies.com/VirtualHome.owl#prepare_breakfast">
        <rdfs:subClassOf rdf:resource="http://www.owl-ontologies.com/VirtualHome.owl#FoodPreparation"/>
        <rdfs:comment>The class with sequence of actions for preparing the breakfast (not 
eating the breakfast).</rdfs:comment>
    </owl:Class>
    


    <!-- http://www.owl-ontologies.com/VirtualHome.owl#prepare_dinner -->


    <owl:Class rdf:about="http://www.owl-ontologies.com/VirtualHome.owl#prepare_dinner">
        <rdfs:subClassOf rdf:resource="http://www.owl-ontologies.com/VirtualHome.owl#FoodPreparation"/>
        <rdfs:comment>Class with sequences for the procedure of getting the able ready to eat dinner.</rdfs:comment>
        <rdfs:comment>The class with sequence of actions for making the dinner (the procedure of cooking).</rdfs:comment>
    </owl:Class>
    


    <!-- http://www.owl-ontologies.com/VirtualHome.owl#prepare_for_work -->


    <owl:Class rdf:about="http://www.owl-ontologies.com/VirtualHome.owl#prepare_for_work">
        <rdfs:subClassOf rdf:resource="http://www.owl-ontologies.com/VirtualHome.owl#Work"/>
        <rdfs:comment>The class with sequence of actions for preparing for work.</rdfs:comment>
    </owl:Class>
    


    <!-- http://www.owl-ontologies.com/VirtualHome.owl#prepare_letter_for_mailing -->


    <owl:Class rdf:about="http://www.owl-ontologies.com/VirtualHome.owl#prepare_letter_for_mailing">
        <rdfs:subClassOf rdf:resource="http://www.owl-ontologies.com/VirtualHome.owl#Work"/>
        <rdfs:comment>The class with sequence of actions to prepare a letter that will be send 
for mailing later.</rdfs:comment>
    </owl:Class>
    


    <!-- http://www.owl-ontologies.com/VirtualHome.owl#prepare_pot_of_boiling_water -->


    <owl:Class rdf:about="http://www.owl-ontologies.com/VirtualHome.owl#prepare_pot_of_boiling_water">
        <rdfs:subClassOf rdf:resource="http://www.owl-ontologies.com/VirtualHome.owl#FoodPreparation"/>
        <rdfs:comment>The class with sequence of actions for prepareing pot of boiling water.</rdfs:comment>
    </owl:Class>
    


    <!-- http://www.owl-ontologies.com/VirtualHome.owl#prepare_sandwich -->


    <owl:Class rdf:about="http://www.owl-ontologies.com/VirtualHome.owl#prepare_sandwich">
        <rdfs:subClassOf rdf:resource="http://www.owl-ontologies.com/VirtualHome.owl#FoodPreparation"/>
        <rdfs:comment>The class with sequence of actions for food preparation.</rdfs:comment>
    </owl:Class>
    


    <!-- http://www.owl-ontologies.com/VirtualHome.owl#prepare_sandwitch -->


    <owl:Class rdf:about="http://www.owl-ontologies.com/VirtualHome.owl#prepare_sandwitch">
        <rdfs:subClassOf rdf:resource="http://www.owl-ontologies.com/VirtualHome.owl#FoodPreparation"/>
        <rdfs:comment>The class with sequence of actions for preparing a sandwich.</rdfs:comment>
    </owl:Class>
    


    <!-- http://www.owl-ontologies.com/VirtualHome.owl#prepare_sitting -->


    <owl:Class rdf:about="http://www.owl-ontologies.com/VirtualHome.owl#prepare_sitting">
        <rdfs:subClassOf rdf:resource="http://www.owl-ontologies.com/VirtualHome.owl#HouseArrangement"/>
    </owl:Class>
    


    <!-- http://www.owl-ontologies.com/VirtualHome.owl#pretend_tea -->


    <owl:Class rdf:about="http://www.owl-ontologies.com/VirtualHome.owl#pretend_tea">
        <rdfs:subClassOf rdf:resource="http://www.owl-ontologies.com/VirtualHome.owl#Other"/>
        <rdfs:comment>The class with sequence of actions for pretending that you are drinking tea.</rdfs:comment>
    </owl:Class>
    


    <!-- http://www.owl-ontologies.com/VirtualHome.owl#print_documents -->


    <owl:Class rdf:about="http://www.owl-ontologies.com/VirtualHome.owl#print_documents">
        <rdfs:subClassOf rdf:resource="http://www.owl-ontologies.com/VirtualHome.owl#Work"/>
        <rdfs:comment>The class with sequence of actions for printing more than one documents.</rdfs:comment>
    </owl:Class>
    


    <!-- http://www.owl-ontologies.com/VirtualHome.owl#print_out_document -->


    <owl:Class rdf:about="http://www.owl-ontologies.com/VirtualHome.owl#print_out_document">
        <rdfs:subClassOf rdf:resource="http://www.owl-ontologies.com/VirtualHome.owl#Work"/>
        <rdfs:comment>The class with sequence of actions to print out a document, no matter 
what document.</rdfs:comment>
    </owl:Class>
    


    <!-- http://www.owl-ontologies.com/VirtualHome.owl#print_out_papers -->


    <owl:Class rdf:about="http://www.owl-ontologies.com/VirtualHome.owl#print_out_papers">
        <rdfs:subClassOf rdf:resource="http://www.owl-ontologies.com/VirtualHome.owl#Work"/>
        <rdfs:comment>The class with sequence of actions for printing out papers, no matter 
what type of paper.</rdfs:comment>
    </owl:Class>
    


    <!-- http://www.owl-ontologies.com/VirtualHome.owl#pull_hair_out_of_drain -->


    <owl:Class rdf:about="http://www.owl-ontologies.com/VirtualHome.owl#pull_hair_out_of_drain">
        <rdfs:subClassOf rdf:resource="http://www.owl-ontologies.com/VirtualHome.owl#HouseCleaning"/>
        <rdfs:comment>The class with sequence of actions for pulling the hair out of drain.</rdfs:comment>
    </owl:Class>
    


    <!-- http://www.owl-ontologies.com/VirtualHome.owl#pull_up_carpet -->


    <owl:Class rdf:about="http://www.owl-ontologies.com/VirtualHome.owl#pull_up_carpet">
        <rdfs:subClassOf rdf:resource="http://www.owl-ontologies.com/VirtualHome.owl#Other"/>
        <rdfs:comment>The class with sequence of actions for pulling up th carpet, form any room.</rdfs:comment>
    </owl:Class>
    


    <!-- http://www.owl-ontologies.com/VirtualHome.owl#push_all_chairs_in -->


    <owl:Class rdf:about="http://www.owl-ontologies.com/VirtualHome.owl#push_all_chairs_in">
        <rdfs:subClassOf rdf:resource="http://www.owl-ontologies.com/VirtualHome.owl#HouseArrangement"/>
        <rdfs:comment>The class with sequence of actions for pushing all chairs in (under the table, or other place).</rdfs:comment>
    </owl:Class>
    


    <!-- http://www.owl-ontologies.com/VirtualHome.owl#push_in_desk_chair -->


    <owl:Class rdf:about="http://www.owl-ontologies.com/VirtualHome.owl#push_in_desk_chair">
        <rdfs:subClassOf rdf:resource="http://www.owl-ontologies.com/VirtualHome.owl#Other"/>
        <rdfs:comment>The class with sequence of actions for pushing in the desk chair.</rdfs:comment>
    </owl:Class>
    


    <!-- http://www.owl-ontologies.com/VirtualHome.owl#push_in_dining_room_chair -->


    <owl:Class rdf:about="http://www.owl-ontologies.com/VirtualHome.owl#push_in_dining_room_chair">
        <rdfs:subClassOf rdf:resource="http://www.owl-ontologies.com/VirtualHome.owl#Other"/>
        <rdfs:comment>The class with sequence of actions for pushing in the dining room chair, 
under the table or in other place.</rdfs:comment>
    </owl:Class>
    


    <!-- http://www.owl-ontologies.com/VirtualHome.owl#put_alarm_clock_in_bedroom -->


    <owl:Class rdf:about="http://www.owl-ontologies.com/VirtualHome.owl#put_alarm_clock_in_bedroom">
        <rdfs:subClassOf rdf:resource="http://www.owl-ontologies.com/VirtualHome.owl#BedTimeSleep"/>
        <rdfs:comment>The class with sequence of actions for setting the alarm clock at 
specific time, which exists in the bedroom.</rdfs:comment>
    </owl:Class>
    


    <!-- http://www.owl-ontologies.com/VirtualHome.owl#put_away_blankets -->


    <owl:Class rdf:about="http://www.owl-ontologies.com/VirtualHome.owl#put_away_blankets">
        <rdfs:subClassOf rdf:resource="http://www.owl-ontologies.com/VirtualHome.owl#Other"/>
        <rdfs:comment>The class with sequence of actions for putting away blankets.</rdfs:comment>
    </owl:Class>
    


    <!-- http://www.owl-ontologies.com/VirtualHome.owl#put_away_clean_clothes -->


    <owl:Class rdf:about="http://www.owl-ontologies.com/VirtualHome.owl#put_away_clean_clothes">
        <rdfs:subClassOf rdf:resource="http://www.owl-ontologies.com/VirtualHome.owl#HouseArrangement"/>
        <rdfs:comment>The class with sequence of actions for for putting away clean clothes.</rdfs:comment>
    </owl:Class>
    


    <!-- http://www.owl-ontologies.com/VirtualHome.owl#put_away_clothes -->


    <owl:Class rdf:about="http://www.owl-ontologies.com/VirtualHome.owl#put_away_clothes">
        <rdfs:subClassOf rdf:resource="http://www.owl-ontologies.com/VirtualHome.owl#Other"/>
        <rdfs:comment>The class with sequence of actions for putting away clothes.</rdfs:comment>
    </owl:Class>
    


    <!-- http://www.owl-ontologies.com/VirtualHome.owl#put_away_dishes -->


    <owl:Class rdf:about="http://www.owl-ontologies.com/VirtualHome.owl#put_away_dishes">
        <rdfs:subClassOf rdf:resource="http://www.owl-ontologies.com/VirtualHome.owl#HouseArrangement"/>
        <rdfs:comment>The class with sequence of actions for putting away the dishes.</rdfs:comment>
    </owl:Class>
    


    <!-- http://www.owl-ontologies.com/VirtualHome.owl#put_away_groceries -->


    <owl:Class rdf:about="http://www.owl-ontologies.com/VirtualHome.owl#put_away_groceries">
        <rdfs:subClassOf rdf:resource="http://www.owl-ontologies.com/VirtualHome.owl#HouseArrangement"/>
        <rdfs:comment>The class with sequence of actions for putting away the groceries, not 
in specific room.</rdfs:comment>
    </owl:Class>
    


    <!-- http://www.owl-ontologies.com/VirtualHome.owl#put_away_jackets -->


    <owl:Class rdf:about="http://www.owl-ontologies.com/VirtualHome.owl#put_away_jackets">
        <rdfs:subClassOf rdf:resource="http://www.owl-ontologies.com/VirtualHome.owl#Other"/>
        <rdfs:comment>The class with sequence of actions for putting away the jackets.</rdfs:comment>
    </owl:Class>
    


    <!-- http://www.owl-ontologies.com/VirtualHome.owl#put_away_keys -->


    <owl:Class rdf:about="http://www.owl-ontologies.com/VirtualHome.owl#put_away_keys">
        <rdfs:subClassOf rdf:resource="http://www.owl-ontologies.com/VirtualHome.owl#Other"/>
        <rdfs:comment>The class with sequence of actions for putting away keys, in their 
storing place.</rdfs:comment>
    </owl:Class>
    


    <!-- http://www.owl-ontologies.com/VirtualHome.owl#put_away_shoes -->


    <owl:Class rdf:about="http://www.owl-ontologies.com/VirtualHome.owl#put_away_shoes">
        <rdfs:subClassOf rdf:resource="http://www.owl-ontologies.com/VirtualHome.owl#Other"/>
        <rdfs:comment>The class with sequence of actions for putting away the shoes.</rdfs:comment>
    </owl:Class>
    


    <!-- http://www.owl-ontologies.com/VirtualHome.owl#put_away_toys -->


    <owl:Class rdf:about="http://www.owl-ontologies.com/VirtualHome.owl#put_away_toys">
        <rdfs:subClassOf rdf:resource="http://www.owl-ontologies.com/VirtualHome.owl#Other"/>
        <rdfs:comment>The class with sequence of actions for putting away the toys.</rdfs:comment>
    </owl:Class>
    


    <!-- http://www.owl-ontologies.com/VirtualHome.owl#put_clothes_away -->


    <owl:Class rdf:about="http://www.owl-ontologies.com/VirtualHome.owl#put_clothes_away">
        <rdfs:subClassOf rdf:resource="http://www.owl-ontologies.com/VirtualHome.owl#Other"/>
        <rdfs:comment>The class with sequence of actions for putting clothes away.</rdfs:comment>
    </owl:Class>
    


    <!-- http://www.owl-ontologies.com/VirtualHome.owl#put_dishes_away -->


    <owl:Class rdf:about="http://www.owl-ontologies.com/VirtualHome.owl#put_dishes_away">
        <rdfs:subClassOf rdf:resource="http://www.owl-ontologies.com/VirtualHome.owl#HouseArrangement"/>
        <rdfs:comment>The class with sequence of actions for putting dishes away from any 
place.</rdfs:comment>
    </owl:Class>
    


    <!-- http://www.owl-ontologies.com/VirtualHome.owl#put_down_bags -->


    <owl:Class rdf:about="http://www.owl-ontologies.com/VirtualHome.owl#put_down_bags">
        <rdfs:subClassOf rdf:resource="http://www.owl-ontologies.com/VirtualHome.owl#Other"/>
        <rdfs:comment>The class with sequence of actions for putting down bags, in any room.</rdfs:comment>
    </owl:Class>
    


    <!-- http://www.owl-ontologies.com/VirtualHome.owl#put_down_decoration -->


    <owl:Class rdf:about="http://www.owl-ontologies.com/VirtualHome.owl#put_down_decoration">
        <rdfs:subClassOf rdf:resource="http://www.owl-ontologies.com/VirtualHome.owl#HouseArrangement"/>
        <rdfs:comment>The class with sequence of actions for putting down decoration, on the 
floor or table.</rdfs:comment>
    </owl:Class>
    


    <!-- http://www.owl-ontologies.com/VirtualHome.owl#put_dvds_on_shelves -->


    <owl:Class rdf:about="http://www.owl-ontologies.com/VirtualHome.owl#put_dvds_on_shelves">
        <rdfs:subClassOf rdf:resource="http://www.owl-ontologies.com/VirtualHome.owl#HouseArrangement"/>
        <rdfs:comment>The class with sequence of actions for putting the dvds on shelves
.</rdfs:comment>
    </owl:Class>
    


    <!-- http://www.owl-ontologies.com/VirtualHome.owl#put_groceries_in_fridge -->


    <owl:Class rdf:about="http://www.owl-ontologies.com/VirtualHome.owl#put_groceries_in_fridge">
        <rdfs:subClassOf rdf:resource="http://www.owl-ontologies.com/VirtualHome.owl#HouseArrangement"/>
        <rdfs:comment>Class with sequences that show how to put groceries and other object in 
the fridge.</rdfs:comment>
    </owl:Class>
    


    <!-- http://www.owl-ontologies.com/VirtualHome.owl#put_in_chair -->


    <owl:Class rdf:about="http://www.owl-ontologies.com/VirtualHome.owl#put_in_chair">
        <rdfs:subClassOf rdf:resource="http://www.owl-ontologies.com/VirtualHome.owl#Other"/>
        <rdfs:comment>The class with sequence of actions for putting in the chair or chairs in 
any room.</rdfs:comment>
    </owl:Class>
    


    <!-- http://www.owl-ontologies.com/VirtualHome.owl#put_mail_away -->


    <owl:Class rdf:about="http://www.owl-ontologies.com/VirtualHome.owl#put_mail_away">
        <rdfs:subClassOf rdf:resource="http://www.owl-ontologies.com/VirtualHome.owl#HouseArrangement"/>
        <rdfs:comment>The class with sequence of actions for putiing mails away, in a specific 
place.</rdfs:comment>
    </owl:Class>
    


    <!-- http://www.owl-ontologies.com/VirtualHome.owl#put_mail_in_mail_organizer -->


    <owl:Class rdf:about="http://www.owl-ontologies.com/VirtualHome.owl#put_mail_in_mail_organizer">
        <rdfs:subClassOf rdf:resource="http://www.owl-ontologies.com/VirtualHome.owl#HouseArrangement"/>
        <rdfs:comment>The class with sequence of actions for puttin mail in mail organizer.</rdfs:comment>
    </owl:Class>
    


    <!-- http://www.owl-ontologies.com/VirtualHome.owl#put_new_books_in_shelves -->


    <owl:Class rdf:about="http://www.owl-ontologies.com/VirtualHome.owl#put_new_books_in_shelves">
        <rdfs:subClassOf rdf:resource="http://www.owl-ontologies.com/VirtualHome.owl#HouseArrangement"/>
        <rdfs:comment>The class with sequence of actions for putting new books in shelves, 
from another place.</rdfs:comment>
    </owl:Class>
    


    <!-- http://www.owl-ontologies.com/VirtualHome.owl#put_on_coat -->


    <owl:Class rdf:about="http://www.owl-ontologies.com/VirtualHome.owl#put_on_coat">
        <rdfs:subClassOf rdf:resource="http://www.owl-ontologies.com/VirtualHome.owl#HygieneStyling"/>
        <rdfs:comment>The class with sequence of actions for putting on your coat.</rdfs:comment>
    </owl:Class>
    


    <!-- http://www.owl-ontologies.com/VirtualHome.owl#put_on_coat_and_shoes -->


    <owl:Class rdf:about="http://www.owl-ontologies.com/VirtualHome.owl#put_on_coat_and_shoes">
        <rdfs:subClassOf rdf:resource="http://www.owl-ontologies.com/VirtualHome.owl#HygieneStyling"/>
        <rdfs:comment>The class with sequence of actions for putiing on coat and shoes.</rdfs:comment>
    </owl:Class>
    


    <!-- http://www.owl-ontologies.com/VirtualHome.owl#put_on_foundation -->


    <owl:Class rdf:about="http://www.owl-ontologies.com/VirtualHome.owl#put_on_foundation">
        <rdfs:subClassOf rdf:resource="http://www.owl-ontologies.com/VirtualHome.owl#HygieneStyling"/>
        <rdfs:comment>The class with sequence of actions for putting on a foundation.</rdfs:comment>
    </owl:Class>
    


    <!-- http://www.owl-ontologies.com/VirtualHome.owl#put_on_glasses -->


    <owl:Class rdf:about="http://www.owl-ontologies.com/VirtualHome.owl#put_on_glasses">
        <rdfs:subClassOf rdf:resource="http://www.owl-ontologies.com/VirtualHome.owl#HygieneStyling"/>
        <rdfs:comment>The class with sequence of actions for putting your glasses on.</rdfs:comment>
    </owl:Class>
    


    <!-- http://www.owl-ontologies.com/VirtualHome.owl#put_on_purse_put_keys_and_lucky_charms_in_pockets_leave_home -->


    <owl:Class rdf:about="http://www.owl-ontologies.com/VirtualHome.owl#put_on_purse_put_keys_and_lucky_charms_in_pockets_leave_home">
        <rdfs:subClassOf rdf:resource="http://www.owl-ontologies.com/VirtualHome.owl#Other"/>
        <rdfs:comment>The class with sequence of actions for putting on purse, putting keys 
and lucjy charm in pockets, and leave home.</rdfs:comment>
    </owl:Class>
    


    <!-- http://www.owl-ontologies.com/VirtualHome.owl#put_on_your_shoes -->


    <owl:Class rdf:about="http://www.owl-ontologies.com/VirtualHome.owl#put_on_your_shoes">
        <rdfs:subClassOf rdf:resource="http://www.owl-ontologies.com/VirtualHome.owl#HygieneStyling"/>
        <rdfs:comment>The class with sequence of actions for putiing on your shoes, in any 
room.</rdfs:comment>
    </owl:Class>
    


    <!-- http://www.owl-ontologies.com/VirtualHome.owl#put_out_flowers -->


    <owl:Class rdf:about="http://www.owl-ontologies.com/VirtualHome.owl#put_out_flowers">
        <rdfs:subClassOf rdf:resource="http://www.owl-ontologies.com/VirtualHome.owl#Other"/>
        <rdfs:comment>The class with sequence of actions for putting out flowers on the balcony, or some external place of the house.</rdfs:comment>
    </owl:Class>
    


    <!-- http://www.owl-ontologies.com/VirtualHome.owl#put_shoes_and_coats -->


    <owl:Class rdf:about="http://www.owl-ontologies.com/VirtualHome.owl#put_shoes_and_coats">
        <rdfs:subClassOf rdf:resource="http://www.owl-ontologies.com/VirtualHome.owl#HygieneStyling"/>
        <rdfs:comment>The class with sequence of actions for putting shoes and coats.</rdfs:comment>
    </owl:Class>
    


    <!-- http://www.owl-ontologies.com/VirtualHome.owl#put_shoes_in_shoe_rack -->


    <owl:Class rdf:about="http://www.owl-ontologies.com/VirtualHome.owl#put_shoes_in_shoe_rack">
        <rdfs:subClassOf rdf:resource="http://www.owl-ontologies.com/VirtualHome.owl#HouseArrangement"/>
        <rdfs:comment>The class with sequence of actions for putting the shoes in shoe rack, wherever the shoe rack is.</rdfs:comment>
    </owl:Class>
    


    <!-- http://www.owl-ontologies.com/VirtualHome.owl#put_slippers_in_closet -->


    <owl:Class rdf:about="http://www.owl-ontologies.com/VirtualHome.owl#put_slippers_in_closet">
        <rdfs:subClassOf rdf:resource="http://www.owl-ontologies.com/VirtualHome.owl#HouseArrangement"/>
        <rdfs:comment>The class with sequence of actions for putting slippers in closet, in 
any room the closet is.</rdfs:comment>
    </owl:Class>
    


    <!-- http://www.owl-ontologies.com/VirtualHome.owl#put_them_to_sleep -->


    <owl:Class rdf:about="http://www.owl-ontologies.com/VirtualHome.owl#put_them_to_sleep">
        <rdfs:subClassOf rdf:resource="http://www.owl-ontologies.com/VirtualHome.owl#BedTimeSleep"/>
        <rdfs:comment>The class with sequence of actions for putting them to sleep.</rdfs:comment>
    </owl:Class>
    


    <!-- http://www.owl-ontologies.com/VirtualHome.owl#put_toys_away -->


    <owl:Class rdf:about="http://www.owl-ontologies.com/VirtualHome.owl#put_toys_away">
        <rdfs:subClassOf rdf:resource="http://www.owl-ontologies.com/VirtualHome.owl#HouseArrangement"/>
        <rdfs:comment>The class with sequence of actions for putting the toys away, that 
belong to childeren or your own.</rdfs:comment>
    </owl:Class>
    


    <!-- http://www.owl-ontologies.com/VirtualHome.owl#put_umbrella_away -->


    <owl:Class rdf:about="http://www.owl-ontologies.com/VirtualHome.owl#put_umbrella_away">
        <rdfs:subClassOf rdf:resource="http://www.owl-ontologies.com/VirtualHome.owl#Other"/>
        <rdfs:comment>The class with sequence of actions for putting the umbrella away, in any 
place.</rdfs:comment>
    </owl:Class>
    


    <!-- http://www.owl-ontologies.com/VirtualHome.owl#put_up_coat -->


    <owl:Class rdf:about="http://www.owl-ontologies.com/VirtualHome.owl#put_up_coat">
        <rdfs:subClassOf rdf:resource="http://www.owl-ontologies.com/VirtualHome.owl#HygieneStyling"/>
        <rdfs:comment>&lt;p style=&quot;margin-top: 0&quot;&gt;
      The class with sequence of actions for putting up coat.
    &lt;/p&gt;</rdfs:comment>
    </owl:Class>
    


    <!-- http://www.owl-ontologies.com/VirtualHome.owl#put_up_decoration -->


    <owl:Class rdf:about="http://www.owl-ontologies.com/VirtualHome.owl#put_up_decoration">
        <rdfs:subClassOf rdf:resource="http://www.owl-ontologies.com/VirtualHome.owl#Other"/>
        <rdfs:comment>The class with sequence of actions for putting up decoration.</rdfs:comment>
    </owl:Class>
    


    <!-- http://www.owl-ontologies.com/VirtualHome.owl#put_up_feet -->


    <owl:Class rdf:about="http://www.owl-ontologies.com/VirtualHome.owl#put_up_feet">
        <rdfs:subClassOf rdf:resource="http://www.owl-ontologies.com/VirtualHome.owl#Other"/>
        <rdfs:comment>The class with sequence of actions for putting up your feet, in any place and room.</rdfs:comment>
    </owl:Class>
    


    <!-- http://www.owl-ontologies.com/VirtualHome.owl#put_up_jacket -->


    <owl:Class rdf:about="http://www.owl-ontologies.com/VirtualHome.owl#put_up_jacket">
        <rdfs:subClassOf rdf:resource="http://www.owl-ontologies.com/VirtualHome.owl#Other"/>
        <rdfs:comment>The class with sequence of actions for putting up a jacket, in any room.</rdfs:comment>
    </owl:Class>
    


    <!-- http://www.owl-ontologies.com/VirtualHome.owl#put_up_towel -->


    <owl:Class rdf:about="http://www.owl-ontologies.com/VirtualHome.owl#put_up_towel">
        <rdfs:subClassOf rdf:resource="http://www.owl-ontologies.com/VirtualHome.owl#Other"/>
        <rdfs:comment>The class with sequence of actions for putting up towel, in any room on 
you.</rdfs:comment>
    </owl:Class>
    


    <!-- http://www.owl-ontologies.com/VirtualHome.owl#put_washed_clothes_in_almirah -->


    <owl:Class rdf:about="http://www.owl-ontologies.com/VirtualHome.owl#put_washed_clothes_in_almirah">
        <rdfs:subClassOf rdf:resource="http://www.owl-ontologies.com/VirtualHome.owl#HouseArrangement"/>
        <rdfs:comment>The class with sequence of actions for putting washed clothes in almirah.</rdfs:comment>
    </owl:Class>
    


    <!-- http://www.owl-ontologies.com/VirtualHome.owl#rain_welcome -->


    <owl:Class rdf:about="http://www.owl-ontologies.com/VirtualHome.owl#rain_welcome">
        <rdfs:subClassOf rdf:resource="http://www.owl-ontologies.com/VirtualHome.owl#Other"/>
        <rdfs:comment>he class with sequence of actions for raining welcome (comming inside 
the house, after rain).</rdfs:comment>
    </owl:Class>
    


    <!-- http://www.owl-ontologies.com/VirtualHome.owl#raise_blinds -->


    <owl:Class rdf:about="http://www.owl-ontologies.com/VirtualHome.owl#raise_blinds">
        <rdfs:subClassOf rdf:resource="http://www.owl-ontologies.com/VirtualHome.owl#Other"/>
        <rdfs:comment>The class with sequence of actions for raising blinds, from any window in any room.
    &lt;/p&gt;</rdfs:comment>
    </owl:Class>
    


    <!-- http://www.owl-ontologies.com/VirtualHome.owl#re_arrange_office -->


    <owl:Class rdf:about="http://www.owl-ontologies.com/VirtualHome.owl#re_arrange_office">
        <rdfs:subClassOf rdf:resource="http://www.owl-ontologies.com/VirtualHome.owl#HouseArrangement"/>
        <rdfs:comment>The class with sequence of actions for re arranging office, cleaning or 
sorting items, etc.</rdfs:comment>
    </owl:Class>
    


    <!-- http://www.owl-ontologies.com/VirtualHome.owl#read_book -->


    <owl:Class rdf:about="http://www.owl-ontologies.com/VirtualHome.owl#read_book">
        <rdfs:subClassOf rdf:resource="http://www.owl-ontologies.com/VirtualHome.owl#Leisure"/>
        <rdfs:comment>Class which contains sequence of action, about how to read of a book.</rdfs:comment>
    </owl:Class>
    


    <!-- http://www.owl-ontologies.com/VirtualHome.owl#read_magazine -->


    <owl:Class rdf:about="http://www.owl-ontologies.com/VirtualHome.owl#read_magazine">
        <rdfs:subClassOf rdf:resource="http://www.owl-ontologies.com/VirtualHome.owl#Leisure"/>
        <rdfs:comment>The class with sequence of actions for reading a magazine (not a 
newspaper).</rdfs:comment>
    </owl:Class>
    


    <!-- http://www.owl-ontologies.com/VirtualHome.owl#read_news -->


    <owl:Class rdf:about="http://www.owl-ontologies.com/VirtualHome.owl#read_news">
        <rdfs:subClassOf rdf:resource="http://www.owl-ontologies.com/VirtualHome.owl#Leisure"/>
        <rdfs:comment>The class with sequence of actions for reading news (either from a 
newspaper, either from the internet).</rdfs:comment>
    </owl:Class>
    


    <!-- http://www.owl-ontologies.com/VirtualHome.owl#read_newspaper -->


    <owl:Class rdf:about="http://www.owl-ontologies.com/VirtualHome.owl#read_newspaper">
        <rdfs:subClassOf rdf:resource="http://www.owl-ontologies.com/VirtualHome.owl#Leisure"/>
        <rdfs:comment>The class with sequence of actions for reading a newspaper.</rdfs:comment>
    </owl:Class>
    


    <!-- http://www.owl-ontologies.com/VirtualHome.owl#read_on_sofa -->


    <owl:Class rdf:about="http://www.owl-ontologies.com/VirtualHome.owl#read_on_sofa">
        <rdfs:subClassOf rdf:resource="http://www.owl-ontologies.com/VirtualHome.owl#Leisure"/>
        <rdfs:comment>The class with sequence of actions reading womehting (newspaper, or 
book or magazine), while on the sofa.</rdfs:comment>
    </owl:Class>
    


    <!-- http://www.owl-ontologies.com/VirtualHome.owl#read_paper -->


    <owl:Class rdf:about="http://www.owl-ontologies.com/VirtualHome.owl#read_paper">
        <rdfs:subClassOf rdf:resource="http://www.owl-ontologies.com/VirtualHome.owl#Work"/>
        <rdfs:comment>The class with sequence of actions for reading some kind of paper.</rdfs:comment>
    </owl:Class>
    


    <!-- http://www.owl-ontologies.com/VirtualHome.owl#read_text_message -->


    <owl:Class rdf:about="http://www.owl-ontologies.com/VirtualHome.owl#read_text_message">
        <rdfs:subClassOf rdf:resource="http://www.owl-ontologies.com/VirtualHome.owl#Other"/>
        <rdfs:comment>The class with sequence of actions for reading text message, form the 
phone, or computer.</rdfs:comment>
    </owl:Class>
    


    <!-- http://www.owl-ontologies.com/VirtualHome.owl#read_them_bedtime_story -->


    <owl:Class rdf:about="http://www.owl-ontologies.com/VirtualHome.owl#read_them_bedtime_story">
        <rdfs:subClassOf rdf:resource="http://www.owl-ontologies.com/VirtualHome.owl#BedTimeSleep"/>
        <rdfs:comment>The class with sequence of actions for reading to someone lese a bedtime 
story.</rdfs:comment>
    </owl:Class>
    


    <!-- http://www.owl-ontologies.com/VirtualHome.owl#read_to_child -->


    <owl:Class rdf:about="http://www.owl-ontologies.com/VirtualHome.owl#read_to_child">
        <rdfs:subClassOf rdf:resource="http://www.owl-ontologies.com/VirtualHome.owl#SocialInteraction"/>
        <rdfs:comment>The class with sequence of actions for readin to your child in any room.</rdfs:comment>
    </owl:Class>
    


    <!-- http://www.owl-ontologies.com/VirtualHome.owl#read_yourself_to_sleep -->


    <owl:Class rdf:about="http://www.owl-ontologies.com/VirtualHome.owl#read_yourself_to_sleep">
        <rdfs:subClassOf rdf:resource="http://www.owl-ontologies.com/VirtualHome.owl#Leisure"/>
        <rdfs:comment>The class with sequence of actions for reading and falling to sleep 
while reading.</rdfs:comment>
    </owl:Class>
    


    <!-- http://www.owl-ontologies.com/VirtualHome.owl#rearrange_photo_frames -->


    <owl:Class rdf:about="http://www.owl-ontologies.com/VirtualHome.owl#rearrange_photo_frames">
        <rdfs:subClassOf rdf:resource="http://www.owl-ontologies.com/VirtualHome.owl#HouseArrangement"/>
        <rdfs:comment>The class with sequence of actions for rearranging photo frames.</rdfs:comment>
    </owl:Class>
    


    <!-- http://www.owl-ontologies.com/VirtualHome.owl#receive_credit_card -->


    <owl:Class rdf:about="http://www.owl-ontologies.com/VirtualHome.owl#receive_credit_card">
        <rdfs:subClassOf rdf:resource="http://www.owl-ontologies.com/VirtualHome.owl#Other"/>
        <rdfs:comment>The class with sequence of actions for receiving a credit card.</rdfs:comment>
    </owl:Class>
    


    <!-- http://www.owl-ontologies.com/VirtualHome.owl#recycle_items -->


    <owl:Class rdf:about="http://www.owl-ontologies.com/VirtualHome.owl#recycle_items">
        <rdfs:subClassOf rdf:resource="http://www.owl-ontologies.com/VirtualHome.owl#Other"/>
        <rdfs:comment>The class with sequence of actions for recycling items.</rdfs:comment>
    </owl:Class>
    


    <!-- http://www.owl-ontologies.com/VirtualHome.owl#relax -->


    <owl:Class rdf:about="http://www.owl-ontologies.com/VirtualHome.owl#relax">
        <rdfs:subClassOf rdf:resource="http://www.owl-ontologies.com/VirtualHome.owl#Leisure"/>
        <rdfs:comment>The class with sequence of actions for relaxing.</rdfs:comment>
    </owl:Class>
    


    <!-- http://www.owl-ontologies.com/VirtualHome.owl#relax_on_sofa -->


    <owl:Class rdf:about="http://www.owl-ontologies.com/VirtualHome.owl#relax_on_sofa">
        <rdfs:subClassOf rdf:resource="http://www.owl-ontologies.com/VirtualHome.owl#Leisure"/>
        <rdfs:comment>This class contains sequence of actions on how you can relax on a sofa.</rdfs:comment>
    </owl:Class>
    


    <!-- http://www.owl-ontologies.com/VirtualHome.owl#replace_toothpaste -->


    <owl:Class rdf:about="http://www.owl-ontologies.com/VirtualHome.owl#replace_toothpaste">
        <rdfs:subClassOf rdf:resource="http://www.owl-ontologies.com/VirtualHome.owl#HouseArrangement"/>
        <rdfs:comment>The class with sequence of actions for replacing the toohtpaste in any 
room.</rdfs:comment>
    </owl:Class>
    


    <!-- http://www.owl-ontologies.com/VirtualHome.owl#replace_towel -->


    <owl:Class rdf:about="http://www.owl-ontologies.com/VirtualHome.owl#replace_towel">
        <rdfs:subClassOf rdf:resource="http://www.owl-ontologies.com/VirtualHome.owl#Other"/>
        <rdfs:comment>The class with sequence of actions for replacing a towel, from any room.</rdfs:comment>
    </owl:Class>
    


    <!-- http://www.owl-ontologies.com/VirtualHome.owl#research -->


    <owl:Class rdf:about="http://www.owl-ontologies.com/VirtualHome.owl#research">
        <rdfs:subClassOf rdf:resource="http://www.owl-ontologies.com/VirtualHome.owl#Work"/>
        <rdfs:comment>The class with sequence of actions for performing research.</rdfs:comment>
    </owl:Class>
    


    <!-- http://www.owl-ontologies.com/VirtualHome.owl#restock -->


    <owl:Class rdf:about="http://www.owl-ontologies.com/VirtualHome.owl#restock">
        <rdfs:subClassOf rdf:resource="http://www.owl-ontologies.com/VirtualHome.owl#Other"/>
        <rdfs:comment>The class with sequence of actions for restocking, any place.</rdfs:comment>
    </owl:Class>
    


    <!-- http://www.owl-ontologies.com/VirtualHome.owl#return_from_store -->


    <owl:Class rdf:about="http://www.owl-ontologies.com/VirtualHome.owl#return_from_store">
        <rdfs:subClassOf rdf:resource="http://www.owl-ontologies.com/VirtualHome.owl#Other"/>
        <rdfs:comment>The class with sequence of actions for returning from the store.</rdfs:comment>
    </owl:Class>
    


    <!-- http://www.owl-ontologies.com/VirtualHome.owl#return_phone_calls -->


    <owl:Class rdf:about="http://www.owl-ontologies.com/VirtualHome.owl#return_phone_calls">
        <rdfs:subClassOf rdf:resource="http://www.owl-ontologies.com/VirtualHome.owl#Other"/>
        <rdfs:comment>The class with sequence of actions for returning phone calls, either 
from your cell phone or home phone.</rdfs:comment>
    </owl:Class>
    


    <!-- http://www.owl-ontologies.com/VirtualHome.owl#rotate_stock_in_refrigerator -->


    <owl:Class rdf:about="http://www.owl-ontologies.com/VirtualHome.owl#rotate_stock_in_refrigerator">
        <rdfs:subClassOf rdf:resource="http://www.owl-ontologies.com/VirtualHome.owl#HouseArrangement"/>
        <rdfs:comment>The class with sequence of actions for rotating stock in Refrigerator.</rdfs:comment>
    </owl:Class>
    


    <!-- http://www.owl-ontologies.com/VirtualHome.owl#say_goodbye -->


    <owl:Class rdf:about="http://www.owl-ontologies.com/VirtualHome.owl#say_goodbye">
        <rdfs:subClassOf rdf:resource="http://www.owl-ontologies.com/VirtualHome.owl#SocialInteraction"/>
        <rdfs:comment>The class with sequence of actions for greeding by saying goodbye.</rdfs:comment>
    </owl:Class>
    


    <!-- http://www.owl-ontologies.com/VirtualHome.owl#say_goodbye_to_guests_leaving -->


    <owl:Class rdf:about="http://www.owl-ontologies.com/VirtualHome.owl#say_goodbye_to_guests_leaving">
        <rdfs:subClassOf rdf:resource="http://www.owl-ontologies.com/VirtualHome.owl#SocialInteraction"/>
        <rdfs:comment>The class with sequence of actions for saying goodbye to guests leaving.</rdfs:comment>
    </owl:Class>
    


    <!-- http://www.owl-ontologies.com/VirtualHome.owl#scrub_bottom_of_feet -->


    <owl:Class rdf:about="http://www.owl-ontologies.com/VirtualHome.owl#scrub_bottom_of_feet">
        <rdfs:subClassOf rdf:resource="http://www.owl-ontologies.com/VirtualHome.owl#HygieneStyling"/>
        <rdfs:comment>The class with sequence of actions for scrubbing just the bottom of your feet.</rdfs:comment>
    </owl:Class>
    


    <!-- http://www.owl-ontologies.com/VirtualHome.owl#scrub_face -->


    <owl:Class rdf:about="http://www.owl-ontologies.com/VirtualHome.owl#scrub_face">
        <rdfs:subClassOf rdf:resource="http://www.owl-ontologies.com/VirtualHome.owl#HygieneStyling"/>
        <rdfs:comment>The class with sequence of actions for scrubing you face.</rdfs:comment>
    </owl:Class>
    


    <!-- http://www.owl-ontologies.com/VirtualHome.owl#scrub_toilet -->


    <owl:Class rdf:about="http://www.owl-ontologies.com/VirtualHome.owl#scrub_toilet">
        <rdfs:subClassOf rdf:resource="http://www.owl-ontologies.com/VirtualHome.owl#HouseCleaning"/>
        <rdfs:comment>The class with sequence of actions for scrubing the toilet.</rdfs:comment>
    </owl:Class>
    


    <!-- http://www.owl-ontologies.com/VirtualHome.owl#scrubbing_living_room_tile_floor_is_once_week_activity_for_me -->


    <owl:Class rdf:about="http://www.owl-ontologies.com/VirtualHome.owl#scrubbing_living_room_tile_floor_is_once_week_activity_for_me">
        <rdfs:subClassOf rdf:resource="http://www.owl-ontologies.com/VirtualHome.owl#HouseCleaning"/>
        <rdfs:comment>The class with sequence of actions for scrubbing living room tile floor is once a week activity for me.</rdfs:comment>
    </owl:Class>
    


    <!-- http://www.owl-ontologies.com/VirtualHome.owl#send__email -->


    <owl:Class rdf:about="http://www.owl-ontologies.com/VirtualHome.owl#send__email">
        <rdfs:subClassOf rdf:resource="http://www.owl-ontologies.com/VirtualHome.owl#Work"/>
        <rdfs:comment>The class with sequence of actions for sending an email.</rdfs:comment>
    </owl:Class>
    


    <!-- http://www.owl-ontologies.com/VirtualHome.owl#sent_email -->


    <owl:Class rdf:about="http://www.owl-ontologies.com/VirtualHome.owl#sent_email">
        <rdfs:subClassOf rdf:resource="http://www.owl-ontologies.com/VirtualHome.owl#Work"/>
        <rdfs:comment>The class with sequence of actions to send a email.</rdfs:comment>
    </owl:Class>
    


    <!-- http://www.owl-ontologies.com/VirtualHome.owl#serve_breakfast -->


    <owl:Class rdf:about="http://www.owl-ontologies.com/VirtualHome.owl#serve_breakfast">
        <rdfs:subClassOf rdf:resource="http://www.owl-ontologies.com/VirtualHome.owl#Other"/>
        <rdfs:comment>The class with sequence of actions for serving breakfast, in any room.</rdfs:comment>
    </owl:Class>
    


    <!-- http://www.owl-ontologies.com/VirtualHome.owl#serve_cookies -->


    <owl:Class rdf:about="http://www.owl-ontologies.com/VirtualHome.owl#serve_cookies">
        <rdfs:subClassOf rdf:resource="http://www.owl-ontologies.com/VirtualHome.owl#Other"/>
        <rdfs:comment>The class with sequence of actions for serving cookies, for any occasion.</rdfs:comment>
    </owl:Class>
    


    <!-- http://www.owl-ontologies.com/VirtualHome.owl#serve_food -->


    <owl:Class rdf:about="http://www.owl-ontologies.com/VirtualHome.owl#serve_food">
        <rdfs:subClassOf rdf:resource="http://www.owl-ontologies.com/VirtualHome.owl#Other"/>
        <rdfs:comment>The class with sequence of actions for serving the food in any room.</rdfs:comment>
    </owl:Class>
    


    <!-- http://www.owl-ontologies.com/VirtualHome.owl#serve_hors_doeurves_to_entering_guests_at_cocktail_party -->


    <owl:Class rdf:about="http://www.owl-ontologies.com/VirtualHome.owl#serve_hors_doeurves_to_entering_guests_at_cocktail_party">
        <rdfs:subClassOf rdf:resource="http://www.owl-ontologies.com/VirtualHome.owl#SocialInteraction"/>
        <rdfs:comment>The class with sequence of actions for srving hors doeurves to entering guest at cocktail party.</rdfs:comment>
    </owl:Class>
    


    <!-- http://www.owl-ontologies.com/VirtualHome.owl#serve_meal -->


    <owl:Class rdf:about="http://www.owl-ontologies.com/VirtualHome.owl#serve_meal">
        <rdfs:subClassOf rdf:resource="http://www.owl-ontologies.com/VirtualHome.owl#Other"/>
        <rdfs:comment>The class with sequence of actions for serving meal in any room.</rdfs:comment>
    </owl:Class>
    


    <!-- http://www.owl-ontologies.com/VirtualHome.owl#set_mail_on_table -->


    <owl:Class rdf:about="http://www.owl-ontologies.com/VirtualHome.owl#set_mail_on_table">
        <rdfs:subClassOf rdf:resource="http://www.owl-ontologies.com/VirtualHome.owl#Other"/>
        <rdfs:comment>The class with sequence of actions for setting the mail on the table, for eating.</rdfs:comment>
    </owl:Class>
    


    <!-- http://www.owl-ontologies.com/VirtualHome.owl#set_out_some_snacks_for_toddler -->


    <owl:Class rdf:about="http://www.owl-ontologies.com/VirtualHome.owl#set_out_some_snacks_for_toddler">
        <rdfs:subClassOf rdf:resource="http://www.owl-ontologies.com/VirtualHome.owl#Other"/>
        <rdfs:comment>The class with sequence of actions for setting out some snacks for toddler.</rdfs:comment>
    </owl:Class>
    


    <!-- http://www.owl-ontologies.com/VirtualHome.owl#set_up_buffet_area -->


    <owl:Class rdf:about="http://www.owl-ontologies.com/VirtualHome.owl#set_up_buffet_area">
        <rdfs:subClassOf rdf:resource="http://www.owl-ontologies.com/VirtualHome.owl#HouseArrangement"/>
        <rdfs:comment>The class with sequence of actions for setting up the buffet area.</rdfs:comment>
    </owl:Class>
    


    <!-- http://www.owl-ontologies.com/VirtualHome.owl#set_up_table -->


    <owl:Class rdf:about="http://www.owl-ontologies.com/VirtualHome.owl#set_up_table">
        <rdfs:subClassOf rdf:resource="http://www.owl-ontologies.com/VirtualHome.owl#HouseArrangement"/>
        <rdfs:comment>Class with sequences about how to perform the set up of a dinner, kitchen table.</rdfs:comment>
    </owl:Class>
    


    <!-- http://www.owl-ontologies.com/VirtualHome.owl#set_up_tv -->


    <owl:Class rdf:about="http://www.owl-ontologies.com/VirtualHome.owl#set_up_tv">
        <rdfs:subClassOf rdf:resource="http://www.owl-ontologies.com/VirtualHome.owl#Other"/>
        <rdfs:comment>The class with sequence of actions for seeting up the TV.</rdfs:comment>
    </owl:Class>
    


    <!-- http://www.owl-ontologies.com/VirtualHome.owl#settle_in -->


    <owl:Class rdf:about="http://www.owl-ontologies.com/VirtualHome.owl#settle_in">
        <rdfs:subClassOf rdf:resource="http://www.owl-ontologies.com/VirtualHome.owl#Other"/>
        <rdfs:comment>The class with sequence of actions for settling in the house.</rdfs:comment>
    </owl:Class>
    


    <!-- http://www.owl-ontologies.com/VirtualHome.owl#sew_button -->


    <owl:Class rdf:about="http://www.owl-ontologies.com/VirtualHome.owl#sew_button">
        <rdfs:subClassOf rdf:resource="http://www.owl-ontologies.com/VirtualHome.owl#Other"/>
        <rdfs:comment>The class with sequence of actions for sewing the button, from any 
remote control.</rdfs:comment>
    </owl:Class>
    


    <!-- http://www.owl-ontologies.com/VirtualHome.owl#shampoo_hair -->


    <owl:Class rdf:about="http://www.owl-ontologies.com/VirtualHome.owl#shampoo_hair">
        <rdfs:subClassOf rdf:resource="http://www.owl-ontologies.com/VirtualHome.owl#HygieneStyling"/>
        <rdfs:comment>The class with sequence of actions for shampooing your hair.</rdfs:comment>
    </owl:Class>
    


    <!-- http://www.owl-ontologies.com/VirtualHome.owl#shoe_removal -->


    <owl:Class rdf:about="http://www.owl-ontologies.com/VirtualHome.owl#shoe_removal">
        <rdfs:subClassOf rdf:resource="http://www.owl-ontologies.com/VirtualHome.owl#Other"/>
        <rdfs:comment>The class with sequence of actions for removing your shoes in any room.</rdfs:comment>
    </owl:Class>
    


    <!-- http://www.owl-ontologies.com/VirtualHome.owl#shop -->


    <owl:Class rdf:about="http://www.owl-ontologies.com/VirtualHome.owl#shop">
        <rdfs:subClassOf rdf:resource="http://www.owl-ontologies.com/VirtualHome.owl#Other"/>
        <rdfs:comment>The class with sequence of actions for shopping either by calling, or 
from the internet (shopping from household environment).</rdfs:comment>
    </owl:Class>
    


    <!-- http://www.owl-ontologies.com/VirtualHome.owl#shred_receipts -->


    <owl:Class rdf:about="http://www.owl-ontologies.com/VirtualHome.owl#shred_receipts">
        <rdfs:subClassOf rdf:resource="http://www.owl-ontologies.com/VirtualHome.owl#HouseCleaning"/>
        <rdfs:comment>The class with sequence of actions for shred of receipts.</rdfs:comment>
    </owl:Class>
    


    <!-- http://www.owl-ontologies.com/VirtualHome.owl#shredding -->


    <owl:Class rdf:about="http://www.owl-ontologies.com/VirtualHome.owl#shredding">
        <rdfs:subClassOf rdf:resource="http://www.owl-ontologies.com/VirtualHome.owl#Other"/>
        <rdfs:comment>The class with sequence of actions for shredding any object in any room.</rdfs:comment>
    </owl:Class>
    


    <!-- http://www.owl-ontologies.com/VirtualHome.owl#shut_front_door -->


    <owl:Class rdf:about="http://www.owl-ontologies.com/VirtualHome.owl#shut_front_door">
        <rdfs:subClassOf rdf:resource="http://www.owl-ontologies.com/VirtualHome.owl#Other"/>
        <rdfs:comment>The class with sequence of actions for shutting front door (door of main entrance).</rdfs:comment>
    </owl:Class>
    


    <!-- http://www.owl-ontologies.com/VirtualHome.owl#shut_off_alarm -->


    <owl:Class rdf:about="http://www.owl-ontologies.com/VirtualHome.owl#shut_off_alarm">
        <rdfs:subClassOf rdf:resource="http://www.owl-ontologies.com/VirtualHome.owl#Other"/>
        <rdfs:comment>The class with sequence of actions for shutting of the alarm in any room.</rdfs:comment>
    </owl:Class>
    


    <!-- http://www.owl-ontologies.com/VirtualHome.owl#sing_karaoke -->


    <owl:Class rdf:about="http://www.owl-ontologies.com/VirtualHome.owl#sing_karaoke">
        <rdfs:subClassOf rdf:resource="http://www.owl-ontologies.com/VirtualHome.owl#Leisure"/>
        <rdfs:comment>The class with sequence of actions for singing at the karoke.</rdfs:comment>
    </owl:Class>
    


    <!-- http://www.owl-ontologies.com/VirtualHome.owl#sing_song -->


    <owl:Class rdf:about="http://www.owl-ontologies.com/VirtualHome.owl#sing_song">
        <rdfs:subClassOf rdf:resource="http://www.owl-ontologies.com/VirtualHome.owl#Leisure"/>
        <rdfs:comment>The class with sequence of actions for singing songs.</rdfs:comment>
    </owl:Class>
    


    <!-- http://www.owl-ontologies.com/VirtualHome.owl#sit_in_chair -->


    <owl:Class rdf:about="http://www.owl-ontologies.com/VirtualHome.owl#sit_in_chair">
        <rdfs:subClassOf rdf:resource="http://www.owl-ontologies.com/VirtualHome.owl#Other"/>
        <rdfs:comment>The class with sequence of actions for sitting in the chair, in any type 
of chair in any room.</rdfs:comment>
    </owl:Class>
    


    <!-- http://www.owl-ontologies.com/VirtualHome.owl#sit_quietly -->


    <owl:Class rdf:about="http://www.owl-ontologies.com/VirtualHome.owl#sit_quietly">
        <rdfs:subClassOf rdf:resource="http://www.owl-ontologies.com/VirtualHome.owl#Other"/>
        <rdfs:comment>The class with sequence of actions for sitting quetly, in any room.</rdfs:comment>
    </owl:Class>
    


    <!-- http://www.owl-ontologies.com/VirtualHome.owl#sleep -->


    <owl:Class rdf:about="http://www.owl-ontologies.com/VirtualHome.owl#sleep">
        <rdfs:subClassOf rdf:resource="http://www.owl-ontologies.com/VirtualHome.owl#BedTimeSleep"/>
        <rdfs:comment>The class with sequence of actions for sleeping.</rdfs:comment>
    </owl:Class>
    


    <!-- http://www.owl-ontologies.com/VirtualHome.owl#slice_apple -->


    <owl:Class rdf:about="http://www.owl-ontologies.com/VirtualHome.owl#slice_apple">
        <rdfs:subClassOf rdf:resource="http://www.owl-ontologies.com/VirtualHome.owl#FoodPreparation"/>
        <rdfs:comment>The class with sequence of actions for slicing an apple.</rdfs:comment>
    </owl:Class>
    


    <!-- http://www.owl-ontologies.com/VirtualHome.owl#social_media__checks -->


    <owl:Class rdf:about="http://www.owl-ontologies.com/VirtualHome.owl#social_media__checks">
        <rdfs:subClassOf rdf:resource="http://www.owl-ontologies.com/VirtualHome.owl#Leisure"/>
        <rdfs:comment>The class with sequence of actions for chencking your social media 
applications.</rdfs:comment>
    </owl:Class>
    


    <!-- http://www.owl-ontologies.com/VirtualHome.owl#sort_and_fold_laundry -->


    <owl:Class rdf:about="http://www.owl-ontologies.com/VirtualHome.owl#sort_and_fold_laundry">
        <rdfs:subClassOf rdf:resource="http://www.owl-ontologies.com/VirtualHome.owl#HouseCleaning"/>
        <rdfs:comment>The class with sequence of actions for sorting and folding laundry.</rdfs:comment>
    </owl:Class>
    


    <!-- http://www.owl-ontologies.com/VirtualHome.owl#sort_clothing_and_care_for_it -->


    <owl:Class rdf:about="http://www.owl-ontologies.com/VirtualHome.owl#sort_clothing_and_care_for_it">
        <rdfs:subClassOf rdf:resource="http://www.owl-ontologies.com/VirtualHome.owl#HouseArrangement"/>
        <rdfs:comment>The class with sequence of actions for sorting clothing in specific order.</rdfs:comment>
    </owl:Class>
    


    <!-- http://www.owl-ontologies.com/VirtualHome.owl#sort_laundry -->


    <owl:Class rdf:about="http://www.owl-ontologies.com/VirtualHome.owl#sort_laundry">
        <rdfs:subClassOf rdf:resource="http://www.owl-ontologies.com/VirtualHome.owl#HouseArrangement"/>
        <rdfs:comment>The class with sequence of actions for sorting laundry by category.</rdfs:comment>
    </owl:Class>
    


    <!-- http://www.owl-ontologies.com/VirtualHome.owl#sort_mail -->


    <owl:Class rdf:about="http://www.owl-ontologies.com/VirtualHome.owl#sort_mail">
        <rdfs:subClassOf rdf:resource="http://www.owl-ontologies.com/VirtualHome.owl#Other"/>
        <rdfs:comment>The class with sequence of actions for sorting mail, in any desired 
order.</rdfs:comment>
    </owl:Class>
    


    <!-- http://www.owl-ontologies.com/VirtualHome.owl#speaking_on_headset_in_skype_or_some_form_of_voip_for_business_call -->


    <owl:Class rdf:about="http://www.owl-ontologies.com/VirtualHome.owl#speaking_on_headset_in_skype_or_some_form_of_voip_for_business_call">
        <rdfs:subClassOf rdf:resource="http://www.owl-ontologies.com/VirtualHome.owl#SocialInteraction"/>
        <rdfs:subClassOf rdf:resource="http://www.owl-ontologies.com/VirtualHome.owl#Work"/>
        <rdfs:comment>The class with sequence of actions for speaking on headset in skype or 
some form of voip for business call.</rdfs:comment>
        <rdfs:comment>The class with sequence of actions for speaking on headset in skype or some form of voip for business call.</rdfs:comment>
    </owl:Class>
    


    <!-- http://www.owl-ontologies.com/VirtualHome.owl#spend_family_time_playing_games -->


    <owl:Class rdf:about="http://www.owl-ontologies.com/VirtualHome.owl#spend_family_time_playing_games">
        <rdfs:subClassOf rdf:resource="http://www.owl-ontologies.com/VirtualHome.owl#SocialInteraction"/>
        <rdfs:comment>The class with sequence of actions for spending family time playing games, videogames of any other games.</rdfs:comment>
    </owl:Class>
    


    <!-- http://www.owl-ontologies.com/VirtualHome.owl#spread_table_with_appropriate_supplies -->


    <owl:Class rdf:about="http://www.owl-ontologies.com/VirtualHome.owl#spread_table_with_appropriate_supplies">
        <rdfs:subClassOf rdf:resource="http://www.owl-ontologies.com/VirtualHome.owl#Other"/>
        <rdfs:comment>The class with sequence of actions for spreading the table with 
approproate supplies.</rdfs:comment>
    </owl:Class>
    


    <!-- http://www.owl-ontologies.com/VirtualHome.owl#squeeze_lemon -->


    <owl:Class rdf:about="http://www.owl-ontologies.com/VirtualHome.owl#squeeze_lemon">
        <rdfs:subClassOf rdf:resource="http://www.owl-ontologies.com/VirtualHome.owl#FoodPreparation"/>
        <rdfs:comment>The class with sequence of actions for squezing a lemon.</rdfs:comment>
    </owl:Class>
    


    <!-- http://www.owl-ontologies.com/VirtualHome.owl#start_computer -->


    <owl:Class rdf:about="http://www.owl-ontologies.com/VirtualHome.owl#start_computer">
        <rdfs:subClassOf rdf:resource="http://www.owl-ontologies.com/VirtualHome.owl#Other"/>
        <rdfs:comment>The class with sequence of actions for starting your computer, either 
laptop or personal computer.</rdfs:comment>
    </owl:Class>
    


    <!-- http://www.owl-ontologies.com/VirtualHome.owl#steam_mop_floor -->


    <owl:Class rdf:about="http://www.owl-ontologies.com/VirtualHome.owl#steam_mop_floor">
        <rdfs:subClassOf rdf:resource="http://www.owl-ontologies.com/VirtualHome.owl#HouseCleaning"/>
        <rdfs:comment>The class with sequence of actions for steaming mop floor.</rdfs:comment>
    </owl:Class>
    


    <!-- http://www.owl-ontologies.com/VirtualHome.owl#story_reading_time -->


    <owl:Class rdf:about="http://www.owl-ontologies.com/VirtualHome.owl#story_reading_time">
        <rdfs:subClassOf rdf:resource="http://www.owl-ontologies.com/VirtualHome.owl#SocialInteraction"/>
        <rdfs:comment>The class with sequence of actions for story reading time, in any room.</rdfs:comment>
    </owl:Class>
    


    <!-- http://www.owl-ontologies.com/VirtualHome.owl#straighten_bookshelf -->


    <owl:Class rdf:about="http://www.owl-ontologies.com/VirtualHome.owl#straighten_bookshelf">
        <rdfs:subClassOf rdf:resource="http://www.owl-ontologies.com/VirtualHome.owl#Other"/>
        <rdfs:comment>The class with sequence of actions for straightening the bookself, in 
any room.</rdfs:comment>
    </owl:Class>
    


    <!-- http://www.owl-ontologies.com/VirtualHome.owl#straighten_magazines -->


    <owl:Class rdf:about="http://www.owl-ontologies.com/VirtualHome.owl#straighten_magazines">
        <rdfs:subClassOf rdf:resource="http://www.owl-ontologies.com/VirtualHome.owl#HouseArrangement"/>
        <rdfs:comment>The class with sequence of actions for straighten magaziens that are 
placed in a folder or on a surface.</rdfs:comment>
    </owl:Class>
    


    <!-- http://www.owl-ontologies.com/VirtualHome.owl#straighten_paintings_on_wall -->


    <owl:Class rdf:about="http://www.owl-ontologies.com/VirtualHome.owl#straighten_paintings_on_wall">
        <rdfs:subClassOf rdf:resource="http://www.owl-ontologies.com/VirtualHome.owl#HouseArrangement"/>
        <rdfs:comment>The class with sequence of actions for straightening paintings on wall 
(only painting not pictures).</rdfs:comment>
    </owl:Class>
    


    <!-- http://www.owl-ontologies.com/VirtualHome.owl#straighten_pictures_on_wall -->


    <owl:Class rdf:about="http://www.owl-ontologies.com/VirtualHome.owl#straighten_pictures_on_wall">
        <rdfs:subClassOf rdf:resource="http://www.owl-ontologies.com/VirtualHome.owl#HouseArrangement"/>
        <rdfs:comment>The class with sequence of actions for straighten pictures on wall, in any room.</rdfs:comment>
    </owl:Class>
    


    <!-- http://www.owl-ontologies.com/VirtualHome.owl#string_green_beans -->


    <owl:Class rdf:about="http://www.owl-ontologies.com/VirtualHome.owl#string_green_beans">
        <rdfs:subClassOf rdf:resource="http://www.owl-ontologies.com/VirtualHome.owl#Other"/>
        <rdfs:comment>The class with sequence of actions for stringing green beans, in any 
room.</rdfs:comment>
    </owl:Class>
    


    <!-- http://www.owl-ontologies.com/VirtualHome.owl#study -->


    <owl:Class rdf:about="http://www.owl-ontologies.com/VirtualHome.owl#study">
        <rdfs:subClassOf rdf:resource="http://www.owl-ontologies.com/VirtualHome.owl#Work"/>
        <rdfs:comment>The class with sequence of actions for studying, no matter on what (computer, paper).</rdfs:comment>
    </owl:Class>
    


    <!-- http://www.owl-ontologies.com/VirtualHome.owl#study_bible -->


    <owl:Class rdf:about="http://www.owl-ontologies.com/VirtualHome.owl#study_bible">
        <rdfs:subClassOf rdf:resource="http://www.owl-ontologies.com/VirtualHome.owl#Work"/>
        <rdfs:comment>The class with sequence of actions for studying the biblie.</rdfs:comment>
    </owl:Class>
    


    <!-- http://www.owl-ontologies.com/VirtualHome.owl#style_hair -->


    <owl:Class rdf:about="http://www.owl-ontologies.com/VirtualHome.owl#style_hair">
        <rdfs:subClassOf rdf:resource="http://www.owl-ontologies.com/VirtualHome.owl#HygieneStyling"/>
        <rdfs:comment>The class with sequence of actions for styling your hair.</rdfs:comment>
    </owl:Class>
    


    <!-- http://www.owl-ontologies.com/VirtualHome.owl#surf_internet -->


    <owl:Class rdf:about="http://www.owl-ontologies.com/VirtualHome.owl#surf_internet">
        <rdfs:subClassOf rdf:resource="http://www.owl-ontologies.com/VirtualHome.owl#Leisure"/>
        <rdfs:comment>The class with sequence of actions for surfing the internet.</rdfs:comment>
    </owl:Class>
    


    <!-- http://www.owl-ontologies.com/VirtualHome.owl#surf_net -->


    <owl:Class rdf:about="http://www.owl-ontologies.com/VirtualHome.owl#surf_net">
        <rdfs:subClassOf rdf:resource="http://www.owl-ontologies.com/VirtualHome.owl#Leisure"/>
        <rdfs:comment>The class with sequence of actions for surfing the net.</rdfs:comment>
    </owl:Class>
    


    <!-- http://www.owl-ontologies.com/VirtualHome.owl#surf_web_for_money_legitimate_making_opportunities -->


    <owl:Class rdf:about="http://www.owl-ontologies.com/VirtualHome.owl#surf_web_for_money_legitimate_making_opportunities">
        <rdfs:subClassOf rdf:resource="http://www.owl-ontologies.com/VirtualHome.owl#Work"/>
        <rdfs:comment>The class with sequence of actions for searching in the internet for 
legitimate maikng opportunities.</rdfs:comment>
    </owl:Class>
    


    <!-- http://www.owl-ontologies.com/VirtualHome.owl#sweep_and_wipe_table_off_with_rag -->


    <owl:Class rdf:about="http://www.owl-ontologies.com/VirtualHome.owl#sweep_and_wipe_table_off_with_rag">
        <rdfs:subClassOf rdf:resource="http://www.owl-ontologies.com/VirtualHome.owl#HouseCleaning"/>
        <rdfs:comment>The class with sequence of actions for sweeping and wiping a table off 
with a rag.</rdfs:comment>
    </owl:Class>
    


    <!-- http://www.owl-ontologies.com/VirtualHome.owl#sweep_entrance_hall -->


    <owl:Class rdf:about="http://www.owl-ontologies.com/VirtualHome.owl#sweep_entrance_hall">
        <rdfs:subClassOf rdf:resource="http://www.owl-ontologies.com/VirtualHome.owl#HouseCleaning"/>
        <rdfs:comment>The class with sequence of actions on how to sweep the entrance hall.</rdfs:comment>
    </owl:Class>
    


    <!-- http://www.owl-ontologies.com/VirtualHome.owl#sweep_floor -->


    <owl:Class rdf:about="http://www.owl-ontologies.com/VirtualHome.owl#sweep_floor">
        <rdfs:subClassOf rdf:resource="http://www.owl-ontologies.com/VirtualHome.owl#HouseCleaning"/>
        <rdfs:comment>The class with sequence of actions for house cleaning.</rdfs:comment>
    </owl:Class>
    


    <!-- http://www.owl-ontologies.com/VirtualHome.owl#sweep_hallway_please -->


    <owl:Class rdf:about="http://www.owl-ontologies.com/VirtualHome.owl#sweep_hallway_please">
        <rdfs:subClassOf rdf:resource="http://www.owl-ontologies.com/VirtualHome.owl#HouseCleaning"/>
        <rdfs:comment>he class with sequence of actions to sweep the hallway after you got 
the verbal token &quot;please&quot;.</rdfs:comment>
    </owl:Class>
    


    <!-- http://www.owl-ontologies.com/VirtualHome.owl#switch_on_lamp -->


    <owl:Class rdf:about="http://www.owl-ontologies.com/VirtualHome.owl#switch_on_lamp">
        <rdfs:subClassOf rdf:resource="http://www.owl-ontologies.com/VirtualHome.owl#Other"/>
        <rdfs:comment>The class with sequence of actions for switching on lamp, in any room.</rdfs:comment>
    </owl:Class>
    


    <!-- http://www.owl-ontologies.com/VirtualHome.owl#tabletop_game -->


    <owl:Class rdf:about="http://www.owl-ontologies.com/VirtualHome.owl#tabletop_game">
        <rdfs:subClassOf rdf:resource="http://www.owl-ontologies.com/VirtualHome.owl#Leisure"/>
        <rdfs:comment>The class with sequence of actions for playin tabletop games (board 
games).</rdfs:comment>
    </owl:Class>
    


    <!-- http://www.owl-ontologies.com/VirtualHome.owl#take_a_nap -->


    <owl:Class rdf:about="http://www.owl-ontologies.com/VirtualHome.owl#take_a_nap">
        <rdfs:subClassOf rdf:resource="http://www.owl-ontologies.com/VirtualHome.owl#BedTimeSleep"/>
    </owl:Class>
    


    <!-- http://www.owl-ontologies.com/VirtualHome.owl#take_bath -->


    <owl:Class rdf:about="http://www.owl-ontologies.com/VirtualHome.owl#take_bath">
        <rdfs:subClassOf rdf:resource="http://www.owl-ontologies.com/VirtualHome.owl#HygieneStyling"/>
        <rdfs:comment>Class with seqeunces on how you can take a bath, and clean yourself (not a shower).</rdfs:comment>
    </owl:Class>
    


    <!-- http://www.owl-ontologies.com/VirtualHome.owl#take_coat -->


    <owl:Class rdf:about="http://www.owl-ontologies.com/VirtualHome.owl#take_coat">
        <rdfs:subClassOf rdf:resource="http://www.owl-ontologies.com/VirtualHome.owl#Other"/>
        <rdfs:comment>The class with sequence of actions for taking the coat, and place it 
somewhere.</rdfs:comment>
    </owl:Class>
    


    <!-- http://www.owl-ontologies.com/VirtualHome.owl#take_dishes_out_of_dishwasher -->


    <owl:Class rdf:about="http://www.owl-ontologies.com/VirtualHome.owl#take_dishes_out_of_dishwasher">
        <rdfs:subClassOf rdf:resource="http://www.owl-ontologies.com/VirtualHome.owl#HouseArrangement"/>
        <rdfs:comment>The class with sequence of actions for taking dishes out of dishwasher.</rdfs:comment>
    </owl:Class>
    


    <!-- http://www.owl-ontologies.com/VirtualHome.owl#take_jacket_off -->


    <owl:Class rdf:about="http://www.owl-ontologies.com/VirtualHome.owl#take_jacket_off">
        <rdfs:subClassOf rdf:resource="http://www.owl-ontologies.com/VirtualHome.owl#HygieneStyling"/>
        <rdfs:comment>The class with sequence of actions for taking your jacket off.</rdfs:comment>
    </owl:Class>
    


    <!-- http://www.owl-ontologies.com/VirtualHome.owl#take_nap -->


    <owl:Class rdf:about="http://www.owl-ontologies.com/VirtualHome.owl#take_nap">
        <rdfs:subClassOf rdf:resource="http://www.owl-ontologies.com/VirtualHome.owl#BedTimeSleep"/>
        <rdfs:comment>A class with sequences on how to go take a small nap.</rdfs:comment>
    </owl:Class>
    


    <!-- http://www.owl-ontologies.com/VirtualHome.owl#take_of_outerwear -->


    <owl:Class rdf:about="http://www.owl-ontologies.com/VirtualHome.owl#take_of_outerwear">
        <rdfs:subClassOf rdf:resource="http://www.owl-ontologies.com/VirtualHome.owl#Other"/>
        <rdfs:comment>The class with sequence of actions for taking of outerwear.</rdfs:comment>
    </owl:Class>
    


    <!-- http://www.owl-ontologies.com/VirtualHome.owl#take_off_clock -->


    <owl:Class rdf:about="http://www.owl-ontologies.com/VirtualHome.owl#take_off_clock">
        <rdfs:subClassOf rdf:resource="http://www.owl-ontologies.com/VirtualHome.owl#HouseArrangement"/>
    </owl:Class>
    


    <!-- http://www.owl-ontologies.com/VirtualHome.owl#take_off_coat -->


    <owl:Class rdf:about="http://www.owl-ontologies.com/VirtualHome.owl#take_off_coat">
        <rdfs:subClassOf rdf:resource="http://www.owl-ontologies.com/VirtualHome.owl#HygieneStyling"/>
        <rdfs:comment>The class with sequence of actions for taking of your coat.</rdfs:comment>
    </owl:Class>
    


    <!-- http://www.owl-ontologies.com/VirtualHome.owl#take_off_outerwear -->


    <owl:Class rdf:about="http://www.owl-ontologies.com/VirtualHome.owl#take_off_outerwear">
        <rdfs:subClassOf rdf:resource="http://www.owl-ontologies.com/VirtualHome.owl#GettingReady"/>
        <rdfs:comment>The class with sequence of actions for getting ready.</rdfs:comment>
    </owl:Class>
    


    <!-- http://www.owl-ontologies.com/VirtualHome.owl#take_off_shoes -->


    <owl:Class rdf:about="http://www.owl-ontologies.com/VirtualHome.owl#take_off_shoes">
        <rdfs:subClassOf rdf:resource="http://www.owl-ontologies.com/VirtualHome.owl#HygieneStyling"/>
        <rdfs:comment>Class with seqeunces on how to take off your shoes after work, or before 
getting to bed, or watch tv.</rdfs:comment>
    </owl:Class>
    


    <!-- http://www.owl-ontologies.com/VirtualHome.owl#take_off_shoes_and_hang_up_coat -->


    <owl:Class rdf:about="http://www.owl-ontologies.com/VirtualHome.owl#take_off_shoes_and_hang_up_coat">
        <rdfs:subClassOf rdf:resource="http://www.owl-ontologies.com/VirtualHome.owl#HygieneStyling"/>
        <rdfs:comment>The class with sequence of actions for hanging up your coat.</rdfs:comment>
    </owl:Class>
    


    <!-- http://www.owl-ontologies.com/VirtualHome.owl#take_shoes_off -->


    <owl:Class rdf:about="http://www.owl-ontologies.com/VirtualHome.owl#take_shoes_off">
        <rdfs:subClassOf rdf:resource="http://www.owl-ontologies.com/VirtualHome.owl#HygieneStyling"/>
        <rdfs:comment>The class with sequence of actions for taking yur shoes off.</rdfs:comment>
    </owl:Class>
    


    <!-- http://www.owl-ontologies.com/VirtualHome.owl#take_shower -->


    <owl:Class rdf:about="http://www.owl-ontologies.com/VirtualHome.owl#take_shower">
        <rdfs:subClassOf rdf:resource="http://www.owl-ontologies.com/VirtualHome.owl#HygieneStyling"/>
        <rdfs:comment>Class with seqeunces of action on how to take a shower (not a bath)
.</rdfs:comment>
    </owl:Class>
    


    <!-- http://www.owl-ontologies.com/VirtualHome.owl#tale_off_shoes -->


    <owl:Class rdf:about="http://www.owl-ontologies.com/VirtualHome.owl#tale_off_shoes">
        <rdfs:subClassOf rdf:resource="http://www.owl-ontologies.com/VirtualHome.owl#HygieneStyling"/>
        <rdfs:comment>The class with sequence of actions for taling of your own shoes.</rdfs:comment>
    </owl:Class>
    


    <!-- http://www.owl-ontologies.com/VirtualHome.owl#talk_on_phone -->


    <owl:Class rdf:about="http://www.owl-ontologies.com/VirtualHome.owl#talk_on_phone">
        <rdfs:subClassOf rdf:resource="http://www.owl-ontologies.com/VirtualHome.owl#SocialInteraction"/>
        <rdfs:comment>The class with sequence of actions for talking on phone, either cell 
phone or phone at home.</rdfs:comment>
    </owl:Class>
    


    <!-- http://www.owl-ontologies.com/VirtualHome.owl#talk_to_kids -->


    <owl:Class rdf:about="http://www.owl-ontologies.com/VirtualHome.owl#talk_to_kids">
        <rdfs:subClassOf rdf:resource="http://www.owl-ontologies.com/VirtualHome.owl#SocialInteraction"/>
        <rdfs:comment>The class with sequence of actions for talking to kids in any room.</rdfs:comment>
    </owl:Class>
    


    <!-- http://www.owl-ontologies.com/VirtualHome.owl#talk_with_friends -->


    <owl:Class rdf:about="http://www.owl-ontologies.com/VirtualHome.owl#talk_with_friends">
        <rdfs:subClassOf rdf:resource="http://www.owl-ontologies.com/VirtualHome.owl#SocialInteraction"/>
        <rdfs:comment>The class with sequence of actions for talking to your friend, no matter 
the genre.</rdfs:comment>
    </owl:Class>
    


    <!-- http://www.owl-ontologies.com/VirtualHome.owl#talk_with_guest -->


    <owl:Class rdf:about="http://www.owl-ontologies.com/VirtualHome.owl#talk_with_guest">
        <rdfs:subClassOf rdf:resource="http://www.owl-ontologies.com/VirtualHome.owl#SocialInteraction"/>
        <rdfs:comment>The class with sequence of actions for talking to guest.</rdfs:comment>
    </owl:Class>
    


    <!-- http://www.owl-ontologies.com/VirtualHome.owl#talk_with_your_child_about_their_day -->


    <owl:Class rdf:about="http://www.owl-ontologies.com/VirtualHome.owl#talk_with_your_child_about_their_day">
        <rdfs:subClassOf rdf:resource="http://www.owl-ontologies.com/VirtualHome.owl#SocialInteraction"/>
        <rdfs:comment>The class with sequence of actions for talking with your child about 
their day.</rdfs:comment>
    </owl:Class>
    


    <!-- http://www.owl-ontologies.com/VirtualHome.owl#tax_filing -->


    <owl:Class rdf:about="http://www.owl-ontologies.com/VirtualHome.owl#tax_filing">
        <rdfs:subClassOf rdf:resource="http://www.owl-ontologies.com/VirtualHome.owl#Work"/>
        <rdfs:comment>The class with sequence of actions for filling your taxes.</rdfs:comment>
    </owl:Class>
    


    <!-- http://www.owl-ontologies.com/VirtualHome.owl#teach_them_to_make_their_bed -->


    <owl:Class rdf:about="http://www.owl-ontologies.com/VirtualHome.owl#teach_them_to_make_their_bed">
        <rdfs:subClassOf rdf:resource="http://www.owl-ontologies.com/VirtualHome.owl#Other"/>
        <rdfs:comment>The class with sequence of actions for teaching them (other persons), to 
make their beds.</rdfs:comment>
    </owl:Class>
    


    <!-- http://www.owl-ontologies.com/VirtualHome.owl#tell_jokes -->


    <owl:Class rdf:about="http://www.owl-ontologies.com/VirtualHome.owl#tell_jokes">
        <rdfs:subClassOf rdf:resource="http://www.owl-ontologies.com/VirtualHome.owl#SocialInteraction"/>
        <rdfs:comment>The class with sequence of actions for telling jokes to any individual.</rdfs:comment>
    </owl:Class>
    


    <!-- http://www.owl-ontologies.com/VirtualHome.owl#text_friend -->


    <owl:Class rdf:about="http://www.owl-ontologies.com/VirtualHome.owl#text_friend">
        <rdfs:subClassOf rdf:resource="http://www.owl-ontologies.com/VirtualHome.owl#SocialInteraction"/>
        <rdfs:comment>The class with sequence of actions for texting a friend.</rdfs:comment>
    </owl:Class>
    


    <!-- http://www.owl-ontologies.com/VirtualHome.owl#text_friends_while_sitting_on_couch -->


    <owl:Class rdf:about="http://www.owl-ontologies.com/VirtualHome.owl#text_friends_while_sitting_on_couch">
        <rdfs:subClassOf rdf:resource="http://www.owl-ontologies.com/VirtualHome.owl#SocialInteraction"/>
        <rdfs:comment>The class with sequence of actions for texting a frined while you are 
sitting on the couch.</rdfs:comment>
    </owl:Class>
    


    <!-- http://www.owl-ontologies.com/VirtualHome.owl#thanksgiving -->


    <owl:Class rdf:about="http://www.owl-ontologies.com/VirtualHome.owl#thanksgiving">
        <rdfs:subClassOf rdf:resource="http://www.owl-ontologies.com/VirtualHome.owl#SocialInteraction"/>
        <rdfs:comment>The class with sequence of actions for thanksgiving.</rdfs:comment>
    </owl:Class>
    


    <!-- http://www.owl-ontologies.com/VirtualHome.owl#throw_away_newspaper -->


    <owl:Class rdf:about="http://www.owl-ontologies.com/VirtualHome.owl#throw_away_newspaper">
        <rdfs:subClassOf rdf:resource="http://www.owl-ontologies.com/VirtualHome.owl#Other"/>
        <rdfs:comment>The class with sequence of actions for throwing away newspaper, in the 
garbage can, or elsewhere.</rdfs:comment>
    </owl:Class>
    


    <!-- http://www.owl-ontologies.com/VirtualHome.owl#throw_away_paper -->


    <owl:Class rdf:about="http://www.owl-ontologies.com/VirtualHome.owl#throw_away_paper">
        <rdfs:subClassOf rdf:resource="http://www.owl-ontologies.com/VirtualHome.owl#Other"/>
        <rdfs:comment>The class with sequence of actions for throwing away paper, in the 
garbage that could be in any room.</rdfs:comment>
    </owl:Class>
    


    <!-- http://www.owl-ontologies.com/VirtualHome.owl#throw_shoes -->


    <owl:Class rdf:about="http://www.owl-ontologies.com/VirtualHome.owl#throw_shoes">
        <rdfs:subClassOf rdf:resource="http://www.owl-ontologies.com/VirtualHome.owl#Other"/>
        <rdfs:comment>The class with sequence of actions for throwing away shoes, in any room.</rdfs:comment>
    </owl:Class>
    


    <!-- http://www.owl-ontologies.com/VirtualHome.owl#tidy -->


    <owl:Class rdf:about="http://www.owl-ontologies.com/VirtualHome.owl#tidy">
        <rdfs:subClassOf rdf:resource="http://www.owl-ontologies.com/VirtualHome.owl#Other"/>
        <rdfs:comment>The class with sequence of actions for tiding anything.</rdfs:comment>
    </owl:Class>
    


    <!-- http://www.owl-ontologies.com/VirtualHome.owl#toast_bread -->


    <owl:Class rdf:about="http://www.owl-ontologies.com/VirtualHome.owl#toast_bread">
        <rdfs:subClassOf rdf:resource="http://www.owl-ontologies.com/VirtualHome.owl#FoodPreparation"/>
        <rdfs:comment>The class with sequence of actions for toasting the bread (to prepare a 
toast or something else).</rdfs:comment>
    </owl:Class>
    


    <!-- http://www.owl-ontologies.com/VirtualHome.owl#toilet -->


    <owl:Class rdf:about="http://www.owl-ontologies.com/VirtualHome.owl#toilet">
        <rdfs:subClassOf rdf:resource="http://www.owl-ontologies.com/VirtualHome.owl#HygieneStyling"/>
        <rdfs:comment>The class with sequence of actions for going to the toilet.</rdfs:comment>
    </owl:Class>
    


    <!-- http://www.owl-ontologies.com/VirtualHome.owl#transcribe_what_i_say -->


    <owl:Class rdf:about="http://www.owl-ontologies.com/VirtualHome.owl#transcribe_what_i_say">
        <rdfs:subClassOf rdf:resource="http://www.owl-ontologies.com/VirtualHome.owl#Work"/>
        <rdfs:comment>The class with sequence of actions for trancribe (or copy) the words that I say.</rdfs:comment>
    </owl:Class>
    


    <!-- http://www.owl-ontologies.com/VirtualHome.owl#trick_or_treat -->


    <owl:Class rdf:about="http://www.owl-ontologies.com/VirtualHome.owl#trick_or_treat">
        <rdfs:subClassOf rdf:resource="http://www.owl-ontologies.com/VirtualHome.owl#SocialInteraction"/>
        <rdfs:comment>The class with sequence of actions for trick or treat.</rdfs:comment>
    </owl:Class>
    


    <!-- http://www.owl-ontologies.com/VirtualHome.owl#try_yourself_off -->


    <owl:Class rdf:about="http://www.owl-ontologies.com/VirtualHome.owl#try_yourself_off">
        <rdfs:subClassOf rdf:resource="http://www.owl-ontologies.com/VirtualHome.owl#Other"/>
        <rdfs:comment>The class with sequence of actions for trying yourself off, with any 
activity in any room.</rdfs:comment>
    </owl:Class>
    


    <!-- http://www.owl-ontologies.com/VirtualHome.owl#tuck_kids_in_bed -->


    <owl:Class rdf:about="http://www.owl-ontologies.com/VirtualHome.owl#tuck_kids_in_bed">
        <rdfs:subClassOf rdf:resource="http://www.owl-ontologies.com/VirtualHome.owl#SocialInteraction"/>
        <rdfs:comment>A class with sequences to put the kids in bed for sleep, or tell a story.</rdfs:comment>
    </owl:Class>
    


    <!-- http://www.owl-ontologies.com/VirtualHome.owl#tummy_time -->


    <owl:Class rdf:about="http://www.owl-ontologies.com/VirtualHome.owl#tummy_time">
        <rdfs:subClassOf rdf:resource="http://www.owl-ontologies.com/VirtualHome.owl#Other"/>
        <rdfs:comment>The class with sequence of actions for tummy time.</rdfs:comment>
    </owl:Class>
    


    <!-- http://www.owl-ontologies.com/VirtualHome.owl#turking -->


    <owl:Class rdf:about="http://www.owl-ontologies.com/VirtualHome.owl#turking">
        <rdfs:subClassOf rdf:resource="http://www.owl-ontologies.com/VirtualHome.owl#Other"/>
        <rdfs:comment>The class with sequence of actions for turking.</rdfs:comment>
    </owl:Class>
    


    <!-- http://www.owl-ontologies.com/VirtualHome.owl#turn_light_off -->


    <owl:Class rdf:about="http://www.owl-ontologies.com/VirtualHome.owl#turn_light_off">
        <rdfs:subClassOf rdf:resource="http://www.owl-ontologies.com/VirtualHome.owl#Other"/>
        <rdfs:comment>The class with sequence of actions for  turning off the light form any 
room.</rdfs:comment>
    </owl:Class>
    


    <!-- http://www.owl-ontologies.com/VirtualHome.owl#turn_night_light_on -->


    <owl:Class rdf:about="http://www.owl-ontologies.com/VirtualHome.owl#turn_night_light_on">
        <rdfs:subClassOf rdf:resource="http://www.owl-ontologies.com/VirtualHome.owl#HouseArrangement"/>
        <rdfs:comment>The class with sequence of actions for turning the night light on.</rdfs:comment>
    </owl:Class>
    


    <!-- http://www.owl-ontologies.com/VirtualHome.owl#turn_off_light -->


    <owl:Class rdf:about="http://www.owl-ontologies.com/VirtualHome.owl#turn_off_light">
        <rdfs:subClassOf rdf:resource="http://www.owl-ontologies.com/VirtualHome.owl#HouseArrangement"/>
        <rdfs:comment>The class with sequence of actions for turning off the lights.</rdfs:comment>
    </owl:Class>
    


    <!-- http://www.owl-ontologies.com/VirtualHome.owl#turn_off_tv -->


    <owl:Class rdf:about="http://www.owl-ontologies.com/VirtualHome.owl#turn_off_tv">
        <rdfs:subClassOf rdf:resource="http://www.owl-ontologies.com/VirtualHome.owl#Leisure"/>
        <rdfs:comment>The class with sequence of actions for turning off the TV.</rdfs:comment>
    </owl:Class>
    


    <!-- http://www.owl-ontologies.com/VirtualHome.owl#turn_on_computer -->


    <owl:Class rdf:about="http://www.owl-ontologies.com/VirtualHome.owl#turn_on_computer">
        <rdfs:subClassOf rdf:resource="http://www.owl-ontologies.com/VirtualHome.owl#Other"/>
        <rdfs:comment>The class with sequence of actions for turning on a computer (laptop, or 
personal computer).</rdfs:comment>
    </owl:Class>
    


    <!-- http://www.owl-ontologies.com/VirtualHome.owl#turn_on_light -->


    <owl:Class rdf:about="http://www.owl-ontologies.com/VirtualHome.owl#turn_on_light">
        <rdfs:subClassOf rdf:resource="http://www.owl-ontologies.com/VirtualHome.owl#Other"/>
        <rdfs:comment>A class with sequences on how to turn on the lights from different 
rooms, and different scenaria such as holding other objects or having to 
stand up from bed.</rdfs:comment>
    </owl:Class>
    


    <!-- http://www.owl-ontologies.com/VirtualHome.owl#turn_on_lights -->


    <owl:Class rdf:about="http://www.owl-ontologies.com/VirtualHome.owl#turn_on_lights">
        <rdfs:subClassOf rdf:resource="http://www.owl-ontologies.com/VirtualHome.owl#Other"/>
        <rdfs:comment>The class with sequence of actions for turning on the lights more than 
one.</rdfs:comment>
    </owl:Class>
    


    <!-- http://www.owl-ontologies.com/VirtualHome.owl#turn_on_radio -->


    <owl:Class rdf:about="http://www.owl-ontologies.com/VirtualHome.owl#turn_on_radio">
        <rdfs:subClassOf rdf:resource="http://www.owl-ontologies.com/VirtualHome.owl#Leisure"/>
        <rdfs:comment>The class with sequence of actions for turning on the radio (just 
turning on).
    &lt;/p&gt;</rdfs:comment>
    </owl:Class>
    


    <!-- http://www.owl-ontologies.com/VirtualHome.owl#turn_on_tv -->


    <owl:Class rdf:about="http://www.owl-ontologies.com/VirtualHome.owl#turn_on_tv">
        <rdfs:subClassOf rdf:resource="http://www.owl-ontologies.com/VirtualHome.owl#Leisure"/>
        <rdfs:comment>The class with sequence of actions on hoe to turn on the TV (just turn on tv, not other actions).</rdfs:comment>
    </owl:Class>
    


    <!-- http://www.owl-ontologies.com/VirtualHome.owl#turn_on_tv_with_remote -->


    <owl:Class rdf:about="http://www.owl-ontologies.com/VirtualHome.owl#turn_on_tv_with_remote">
        <rdfs:subClassOf rdf:resource="http://www.owl-ontologies.com/VirtualHome.owl#Leisure"/>
        <rdfs:comment>The class with sequence of actions for watching tv while using remote control.</rdfs:comment>
    </owl:Class>
    


    <!-- http://www.owl-ontologies.com/VirtualHome.owl#type_up_document -->


    <owl:Class rdf:about="http://www.owl-ontologies.com/VirtualHome.owl#type_up_document">
        <rdfs:subClassOf rdf:resource="http://www.owl-ontologies.com/VirtualHome.owl#Work"/>
        <rdfs:comment>The class with sequence of actions for typing up a document.</rdfs:comment>
    </owl:Class>
    


    <!-- http://www.owl-ontologies.com/VirtualHome.owl#unload_dishwasher -->


    <owl:Class rdf:about="http://www.owl-ontologies.com/VirtualHome.owl#unload_dishwasher">
        <rdfs:subClassOf rdf:resource="http://www.owl-ontologies.com/VirtualHome.owl#HouseArrangement"/>
        <rdfs:comment>The class with sequence of actions for unloadinf the dishwasher.</rdfs:comment>
    </owl:Class>
    


    <!-- http://www.owl-ontologies.com/VirtualHome.owl#unload_various_items_from_pockets_and_place_them_in_bowl_on_table -->


    <owl:Class rdf:about="http://www.owl-ontologies.com/VirtualHome.owl#unload_various_items_from_pockets_and_place_them_in_bowl_on_table">
        <rdfs:subClassOf rdf:resource="http://www.owl-ontologies.com/VirtualHome.owl#HouseArrangement"/>
        <rdfs:comment>The class with sequence of actions for unloading various itmes form 
pockets and place them in bowl on table.</rdfs:comment>
    </owl:Class>
    


    <!-- http://www.owl-ontologies.com/VirtualHome.owl#update_address_book -->


    <owl:Class rdf:about="http://www.owl-ontologies.com/VirtualHome.owl#update_address_book">
        <rdfs:subClassOf rdf:resource="http://www.owl-ontologies.com/VirtualHome.owl#Work"/>
        <rdfs:comment>The class with sequence of actions that are neede to update your address 
book.</rdfs:comment>
    </owl:Class>
    


    <!-- http://www.owl-ontologies.com/VirtualHome.owl#use_bathroom -->


    <owl:Class rdf:about="http://www.owl-ontologies.com/VirtualHome.owl#use_bathroom">
        <rdfs:subClassOf rdf:resource="http://www.owl-ontologies.com/VirtualHome.owl#HygieneStyling"/>
        <rdfs:comment>The class with sequence of actions for using the bathroom, the whole 
room.</rdfs:comment>
    </owl:Class>
    


    <!-- http://www.owl-ontologies.com/VirtualHome.owl#use_computer -->


    <owl:Class rdf:about="http://www.owl-ontologies.com/VirtualHome.owl#use_computer">
        <rdfs:subClassOf rdf:resource="http://www.owl-ontologies.com/VirtualHome.owl#Work"/>
        <rdfs:comment>Class wih sequences on how to perform general task with a computer.</rdfs:comment>
    </owl:Class>
    


    <!-- http://www.owl-ontologies.com/VirtualHome.owl#use_laptop -->


    <owl:Class rdf:about="http://www.owl-ontologies.com/VirtualHome.owl#use_laptop">
        <rdfs:subClassOf rdf:resource="http://www.owl-ontologies.com/VirtualHome.owl#Other"/>
        <rdfs:comment>The class with sequence of actions for using your laptop, variety of 
functions.</rdfs:comment>
    </owl:Class>
    


    <!-- http://www.owl-ontologies.com/VirtualHome.owl#use_restroom -->


    <owl:Class rdf:about="http://www.owl-ontologies.com/VirtualHome.owl#use_restroom">
        <rdfs:subClassOf rdf:resource="http://www.owl-ontologies.com/VirtualHome.owl#HygieneStyling"/>
        <rdfs:comment>The class with sequence of actions for using the restroom.</rdfs:comment>
    </owl:Class>
    


    <!-- http://www.owl-ontologies.com/VirtualHome.owl#use_smartphone -->


    <owl:Class rdf:about="http://www.owl-ontologies.com/VirtualHome.owl#use_smartphone">
        <rdfs:subClassOf rdf:resource="http://www.owl-ontologies.com/VirtualHome.owl#Leisure"/>
    </owl:Class>
    


    <!-- http://www.owl-ontologies.com/VirtualHome.owl#use_toilet -->


    <owl:Class rdf:about="http://www.owl-ontologies.com/VirtualHome.owl#use_toilet">
        <rdfs:subClassOf rdf:resource="http://www.owl-ontologies.com/VirtualHome.owl#HygieneStyling"/>
        <rdfs:comment>The class with sequence of actions for using the toilet.</rdfs:comment>
    </owl:Class>
    


    <!-- http://www.owl-ontologies.com/VirtualHome.owl#vacuum_carpet -->


    <owl:Class rdf:about="http://www.owl-ontologies.com/VirtualHome.owl#vacuum_carpet">
        <rdfs:subClassOf rdf:resource="http://www.owl-ontologies.com/VirtualHome.owl#HouseCleaning"/>
        <rdfs:comment>The class with sequence of actions for vacuum the carpet.</rdfs:comment>
    </owl:Class>
    


    <!-- http://www.owl-ontologies.com/VirtualHome.owl#visit -->


    <owl:Class rdf:about="http://www.owl-ontologies.com/VirtualHome.owl#visit">
        <rdfs:subClassOf rdf:resource="http://www.owl-ontologies.com/VirtualHome.owl#SocialInteraction"/>
        <rdfs:comment>The class with sequence of actions for visitng someone elses house.</rdfs:comment>
    </owl:Class>
    


    <!-- http://www.owl-ontologies.com/VirtualHome.owl#visit_neighbors -->


    <owl:Class rdf:about="http://www.owl-ontologies.com/VirtualHome.owl#visit_neighbors">
        <rdfs:subClassOf rdf:resource="http://www.owl-ontologies.com/VirtualHome.owl#SocialInteraction"/>
        <rdfs:comment>The class with sequence of actions for visitng neighbors.</rdfs:comment>
    </owl:Class>
    


    <!-- http://www.owl-ontologies.com/VirtualHome.owl#visit_with_friends_while_engaging_in_games -->


    <owl:Class rdf:about="http://www.owl-ontologies.com/VirtualHome.owl#visit_with_friends_while_engaging_in_games">
        <rdfs:subClassOf rdf:resource="http://www.owl-ontologies.com/VirtualHome.owl#Other"/>
        <rdfs:comment>The class with sequence of actions for visiting friends while engaging in games.</rdfs:comment>
    </owl:Class>
    


    <!-- http://www.owl-ontologies.com/VirtualHome.owl#wake_kids_up -->


    <owl:Class rdf:about="http://www.owl-ontologies.com/VirtualHome.owl#wake_kids_up">
        <rdfs:subClassOf rdf:resource="http://www.owl-ontologies.com/VirtualHome.owl#SocialInteraction"/>
        <rdfs:comment>The class with sequence of actions for waking kids up from sleep.</rdfs:comment>
    </owl:Class>
    


    <!-- http://www.owl-ontologies.com/VirtualHome.owl#wake_me_up -->


    <owl:Class rdf:about="http://www.owl-ontologies.com/VirtualHome.owl#wake_me_up">
        <rdfs:subClassOf rdf:resource="http://www.owl-ontologies.com/VirtualHome.owl#BedTimeSleep"/>
        <rdfs:comment>The class with sequence of actions for telling the system to wake up the user.</rdfs:comment>
    </owl:Class>
    


    <!-- http://www.owl-ontologies.com/VirtualHome.owl#walk_through -->


    <owl:Class rdf:about="http://www.owl-ontologies.com/VirtualHome.owl#walk_through">
        <rdfs:subClassOf rdf:resource="http://www.owl-ontologies.com/VirtualHome.owl#Other"/>
        <rdfs:comment>The class with sequence of actions for walking through a door.</rdfs:comment>
    </owl:Class>
    


    <!-- http://www.owl-ontologies.com/VirtualHome.owl#walk_to_room -->


    <owl:Class rdf:about="http://www.owl-ontologies.com/VirtualHome.owl#walk_to_room">
        <rdfs:subClassOf rdf:resource="http://www.owl-ontologies.com/VirtualHome.owl#Other"/>
        <rdfs:comment>The class with sequence of actions for walking to room, any room.</rdfs:comment>
    </owl:Class>
    


    <!-- http://www.owl-ontologies.com/VirtualHome.owl#wash_and_clean_all_crystal_in_china_cabinet -->


    <owl:Class rdf:about="http://www.owl-ontologies.com/VirtualHome.owl#wash_and_clean_all_crystal_in_china_cabinet">
        <rdfs:subClassOf rdf:resource="http://www.owl-ontologies.com/VirtualHome.owl#HouseArrangement"/>
        <rdfs:comment>The class with sequence of actions for washing and cleaning all crystal 
in china cabinet.</rdfs:comment>
    </owl:Class>
    


    <!-- http://www.owl-ontologies.com/VirtualHome.owl#wash_back -->


    <owl:Class rdf:about="http://www.owl-ontologies.com/VirtualHome.owl#wash_back">
        <rdfs:subClassOf rdf:resource="http://www.owl-ontologies.com/VirtualHome.owl#Other"/>
        <rdfs:comment>The class with sequence of actions for washing back, your own or others 
back.</rdfs:comment>
    </owl:Class>
    


    <!-- http://www.owl-ontologies.com/VirtualHome.owl#wash_clothes -->


    <owl:Class rdf:about="http://www.owl-ontologies.com/VirtualHome.owl#wash_clothes">
        <rdfs:subClassOf rdf:resource="http://www.owl-ontologies.com/VirtualHome.owl#HouseArrangement"/>
        <rdfs:subClassOf rdf:resource="http://www.owl-ontologies.com/VirtualHome.owl#HouseCleaning"/>
        <rdfs:comment>Class with sequences for washing clothes.</rdfs:comment>
    </owl:Class>
    


    <!-- http://www.owl-ontologies.com/VirtualHome.owl#wash_dining_table -->


    <owl:Class rdf:about="http://www.owl-ontologies.com/VirtualHome.owl#wash_dining_table">
        <rdfs:subClassOf rdf:resource="http://www.owl-ontologies.com/VirtualHome.owl#Other"/>
        <rdfs:comment>The class with sequence of actions for washing dining table.</rdfs:comment>
    </owl:Class>
    


    <!-- http://www.owl-ontologies.com/VirtualHome.owl#wash_dirty_dishes -->


    <owl:Class rdf:about="http://www.owl-ontologies.com/VirtualHome.owl#wash_dirty_dishes">
        <rdfs:subClassOf rdf:resource="http://www.owl-ontologies.com/VirtualHome.owl#HouseCleaning"/>
        <rdfs:comment>The class with sequence of actions for washing dirty dishes.</rdfs:comment>
    </owl:Class>
    


    <!-- http://www.owl-ontologies.com/VirtualHome.owl#wash_dishes -->


    <owl:Class rdf:about="http://www.owl-ontologies.com/VirtualHome.owl#wash_dishes">
        <rdfs:subClassOf rdf:resource="http://www.owl-ontologies.com/VirtualHome.owl#HouseArrangement"/>
        <rdfs:comment>The class with sequence of actions for washing up dishes, in the general case or getting ready to wash dishes.</rdfs:comment>
    </owl:Class>
    


    <!-- http://www.owl-ontologies.com/VirtualHome.owl#wash_dishes_by_hand -->


    <owl:Class rdf:about="http://www.owl-ontologies.com/VirtualHome.owl#wash_dishes_by_hand">
        <rdfs:subClassOf rdf:resource="http://www.owl-ontologies.com/VirtualHome.owl#HouseArrangement"/>
        <rdfs:comment>The class with sequence of actions for washing yp dishes by hand only.</rdfs:comment>
    </owl:Class>
    


    <!-- http://www.owl-ontologies.com/VirtualHome.owl#wash_dishes_with_dishwasher -->


    <owl:Class rdf:about="http://www.owl-ontologies.com/VirtualHome.owl#wash_dishes_with_dishwasher">
        <rdfs:subClassOf rdf:resource="http://www.owl-ontologies.com/VirtualHome.owl#HouseArrangement"/>
        <rdfs:comment>The class with sequence of actions for washing up dishes with dishwasher.</rdfs:comment>
    </owl:Class>
    


    <!-- http://www.owl-ontologies.com/VirtualHome.owl#wash_face -->


    <owl:Class rdf:about="http://www.owl-ontologies.com/VirtualHome.owl#wash_face">
        <rdfs:subClassOf rdf:resource="http://www.owl-ontologies.com/VirtualHome.owl#HygieneStyling"/>
        <rdfs:comment>The class with sequence of actions for washing your face.</rdfs:comment>
    </owl:Class>
    


    <!-- http://www.owl-ontologies.com/VirtualHome.owl#wash_hair -->


    <owl:Class rdf:about="http://www.owl-ontologies.com/VirtualHome.owl#wash_hair">
        <rdfs:subClassOf rdf:resource="http://www.owl-ontologies.com/VirtualHome.owl#HygieneStyling"/>
        <rdfs:comment>The class with sequence of actions for washing your hair.</rdfs:comment>
    </owl:Class>
    


    <!-- http://www.owl-ontologies.com/VirtualHome.owl#wash_hands -->


    <owl:Class rdf:about="http://www.owl-ontologies.com/VirtualHome.owl#wash_hands">
        <rdfs:subClassOf rdf:resource="http://www.owl-ontologies.com/VirtualHome.owl#HygieneStyling"/>
        <rdfs:comment>The class with sequence of actions for washing your hands.</rdfs:comment>
    </owl:Class>
    


    <!-- http://www.owl-ontologies.com/VirtualHome.owl#wash_monitor -->


    <owl:Class rdf:about="http://www.owl-ontologies.com/VirtualHome.owl#wash_monitor">
        <rdfs:subClassOf rdf:resource="http://www.owl-ontologies.com/VirtualHome.owl#HouseCleaning"/>
        <rdfs:comment>The class with sequence of actions for washing a some kind of monitor.</rdfs:comment>
    </owl:Class>
    


    <!-- http://www.owl-ontologies.com/VirtualHome.owl#wash_pillow -->


    <owl:Class rdf:about="http://www.owl-ontologies.com/VirtualHome.owl#wash_pillow">
        <rdfs:subClassOf rdf:resource="http://www.owl-ontologies.com/VirtualHome.owl#HouseCleaning"/>
    </owl:Class>
    


    <!-- http://www.owl-ontologies.com/VirtualHome.owl#wash_sink -->


    <owl:Class rdf:about="http://www.owl-ontologies.com/VirtualHome.owl#wash_sink">
        <rdfs:subClassOf rdf:resource="http://www.owl-ontologies.com/VirtualHome.owl#HouseCleaning"/>
        <rdfs:comment>The class with sequence of actions for house cleaning.</rdfs:comment>
    </owl:Class>
    


    <!-- http://www.owl-ontologies.com/VirtualHome.owl#wash_table -->


    <owl:Class rdf:about="http://www.owl-ontologies.com/VirtualHome.owl#wash_table">
        <rdfs:subClassOf rdf:resource="http://www.owl-ontologies.com/VirtualHome.owl#HouseCleaning"/>
        <rdfs:comment>The class with sequence of actions for washing the table.</rdfs:comment>
    </owl:Class>
    


    <!-- http://www.owl-ontologies.com/VirtualHome.owl#wash_teeth -->


    <owl:Class rdf:about="http://www.owl-ontologies.com/VirtualHome.owl#wash_teeth">
        <rdfs:subClassOf rdf:resource="http://www.owl-ontologies.com/VirtualHome.owl#HygieneStyling"/>
        <rdfs:comment>The class with sequence of actions for washing teeth (with water for example).</rdfs:comment>
    </owl:Class>
    


    <!-- http://www.owl-ontologies.com/VirtualHome.owl#watch__horror__movie -->


    <owl:Class rdf:about="http://www.owl-ontologies.com/VirtualHome.owl#watch__horror__movie">
        <rdfs:subClassOf rdf:resource="http://www.owl-ontologies.com/VirtualHome.owl#Leisure"/>
        <rdfs:comment>The class with sequence of actions for watching a horror movie 
specifically.</rdfs:comment>
    </owl:Class>
    


    <!-- http://www.owl-ontologies.com/VirtualHome.owl#watch_fly -->


    <owl:Class rdf:about="http://www.owl-ontologies.com/VirtualHome.owl#watch_fly">
        <rdfs:subClassOf rdf:resource="http://www.owl-ontologies.com/VirtualHome.owl#Other"/>
        <rdfs:comment>The class with sequence of actions for watching a fly that has entered a 
room.</rdfs:comment>
    </owl:Class>
    


    <!-- http://www.owl-ontologies.com/VirtualHome.owl#watch_movie -->


    <owl:Class rdf:about="http://www.owl-ontologies.com/VirtualHome.owl#watch_movie">
        <rdfs:subClassOf rdf:resource="http://www.owl-ontologies.com/VirtualHome.owl#Leisure"/>
        <rdfs:comment>A class about how to watch a movie either on the TV or laptop.</rdfs:comment>
    </owl:Class>
    


    <!-- http://www.owl-ontologies.com/VirtualHome.owl#watch_tv -->


    <owl:Class rdf:about="http://www.owl-ontologies.com/VirtualHome.owl#watch_tv">
        <rdfs:subClassOf rdf:resource="http://www.owl-ontologies.com/VirtualHome.owl#Leisure"/>
        <rdfs:comment>It contains some subclasses on how to watch TV</rdfs:comment>
    </owl:Class>
    


    <!-- http://www.owl-ontologies.com/VirtualHome.owl#watch_youtube -->


    <owl:Class rdf:about="http://www.owl-ontologies.com/VirtualHome.owl#watch_youtube">
        <rdfs:subClassOf rdf:resource="http://www.owl-ontologies.com/VirtualHome.owl#Leisure"/>
        <rdfs:comment>The class with sequence of actions for wathcing YouTube videos.</rdfs:comment>
    </owl:Class>
    


    <!-- http://www.owl-ontologies.com/VirtualHome.owl#water_plants -->


    <owl:Class rdf:about="http://www.owl-ontologies.com/VirtualHome.owl#water_plants">
        <rdfs:subClassOf rdf:resource="http://www.owl-ontologies.com/VirtualHome.owl#HouseArrangement"/>
        <rdfs:comment>The class with sequence of actions for watering the plants.</rdfs:comment>
    </owl:Class>
    


    <!-- http://www.owl-ontologies.com/VirtualHome.owl#wave_at_people_walking_by_through_window -->


    <owl:Class rdf:about="http://www.owl-ontologies.com/VirtualHome.owl#wave_at_people_walking_by_through_window">
        <rdfs:subClassOf rdf:resource="http://www.owl-ontologies.com/VirtualHome.owl#SocialInteraction"/>
        <rdfs:comment>The class with sequence of actions for waving at people walking by 
through window.</rdfs:comment>
    </owl:Class>
    


    <!-- http://www.owl-ontologies.com/VirtualHome.owl#whine -->


    <owl:Class rdf:about="http://www.owl-ontologies.com/VirtualHome.owl#whine">
        <rdfs:subClassOf rdf:resource="http://www.owl-ontologies.com/VirtualHome.owl#Other"/>
        <rdfs:comment>The class with sequence of actions for whining in any room.</rdfs:comment>
    </owl:Class>
    


    <!-- http://www.owl-ontologies.com/VirtualHome.owl#wipe_down_baseboards_please -->


    <owl:Class rdf:about="http://www.owl-ontologies.com/VirtualHome.owl#wipe_down_baseboards_please">
        <rdfs:subClassOf rdf:resource="http://www.owl-ontologies.com/VirtualHome.owl#Other"/>
        <rdfs:comment>The class with sequence of actions for wipe down baseboards please.</rdfs:comment>
    </owl:Class>
    


    <!-- http://www.owl-ontologies.com/VirtualHome.owl#wipe_down_counter -->


    <owl:Class rdf:about="http://www.owl-ontologies.com/VirtualHome.owl#wipe_down_counter">
        <rdfs:subClassOf rdf:resource="http://www.owl-ontologies.com/VirtualHome.owl#Other"/>
        <rdfs:comment>The class with sequence of actions for wiping down counter, for any domestic machine that has such.</rdfs:comment>
    </owl:Class>
    


    <!-- http://www.owl-ontologies.com/VirtualHome.owl#wipe_down_sink -->


    <owl:Class rdf:about="http://www.owl-ontologies.com/VirtualHome.owl#wipe_down_sink">
        <rdfs:subClassOf rdf:resource="http://www.owl-ontologies.com/VirtualHome.owl#HouseCleaning"/>
        <rdfs:comment>The class with sequence of actions in order to wipe down sink, only this 
part of cleaning not all the cleaning procedure.</rdfs:comment>
    </owl:Class>
    


    <!-- http://www.owl-ontologies.com/VirtualHome.owl#wipe_feet -->


    <owl:Class rdf:about="http://www.owl-ontologies.com/VirtualHome.owl#wipe_feet">
        <rdfs:subClassOf rdf:resource="http://www.owl-ontologies.com/VirtualHome.owl#HygieneStyling"/>
        <rdfs:comment>The class with sequence of actions for wiping your own feet.</rdfs:comment>
    </owl:Class>
    


    <!-- http://www.owl-ontologies.com/VirtualHome.owl#wipe_off_shoes -->


    <owl:Class rdf:about="http://www.owl-ontologies.com/VirtualHome.owl#wipe_off_shoes">
        <rdfs:subClassOf rdf:resource="http://www.owl-ontologies.com/VirtualHome.owl#Other"/>
        <rdfs:comment>The class with sequence of actions for wiping your shoes off.</rdfs:comment>
    </owl:Class>
    


    <!-- http://www.owl-ontologies.com/VirtualHome.owl#wipe_room_down_with_lysol -->


    <owl:Class rdf:about="http://www.owl-ontologies.com/VirtualHome.owl#wipe_room_down_with_lysol">
        <rdfs:subClassOf rdf:resource="http://www.owl-ontologies.com/VirtualHome.owl#HouseCleaning"/>
        <rdfs:comment>The class with sequence of actions for wiping down the room with lysol.</rdfs:comment>
    </owl:Class>
    


    <!-- http://www.owl-ontologies.com/VirtualHome.owl#workout -->


    <owl:Class rdf:about="http://www.owl-ontologies.com/VirtualHome.owl#workout">
        <rdfs:subClassOf rdf:resource="http://www.owl-ontologies.com/VirtualHome.owl#PhysicalActivity"/>
        <rdfs:comment>A class with soft physical activity, or exercise, such as weight 
lifting, workout.</rdfs:comment>
    </owl:Class>
    


    <!-- http://www.owl-ontologies.com/VirtualHome.owl#write_an_email -->


    <owl:Class rdf:about="http://www.owl-ontologies.com/VirtualHome.owl#write_an_email">
        <rdfs:subClassOf rdf:resource="http://www.owl-ontologies.com/VirtualHome.owl#Work"/>
        <rdfs:comment>The class with sequence of actions for wrtiting ana email.</rdfs:comment>
    </owl:Class>
    


    <!-- http://www.owl-ontologies.com/VirtualHome.owl#write_book -->


    <owl:Class rdf:about="http://www.owl-ontologies.com/VirtualHome.owl#write_book">
        <rdfs:subClassOf rdf:resource="http://www.owl-ontologies.com/VirtualHome.owl#Other"/>
        <rdfs:comment>The class with sequence of actions for writing a book, in any room.</rdfs:comment>
    </owl:Class>
    


    <!-- http://www.owl-ontologies.com/VirtualHome.owl#write_in_your_diary -->


    <owl:Class rdf:about="http://www.owl-ontologies.com/VirtualHome.owl#write_in_your_diary">
        <rdfs:subClassOf rdf:resource="http://www.owl-ontologies.com/VirtualHome.owl#Other"/>
        <rdfs:comment>The class with sequence of actions for writing in your diary, in any 
room.</rdfs:comment>
    </owl:Class>
    


    <!-- http://www.owl-ontologies.com/VirtualHome.owl#write_letter -->


    <owl:Class rdf:about="http://www.owl-ontologies.com/VirtualHome.owl#write_letter">
        <rdfs:subClassOf rdf:resource="http://www.owl-ontologies.com/VirtualHome.owl#Work"/>
        <rdfs:comment>Class with sequences on how to write a letter.</rdfs:comment>
    </owl:Class>
    


    <!-- http://www.owl-ontologies.com/VirtualHome.owl#write_report -->


    <owl:Class rdf:about="http://www.owl-ontologies.com/VirtualHome.owl#write_report">
        <rdfs:subClassOf rdf:resource="http://www.owl-ontologies.com/VirtualHome.owl#Work"/>
        <rdfs:comment>The class with sequence of actions for writing some kind of report.</rdfs:comment>
    </owl:Class>
    


    <!-- http://www.owl-ontologies.com/VirtualHome.owl#write_research_paper -->


    <owl:Class rdf:about="http://www.owl-ontologies.com/VirtualHome.owl#write_research_paper">
        <rdfs:subClassOf rdf:resource="http://www.owl-ontologies.com/VirtualHome.owl#Work"/>
        <rdfs:comment>The class with sequence of actions for writing a research paper.</rdfs:comment>
    </owl:Class>
    


    <!-- http://www.owl-ontologies.com/VirtualHome.owl#write_research_papers -->


    <owl:Class rdf:about="http://www.owl-ontologies.com/VirtualHome.owl#write_research_papers">
        <rdfs:subClassOf rdf:resource="http://www.owl-ontologies.com/VirtualHome.owl#Work"/>
        <rdfs:comment>The class with sequence of actions for writing reaseach papers (only 
research paper).</rdfs:comment>
    </owl:Class>
    


    <!-- http://www.owl-ontologies.com/VirtualHome.owl#write_school_paper -->


    <owl:Class rdf:about="http://www.owl-ontologies.com/VirtualHome.owl#write_school_paper">
        <rdfs:subClassOf rdf:resource="http://www.owl-ontologies.com/VirtualHome.owl#Work"/>
        <rdfs:comment>The class with sequence of actions writing school papers, it should not 
be confused with research paper.</rdfs:comment>
    </owl:Class>
    


    <!-- http://www.owl-ontologies.com/VirtualHome.owl#write_story -->


    <owl:Class rdf:about="http://www.owl-ontologies.com/VirtualHome.owl#write_story">
        <rdfs:subClassOf rdf:resource="http://www.owl-ontologies.com/VirtualHome.owl#Other"/>
        <rdfs:comment>The class with sequence of actions for writing a story, on the computer 
or on paper.</rdfs:comment>
    </owl:Class>
    


    <!-- http://www.owl-ontologies.com/VirtualHome.owl#write_thank_you_notes -->


    <owl:Class rdf:about="http://www.owl-ontologies.com/VirtualHome.owl#write_thank_you_notes">
        <rdfs:subClassOf rdf:resource="http://www.owl-ontologies.com/VirtualHome.owl#Work"/>
        <rdfs:comment>The class with sequence of actions to write a thank you note to somebody.</rdfs:comment>
    </owl:Class>
    


    <!-- http://www.owl-ontologies.com/VirtualHome.owl#yoga -->


    <owl:Class rdf:about="http://www.owl-ontologies.com/VirtualHome.owl#yoga">
        <rdfs:subClassOf rdf:resource="http://www.owl-ontologies.com/VirtualHome.owl#PhysicalActivity"/>
        <rdfs:comment>The class with sequence of actions for doing yoga.</rdfs:comment>
    </owl:Class>
    


    <!-- http://www.w3.org/2006/time#Duration -->


    <owl:Class rdf:about="http://www.w3.org/2006/time#Duration">
        <rdfs:subClassOf rdf:resource="http://www.w3.org/2006/time#TemporalDuration"/>
    </owl:Class>
    


    <!-- http://www.w3.org/2006/time#TemporalDuration -->


    <owl:Class rdf:about="http://www.w3.org/2006/time#TemporalDuration"/>
    


    <!-- http://www.w3.org/2006/time#TemporalEntity -->


    <owl:Class rdf:about="http://www.w3.org/2006/time#TemporalEntity"/>
    


    <!-- http://www.w3.org/2006/time#TemporalUnit -->


    <owl:Class rdf:about="http://www.w3.org/2006/time#TemporalUnit"/>
    


    <!-- https://www.web3d.org/specifications/X3dOntology4.0#SFDouble -->


    <owl:Class rdf:about="https://www.web3d.org/specifications/X3dOntology4.0#SFDouble">
        <rdfs:subClassOf rdf:resource="https://www.web3d.org/specifications/X3dOntology4.0#X3DField"/>
    </owl:Class>
    


    <!-- https://www.web3d.org/specifications/X3dOntology4.0#SFVec3f -->


    <owl:Class rdf:about="https://www.web3d.org/specifications/X3dOntology4.0#SFVec3f">
        <rdfs:subClassOf rdf:resource="https://www.web3d.org/specifications/X3dOntology4.0#X3DField"/>
    </owl:Class>
    


    <!-- https://www.web3d.org/specifications/X3dOntology4.0#Shape -->


    <owl:Class rdf:about="https://www.web3d.org/specifications/X3dOntology4.0#Shape">
        <rdfs:comment>used for 3D bounding box</rdfs:comment>
    </owl:Class>
    <owl:Axiom>
        <owl:annotatedSource rdf:resource="https://www.web3d.org/specifications/X3dOntology4.0#Shape"/>
        <owl:annotatedProperty rdf:resource="http://www.w3.org/2000/01/rdf-schema#comment"/>
        <owl:annotatedTarget>used for 3D bounding box</owl:annotatedTarget>
        <rdfs:comment>commented by vh2kg_ontology</rdfs:comment>
    </owl:Axiom>
    


    <!-- https://www.web3d.org/specifications/X3dOntology4.0#X3DField -->


    <owl:Class rdf:about="https://www.web3d.org/specifications/X3dOntology4.0#X3DField">
        <rdfs:comment>X3DField is the abstract field type from which all single-valued field types are derived.</rdfs:comment>
    </owl:Class>
    


    <!-- 
    ///////////////////////////////////////////////////////////////////////////////////////
    //
    // Individuals
    //
    ///////////////////////////////////////////////////////////////////////////////////////
     -->


    


    <!-- http://example.org/virtualhome2kg/ontology/BROKEN -->


    <owl:NamedIndividual rdf:about="http://example.org/virtualhome2kg/ontology/BROKEN">
        <rdf:type rdf:resource="http://example.org/virtualhome2kg/ontology/StateType"/>
    </owl:NamedIndividual>
    


    <!-- http://example.org/virtualhome2kg/ontology/BURNING -->


    <owl:NamedIndividual rdf:about="http://example.org/virtualhome2kg/ontology/BURNING">
        <rdf:type rdf:resource="http://example.org/virtualhome2kg/ontology/StateType"/>
    </owl:NamedIndividual>
    


    <!-- http://example.org/virtualhome2kg/ontology/CLEAN -->


    <owl:NamedIndividual rdf:about="http://example.org/virtualhome2kg/ontology/CLEAN">
        <rdf:type rdf:resource="http://example.org/virtualhome2kg/ontology/StateType"/>
    </owl:NamedIndividual>
    


    <!-- http://example.org/virtualhome2kg/ontology/CLOSED -->


    <owl:NamedIndividual rdf:about="http://example.org/virtualhome2kg/ontology/CLOSED">
        <rdf:type rdf:resource="http://example.org/virtualhome2kg/ontology/StateType"/>
    </owl:NamedIndividual>
    


    <!-- http://example.org/virtualhome2kg/ontology/COOKED -->


    <owl:NamedIndividual rdf:about="http://example.org/virtualhome2kg/ontology/COOKED">
        <rdf:type rdf:resource="http://example.org/virtualhome2kg/ontology/StateType"/>
    </owl:NamedIndividual>
    


    <!-- http://example.org/virtualhome2kg/ontology/DIRTY -->


    <owl:NamedIndividual rdf:about="http://example.org/virtualhome2kg/ontology/DIRTY">
        <rdf:type rdf:resource="http://example.org/virtualhome2kg/ontology/StateType"/>
    </owl:NamedIndividual>
    


    <!-- http://example.org/virtualhome2kg/ontology/DONE -->


    <owl:NamedIndividual rdf:about="http://example.org/virtualhome2kg/ontology/DONE">
        <rdf:type rdf:resource="http://example.org/virtualhome2kg/ontology/StateType"/>
    </owl:NamedIndividual>
    


    <!-- http://example.org/virtualhome2kg/ontology/DRUNK -->


    <owl:NamedIndividual rdf:about="http://example.org/virtualhome2kg/ontology/DRUNK">
        <rdf:type rdf:resource="http://example.org/virtualhome2kg/ontology/StateType"/>
    </owl:NamedIndividual>
    


    <!-- http://example.org/virtualhome2kg/ontology/DRY -->


    <owl:NamedIndividual rdf:about="http://example.org/virtualhome2kg/ontology/DRY">
        <rdf:type rdf:resource="http://example.org/virtualhome2kg/ontology/StateType"/>
    </owl:NamedIndividual>
    


    <!-- http://example.org/virtualhome2kg/ontology/EMPTY -->


    <owl:NamedIndividual rdf:about="http://example.org/virtualhome2kg/ontology/EMPTY">
        <rdf:type rdf:resource="http://example.org/virtualhome2kg/ontology/StateType"/>
    </owl:NamedIndividual>
    


    <!-- http://example.org/virtualhome2kg/ontology/FLUSHED -->


    <owl:NamedIndividual rdf:about="http://example.org/virtualhome2kg/ontology/FLUSHED">
        <rdf:type rdf:resource="http://example.org/virtualhome2kg/ontology/StateType"/>
    </owl:NamedIndividual>
    


    <!-- http://example.org/virtualhome2kg/ontology/FOLDED -->


    <owl:NamedIndividual rdf:about="http://example.org/virtualhome2kg/ontology/FOLDED">
        <rdf:type rdf:resource="http://example.org/virtualhome2kg/ontology/StateType"/>
    </owl:NamedIndividual>
    


    <!-- http://example.org/virtualhome2kg/ontology/FROZEN -->


    <owl:NamedIndividual rdf:about="http://example.org/virtualhome2kg/ontology/FROZEN">
        <rdf:type rdf:resource="http://example.org/virtualhome2kg/ontology/StateType"/>
    </owl:NamedIndividual>
    


    <!-- http://example.org/virtualhome2kg/ontology/FULL -->


    <owl:NamedIndividual rdf:about="http://example.org/virtualhome2kg/ontology/FULL">
        <rdf:type rdf:resource="http://example.org/virtualhome2kg/ontology/StateType"/>
    </owl:NamedIndividual>
    


    <!-- http://example.org/virtualhome2kg/ontology/HANGED -->


    <owl:NamedIndividual rdf:about="http://example.org/virtualhome2kg/ontology/HANGED">
        <rdf:type rdf:resource="http://example.org/virtualhome2kg/ontology/StateType"/>
    </owl:NamedIndividual>
    


    <!-- http://example.org/virtualhome2kg/ontology/HURT -->


    <owl:NamedIndividual rdf:about="http://example.org/virtualhome2kg/ontology/HURT">
        <rdf:type rdf:resource="http://example.org/virtualhome2kg/ontology/StateType"/>
    </owl:NamedIndividual>
    


    <!-- http://example.org/virtualhome2kg/ontology/LYING -->


    <owl:NamedIndividual rdf:about="http://example.org/virtualhome2kg/ontology/LYING">
        <rdf:type rdf:resource="http://example.org/virtualhome2kg/ontology/StateType"/>
    </owl:NamedIndividual>
    


    <!-- http://example.org/virtualhome2kg/ontology/MELTED -->


    <owl:NamedIndividual rdf:about="http://example.org/virtualhome2kg/ontology/MELTED">
        <rdf:type rdf:resource="http://example.org/virtualhome2kg/ontology/StateType"/>
    </owl:NamedIndividual>
    


    <!-- http://example.org/virtualhome2kg/ontology/OCCUPIED -->


    <owl:NamedIndividual rdf:about="http://example.org/virtualhome2kg/ontology/OCCUPIED">
        <rdf:type rdf:resource="http://example.org/virtualhome2kg/ontology/StateType"/>
    </owl:NamedIndividual>
    


    <!-- http://example.org/virtualhome2kg/ontology/OFF -->


    <owl:NamedIndividual rdf:about="http://example.org/virtualhome2kg/ontology/OFF">
        <rdf:type rdf:resource="http://example.org/virtualhome2kg/ontology/StateType"/>
    </owl:NamedIndividual>
    


    <!-- http://example.org/virtualhome2kg/ontology/ON -->


    <owl:NamedIndividual rdf:about="http://example.org/virtualhome2kg/ontology/ON">
        <rdf:type rdf:resource="http://example.org/virtualhome2kg/ontology/StateType"/>
    </owl:NamedIndividual>
    


    <!-- http://example.org/virtualhome2kg/ontology/OPEN -->


    <owl:NamedIndividual rdf:about="http://example.org/virtualhome2kg/ontology/OPEN">
        <rdf:type rdf:resource="http://example.org/virtualhome2kg/ontology/StateType"/>
    </owl:NamedIndividual>
    


    <!-- http://example.org/virtualhome2kg/ontology/PEELED -->


    <owl:NamedIndividual rdf:about="http://example.org/virtualhome2kg/ontology/PEELED">
        <rdf:type rdf:resource="http://example.org/virtualhome2kg/ontology/StateType"/>
    </owl:NamedIndividual>
    


    <!-- http://example.org/virtualhome2kg/ontology/PERSON -->


    <owl:NamedIndividual rdf:about="http://example.org/virtualhome2kg/ontology/PERSON">
        <rdf:type rdf:resource="http://example.org/virtualhome2kg/ontology/Attribute"/>
    </owl:NamedIndividual>
    


    <!-- http://example.org/virtualhome2kg/ontology/PLUGGED_IN -->


    <owl:NamedIndividual rdf:about="http://example.org/virtualhome2kg/ontology/PLUGGED_IN">
        <rdf:type rdf:resource="http://example.org/virtualhome2kg/ontology/StateType"/>
    </owl:NamedIndividual>
    


    <!-- http://example.org/virtualhome2kg/ontology/PLUGGED_OUT -->


    <owl:NamedIndividual rdf:about="http://example.org/virtualhome2kg/ontology/PLUGGED_OUT">
        <rdf:type rdf:resource="http://example.org/virtualhome2kg/ontology/StateType"/>
    </owl:NamedIndividual>
    


    <!-- http://example.org/virtualhome2kg/ontology/ROTTEN -->


    <owl:NamedIndividual rdf:about="http://example.org/virtualhome2kg/ontology/ROTTEN">
        <rdf:type rdf:resource="http://example.org/virtualhome2kg/ontology/StateType"/>
    </owl:NamedIndividual>
    


    <!-- http://example.org/virtualhome2kg/ontology/SHARPENED -->


    <owl:NamedIndividual rdf:about="http://example.org/virtualhome2kg/ontology/SHARPENED">
        <rdf:type rdf:resource="http://example.org/virtualhome2kg/ontology/StateType"/>
    </owl:NamedIndividual>
    


    <!-- http://example.org/virtualhome2kg/ontology/SHAVED -->


    <owl:NamedIndividual rdf:about="http://example.org/virtualhome2kg/ontology/SHAVED">
        <rdf:type rdf:resource="http://example.org/virtualhome2kg/ontology/StateType"/>
    </owl:NamedIndividual>
    


    <!-- http://example.org/virtualhome2kg/ontology/SITTING -->


    <owl:NamedIndividual rdf:about="http://example.org/virtualhome2kg/ontology/SITTING">
        <rdf:type rdf:resource="http://example.org/virtualhome2kg/ontology/StateType"/>
    </owl:NamedIndividual>
    


    <!-- http://example.org/virtualhome2kg/ontology/SLICED -->


    <owl:NamedIndividual rdf:about="http://example.org/virtualhome2kg/ontology/SLICED">
        <rdf:type rdf:resource="http://example.org/virtualhome2kg/ontology/StateType"/>
    </owl:NamedIndividual>
    


    <!-- http://example.org/virtualhome2kg/ontology/SQUEEZED -->


    <owl:NamedIndividual rdf:about="http://example.org/virtualhome2kg/ontology/SQUEEZED">
        <rdf:type rdf:resource="http://example.org/virtualhome2kg/ontology/StateType"/>
    </owl:NamedIndividual>
    


    <!-- http://example.org/virtualhome2kg/ontology/UNDONE -->


    <owl:NamedIndividual rdf:about="http://example.org/virtualhome2kg/ontology/UNDONE">
        <rdf:type rdf:resource="http://example.org/virtualhome2kg/ontology/StateType"/>
    </owl:NamedIndividual>
    


    <!-- http://example.org/virtualhome2kg/ontology/WET -->


    <owl:NamedIndividual rdf:about="http://example.org/virtualhome2kg/ontology/WET">
        <rdf:type rdf:resource="http://example.org/virtualhome2kg/ontology/StateType"/>
    </owl:NamedIndividual>
    


    <!-- http://example.org/virtualhome2kg/ontology/bright -->


    <owl:NamedIndividual rdf:about="http://example.org/virtualhome2kg/ontology/bright">
        <rdf:type rdf:resource="http://example.org/virtualhome2kg/ontology/Attribute"/>
    </owl:NamedIndividual>
    


    <!-- http://example.org/virtualhome2kg/ontology/clothes -->


    <owl:NamedIndividual rdf:about="http://example.org/virtualhome2kg/ontology/clothes">
        <rdf:type rdf:resource="http://example.org/virtualhome2kg/ontology/Attribute"/>
    </owl:NamedIndividual>
    


    <!-- http://example.org/virtualhome2kg/ontology/cold -->


    <owl:NamedIndividual rdf:about="http://example.org/virtualhome2kg/ontology/cold">
        <rdf:type rdf:resource="http://example.org/virtualhome2kg/ontology/Attribute"/>
    </owl:NamedIndividual>
    


    <!-- http://example.org/virtualhome2kg/ontology/containers -->


    <owl:NamedIndividual rdf:about="http://example.org/virtualhome2kg/ontology/containers">
        <rdf:type rdf:resource="http://example.org/virtualhome2kg/ontology/Attribute"/>
    </owl:NamedIndividual>
    


    <!-- http://example.org/virtualhome2kg/ontology/cover_object -->


    <owl:NamedIndividual rdf:about="http://example.org/virtualhome2kg/ontology/cover_object">
        <rdf:type rdf:resource="http://example.org/virtualhome2kg/ontology/Attribute"/>
    </owl:NamedIndividual>
    


    <!-- http://example.org/virtualhome2kg/ontology/cream -->


    <owl:NamedIndividual rdf:about="http://example.org/virtualhome2kg/ontology/cream">
        <rdf:type rdf:resource="http://example.org/virtualhome2kg/ontology/Attribute"/>
    </owl:NamedIndividual>
    


    <!-- http://example.org/virtualhome2kg/ontology/dark -->


    <owl:NamedIndividual rdf:about="http://example.org/virtualhome2kg/ontology/dark">
        <rdf:type rdf:resource="http://example.org/virtualhome2kg/ontology/Attribute"/>
    </owl:NamedIndividual>
    


    <!-- http://example.org/virtualhome2kg/ontology/deep -->


    <owl:NamedIndividual rdf:about="http://example.org/virtualhome2kg/ontology/deep">
        <rdf:type rdf:resource="http://example.org/virtualhome2kg/ontology/Attribute"/>
    </owl:NamedIndividual>
    


    <!-- http://example.org/virtualhome2kg/ontology/has_paper -->


    <owl:NamedIndividual rdf:about="http://example.org/virtualhome2kg/ontology/has_paper">
        <rdf:type rdf:resource="http://example.org/virtualhome2kg/ontology/Attribute"/>
    </owl:NamedIndividual>
    


    <!-- http://example.org/virtualhome2kg/ontology/has_plug -->


    <owl:NamedIndividual rdf:about="http://example.org/virtualhome2kg/ontology/has_plug">
        <rdf:type rdf:resource="http://example.org/virtualhome2kg/ontology/Attribute"/>
    </owl:NamedIndividual>
    


    <!-- http://example.org/virtualhome2kg/ontology/has_surface -->


    <owl:NamedIndividual rdf:about="http://example.org/virtualhome2kg/ontology/has_surface">
        <rdf:type rdf:resource="http://example.org/virtualhome2kg/ontology/Attribute"/>
    </owl:NamedIndividual>
    


    <!-- http://example.org/virtualhome2kg/ontology/has_switch -->


    <owl:NamedIndividual rdf:about="http://example.org/virtualhome2kg/ontology/has_switch">
        <rdf:type rdf:resource="http://example.org/virtualhome2kg/ontology/Attribute"/>
    </owl:NamedIndividual>
    


    <!-- http://example.org/virtualhome2kg/ontology/heavy -->


    <owl:NamedIndividual rdf:about="http://example.org/virtualhome2kg/ontology/heavy">
        <rdf:type rdf:resource="http://example.org/virtualhome2kg/ontology/Attribute"/>
    </owl:NamedIndividual>
    


    <!-- http://example.org/virtualhome2kg/ontology/high -->


    <owl:NamedIndividual rdf:about="http://example.org/virtualhome2kg/ontology/high">
        <rdf:type rdf:resource="http://example.org/virtualhome2kg/ontology/Attribute"/>
    </owl:NamedIndividual>
    


    <!-- http://example.org/virtualhome2kg/ontology/hot -->


    <owl:NamedIndividual rdf:about="http://example.org/virtualhome2kg/ontology/hot">
        <rdf:type rdf:resource="http://example.org/virtualhome2kg/ontology/Attribute"/>
    </owl:NamedIndividual>
    


    <!-- http://example.org/virtualhome2kg/ontology/jumpUp -->


    <owl:NamedIndividual rdf:about="http://example.org/virtualhome2kg/ontology/jumpUp">
        <rdf:type rdf:resource="http://example.org/virtualhome2kg/ontology/Action"/>
    </owl:NamedIndividual>
    


    <!-- http://example.org/virtualhome2kg/ontology/kg -->


    <owl:NamedIndividual rdf:about="http://example.org/virtualhome2kg/ontology/kg">
        <rdf:type rdf:resource="http://example.org/virtualhome2kg/ontology/Unit"/>
    </owl:NamedIndividual>
    


    <!-- http://example.org/virtualhome2kg/ontology/light -->


    <owl:NamedIndividual rdf:about="http://example.org/virtualhome2kg/ontology/light">
        <rdf:type rdf:resource="http://example.org/virtualhome2kg/ontology/Attribute"/>
    </owl:NamedIndividual>
    


    <!-- http://example.org/virtualhome2kg/ontology/long -->


    <owl:NamedIndividual rdf:about="http://example.org/virtualhome2kg/ontology/long">
        <rdf:type rdf:resource="http://example.org/virtualhome2kg/ontology/Attribute"/>
    </owl:NamedIndividual>
    


    <!-- http://example.org/virtualhome2kg/ontology/low -->


    <owl:NamedIndividual rdf:about="http://example.org/virtualhome2kg/ontology/low">
        <rdf:type rdf:resource="http://example.org/virtualhome2kg/ontology/Attribute"/>
    </owl:NamedIndividual>
    


    <!-- http://example.org/virtualhome2kg/ontology/meter -->


    <owl:NamedIndividual rdf:about="http://example.org/virtualhome2kg/ontology/meter">
        <rdf:type rdf:resource="http://example.org/virtualhome2kg/ontology/Unit"/>
    </owl:NamedIndividual>
    


    <!-- http://example.org/virtualhome2kg/ontology/recipient -->


    <owl:NamedIndividual rdf:about="http://example.org/virtualhome2kg/ontology/recipient">
        <rdf:type rdf:resource="http://example.org/virtualhome2kg/ontology/Attribute"/>
    </owl:NamedIndividual>
    


    <!-- http://example.org/virtualhome2kg/ontology/shallow -->


    <owl:NamedIndividual rdf:about="http://example.org/virtualhome2kg/ontology/shallow">
        <rdf:type rdf:resource="http://example.org/virtualhome2kg/ontology/Attribute"/>
    </owl:NamedIndividual>
    


    <!-- http://example.org/virtualhome2kg/ontology/short -->


    <owl:NamedIndividual rdf:about="http://example.org/virtualhome2kg/ontology/short">
        <rdf:type rdf:resource="http://example.org/virtualhome2kg/ontology/Attribute"/>
    </owl:NamedIndividual>
    


    <!-- http://example.org/virtualhome2kg/ontology/thick -->


    <owl:NamedIndividual rdf:about="http://example.org/virtualhome2kg/ontology/thick">
        <rdf:type rdf:resource="http://example.org/virtualhome2kg/ontology/Attribute"/>
    </owl:NamedIndividual>
    


    <!-- http://example.org/virtualhome2kg/ontology/thin -->


    <owl:NamedIndividual rdf:about="http://example.org/virtualhome2kg/ontology/thin">
        <rdf:type rdf:resource="http://example.org/virtualhome2kg/ontology/Attribute"/>
    </owl:NamedIndividual>
    


    <!-- http://example.org/virtualhome2kg/ontology/action/bend -->


    <owl:NamedIndividual rdf:about="http://example.org/virtualhome2kg/ontology/action/bend">
        <rdf:type rdf:resource="http://example.org/virtualhome2kg/ontology/Action"/>
    </owl:NamedIndividual>
    


    <!-- http://example.org/virtualhome2kg/ontology/action/break -->


    <owl:NamedIndividual rdf:about="http://example.org/virtualhome2kg/ontology/action/break">
        <rdf:type rdf:resource="http://example.org/virtualhome2kg/ontology/Action"/>
    </owl:NamedIndividual>
    


    <!-- http://example.org/virtualhome2kg/ontology/action/breatheIn -->


    <owl:NamedIndividual rdf:about="http://example.org/virtualhome2kg/ontology/action/breatheIn">
        <rdf:type rdf:resource="http://example.org/virtualhome2kg/ontology/Action"/>
    </owl:NamedIndividual>
    


    <!-- http://example.org/virtualhome2kg/ontology/action/breatheOut -->


    <owl:NamedIndividual rdf:about="http://example.org/virtualhome2kg/ontology/action/breatheOut">
        <rdf:type rdf:resource="http://example.org/virtualhome2kg/ontology/Action"/>
    </owl:NamedIndividual>
    


    <!-- http://example.org/virtualhome2kg/ontology/action/brush -->


    <owl:NamedIndividual rdf:about="http://example.org/virtualhome2kg/ontology/action/brush">
        <rdf:type rdf:resource="http://example.org/virtualhome2kg/ontology/Action"/>
    </owl:NamedIndividual>
    


    <!-- http://example.org/virtualhome2kg/ontology/action/call -->


    <owl:NamedIndividual rdf:about="http://example.org/virtualhome2kg/ontology/action/call">
        <rdf:type rdf:resource="http://example.org/virtualhome2kg/ontology/Action"/>
    </owl:NamedIndividual>
    


    <!-- http://example.org/virtualhome2kg/ontology/action/carry -->


    <owl:NamedIndividual rdf:about="http://example.org/virtualhome2kg/ontology/action/carry">
        <rdf:type rdf:resource="http://example.org/virtualhome2kg/ontology/Action"/>
    </owl:NamedIndividual>
    


    <!-- http://example.org/virtualhome2kg/ontology/action/climb -->


    <owl:NamedIndividual rdf:about="http://example.org/virtualhome2kg/ontology/action/climb">
        <rdf:type rdf:resource="http://example.org/virtualhome2kg/ontology/Action"/>
    </owl:NamedIndividual>
    


    <!-- http://example.org/virtualhome2kg/ontology/action/climbDown -->


    <owl:NamedIndividual rdf:about="http://example.org/virtualhome2kg/ontology/action/climbDown">
        <rdf:type rdf:resource="http://example.org/virtualhome2kg/ontology/Action"/>
    </owl:NamedIndividual>
    


    <!-- http://example.org/virtualhome2kg/ontology/action/close -->


    <owl:NamedIndividual rdf:about="http://example.org/virtualhome2kg/ontology/action/close">
        <rdf:type rdf:resource="http://example.org/virtualhome2kg/ontology/Action"/>
    </owl:NamedIndividual>
    


    <!-- http://example.org/virtualhome2kg/ontology/action/cover -->


    <owl:NamedIndividual rdf:about="http://example.org/virtualhome2kg/ontology/action/cover">
        <rdf:type rdf:resource="http://example.org/virtualhome2kg/ontology/Action"/>
    </owl:NamedIndividual>
    


    <!-- http://example.org/virtualhome2kg/ontology/action/crawl -->


    <owl:NamedIndividual rdf:about="http://example.org/virtualhome2kg/ontology/action/crawl">
        <rdf:type rdf:resource="http://example.org/virtualhome2kg/ontology/Action"/>
    </owl:NamedIndividual>
    


    <!-- http://example.org/virtualhome2kg/ontology/action/cut -->


    <owl:NamedIndividual rdf:about="http://example.org/virtualhome2kg/ontology/action/cut">
        <rdf:type rdf:resource="http://example.org/virtualhome2kg/ontology/Action"/>
    </owl:NamedIndividual>
    


    <!-- http://example.org/virtualhome2kg/ontology/action/dance -->


    <owl:NamedIndividual rdf:about="http://example.org/virtualhome2kg/ontology/action/dance">
        <rdf:type rdf:resource="http://example.org/virtualhome2kg/ontology/Action"/>
    </owl:NamedIndividual>
    


    <!-- http://example.org/virtualhome2kg/ontology/action/dial -->


    <owl:NamedIndividual rdf:about="http://example.org/virtualhome2kg/ontology/action/dial">
        <rdf:type rdf:resource="http://example.org/virtualhome2kg/ontology/Action"/>
    </owl:NamedIndividual>
    


    <!-- http://example.org/virtualhome2kg/ontology/action/dive -->


    <owl:NamedIndividual rdf:about="http://example.org/virtualhome2kg/ontology/action/dive">
        <rdf:type rdf:resource="http://example.org/virtualhome2kg/ontology/Action"/>
    </owl:NamedIndividual>
    


    <!-- http://example.org/virtualhome2kg/ontology/action/drink -->


    <owl:NamedIndividual rdf:about="http://example.org/virtualhome2kg/ontology/action/drink">
        <rdf:type rdf:resource="http://example.org/virtualhome2kg/ontology/Action"/>
    </owl:NamedIndividual>
    


    <!-- http://example.org/virtualhome2kg/ontology/action/drop -->


    <owl:NamedIndividual rdf:about="http://example.org/virtualhome2kg/ontology/action/drop">
        <rdf:type rdf:resource="http://example.org/virtualhome2kg/ontology/Action"/>
    </owl:NamedIndividual>
    


    <!-- http://example.org/virtualhome2kg/ontology/action/eat -->


    <owl:NamedIndividual rdf:about="http://example.org/virtualhome2kg/ontology/action/eat">
        <rdf:type rdf:resource="http://example.org/virtualhome2kg/ontology/Action"/>
    </owl:NamedIndividual>
    


    <!-- http://example.org/virtualhome2kg/ontology/action/enter -->


    <owl:NamedIndividual rdf:about="http://example.org/virtualhome2kg/ontology/action/enter">
        <rdf:type rdf:resource="http://example.org/virtualhome2kg/ontology/Action"/>
    </owl:NamedIndividual>
    


    <!-- http://example.org/virtualhome2kg/ontology/action/excrete -->


    <owl:NamedIndividual rdf:about="http://example.org/virtualhome2kg/ontology/action/excrete">
        <rdf:type rdf:resource="http://example.org/virtualhome2kg/ontology/Action"/>
    </owl:NamedIndividual>
    


    <!-- http://example.org/virtualhome2kg/ontology/action/find -->


    <owl:NamedIndividual rdf:about="http://example.org/virtualhome2kg/ontology/action/find">
        <rdf:type rdf:resource="http://example.org/virtualhome2kg/ontology/Action"/>
    </owl:NamedIndividual>
    


    <!-- http://example.org/virtualhome2kg/ontology/action/flush -->


    <owl:NamedIndividual rdf:about="http://example.org/virtualhome2kg/ontology/action/flush">
        <rdf:type rdf:resource="http://example.org/virtualhome2kg/ontology/Action"/>
    </owl:NamedIndividual>
    


    <!-- http://example.org/virtualhome2kg/ontology/action/fold -->


    <owl:NamedIndividual rdf:about="http://example.org/virtualhome2kg/ontology/action/fold">
        <rdf:type rdf:resource="http://example.org/virtualhome2kg/ontology/Action"/>
    </owl:NamedIndividual>
    


    <!-- http://example.org/virtualhome2kg/ontology/action/gargle -->


    <owl:NamedIndividual rdf:about="http://example.org/virtualhome2kg/ontology/action/gargle">
        <rdf:type rdf:resource="http://example.org/virtualhome2kg/ontology/Action"/>
    </owl:NamedIndividual>
    


    <!-- http://example.org/virtualhome2kg/ontology/action/grab -->


    <owl:NamedIndividual rdf:about="http://example.org/virtualhome2kg/ontology/action/grab">
        <rdf:type rdf:resource="http://example.org/virtualhome2kg/ontology/Action"/>
    </owl:NamedIndividual>
    


    <!-- http://example.org/virtualhome2kg/ontology/action/greet -->


    <owl:NamedIndividual rdf:about="http://example.org/virtualhome2kg/ontology/action/greet">
        <rdf:type rdf:resource="http://example.org/virtualhome2kg/ontology/Action"/>
    </owl:NamedIndividual>
    


    <!-- http://example.org/virtualhome2kg/ontology/action/hang -->


    <owl:NamedIndividual rdf:about="http://example.org/virtualhome2kg/ontology/action/hang">
        <rdf:type rdf:resource="http://example.org/virtualhome2kg/ontology/Action"/>
    </owl:NamedIndividual>
    


    <!-- http://example.org/virtualhome2kg/ontology/action/hit -->


    <owl:NamedIndividual rdf:about="http://example.org/virtualhome2kg/ontology/action/hit">
        <rdf:type rdf:resource="http://example.org/virtualhome2kg/ontology/Action"/>
    </owl:NamedIndividual>
    


    <!-- http://example.org/virtualhome2kg/ontology/action/insert -->


    <owl:NamedIndividual rdf:about="http://example.org/virtualhome2kg/ontology/action/insert">
        <rdf:type rdf:resource="http://example.org/virtualhome2kg/ontology/Action"/>
    </owl:NamedIndividual>
    


    <!-- http://example.org/virtualhome2kg/ontology/action/jump -->


    <owl:NamedIndividual rdf:about="http://example.org/virtualhome2kg/ontology/action/jump">
        <rdf:type rdf:resource="http://example.org/virtualhome2kg/ontology/Action"/>
    </owl:NamedIndividual>
    


    <!-- http://example.org/virtualhome2kg/ontology/action/kneel -->


    <owl:NamedIndividual rdf:about="http://example.org/virtualhome2kg/ontology/action/kneel">
        <rdf:type rdf:resource="http://example.org/virtualhome2kg/ontology/Action"/>
    </owl:NamedIndividual>
    


    <!-- http://example.org/virtualhome2kg/ontology/action/laugh -->


    <owl:NamedIndividual rdf:about="http://example.org/virtualhome2kg/ontology/action/laugh">
        <rdf:type rdf:resource="http://example.org/virtualhome2kg/ontology/Action"/>
    </owl:NamedIndividual>
    


    <!-- http://example.org/virtualhome2kg/ontology/action/leave -->


    <owl:NamedIndividual rdf:about="http://example.org/virtualhome2kg/ontology/action/leave">
        <rdf:type rdf:resource="http://example.org/virtualhome2kg/ontology/Action"/>
    </owl:NamedIndividual>
    


    <!-- http://example.org/virtualhome2kg/ontology/action/lie -->


    <owl:NamedIndividual rdf:about="http://example.org/virtualhome2kg/ontology/action/lie">
        <rdf:type rdf:resource="http://example.org/virtualhome2kg/ontology/Action"/>
    </owl:NamedIndividual>
    


    <!-- http://example.org/virtualhome2kg/ontology/action/lift -->


    <owl:NamedIndividual rdf:about="http://example.org/virtualhome2kg/ontology/action/lift">
        <rdf:type rdf:resource="http://example.org/virtualhome2kg/ontology/Action"/>
    </owl:NamedIndividual>
    


    <!-- http://example.org/virtualhome2kg/ontology/action/listen -->


    <owl:NamedIndividual rdf:about="http://example.org/virtualhome2kg/ontology/action/listen">
        <rdf:type rdf:resource="http://example.org/virtualhome2kg/ontology/Action"/>
    </owl:NamedIndividual>
    


    <!-- http://example.org/virtualhome2kg/ontology/action/lookAt -->


    <owl:NamedIndividual rdf:about="http://example.org/virtualhome2kg/ontology/action/lookAt">
        <rdf:type rdf:resource="http://example.org/virtualhome2kg/ontology/Action"/>
    </owl:NamedIndividual>
    


    <!-- http://example.org/virtualhome2kg/ontology/action/maintain -->


    <owl:NamedIndividual rdf:about="http://example.org/virtualhome2kg/ontology/action/maintain">
        <rdf:type rdf:resource="http://example.org/virtualhome2kg/ontology/Action"/>
    </owl:NamedIndividual>
    


    <!-- http://example.org/virtualhome2kg/ontology/action/move -->


    <owl:NamedIndividual rdf:about="http://example.org/virtualhome2kg/ontology/action/move">
        <rdf:type rdf:resource="http://example.org/virtualhome2kg/ontology/Action"/>
    </owl:NamedIndividual>
    


    <!-- http://example.org/virtualhome2kg/ontology/action/open -->


    <owl:NamedIndividual rdf:about="http://example.org/virtualhome2kg/ontology/action/open">
        <rdf:type rdf:resource="http://example.org/virtualhome2kg/ontology/Action"/>
    </owl:NamedIndividual>
    


    <!-- http://example.org/virtualhome2kg/ontology/action/pickUp -->


    <owl:NamedIndividual rdf:about="http://example.org/virtualhome2kg/ontology/action/pickUp">
        <rdf:type rdf:resource="http://example.org/virtualhome2kg/ontology/Action"/>
    </owl:NamedIndividual>
    


    <!-- http://example.org/virtualhome2kg/ontology/action/plugIn -->


    <owl:NamedIndividual rdf:about="http://example.org/virtualhome2kg/ontology/action/plugIn">
        <rdf:type rdf:resource="http://example.org/virtualhome2kg/ontology/Action"/>
    </owl:NamedIndividual>
    


    <!-- http://example.org/virtualhome2kg/ontology/action/plugOut -->


    <owl:NamedIndividual rdf:about="http://example.org/virtualhome2kg/ontology/action/plugOut">
        <rdf:type rdf:resource="http://example.org/virtualhome2kg/ontology/Action"/>
    </owl:NamedIndividual>
    


    <!-- http://example.org/virtualhome2kg/ontology/action/pointAt -->


    <owl:NamedIndividual rdf:about="http://example.org/virtualhome2kg/ontology/action/pointAt">
        <rdf:type rdf:resource="http://example.org/virtualhome2kg/ontology/Action"/>
    </owl:NamedIndividual>
    


    <!-- http://example.org/virtualhome2kg/ontology/action/pour -->


    <owl:NamedIndividual rdf:about="http://example.org/virtualhome2kg/ontology/action/pour">
        <rdf:type rdf:resource="http://example.org/virtualhome2kg/ontology/Action"/>
    </owl:NamedIndividual>
    


    <!-- http://example.org/virtualhome2kg/ontology/action/pull -->


    <owl:NamedIndividual rdf:about="http://example.org/virtualhome2kg/ontology/action/pull">
        <rdf:type rdf:resource="http://example.org/virtualhome2kg/ontology/Action"/>
    </owl:NamedIndividual>
    


    <!-- http://example.org/virtualhome2kg/ontology/action/pullOut -->


    <owl:NamedIndividual rdf:about="http://example.org/virtualhome2kg/ontology/action/pullOut">
        <rdf:type rdf:resource="http://example.org/virtualhome2kg/ontology/Action"/>
    </owl:NamedIndividual>
    


    <!-- http://example.org/virtualhome2kg/ontology/action/push -->


    <owl:NamedIndividual rdf:about="http://example.org/virtualhome2kg/ontology/action/push">
        <rdf:type rdf:resource="http://example.org/virtualhome2kg/ontology/Action"/>
    </owl:NamedIndividual>
    


    <!-- http://example.org/virtualhome2kg/ontology/action/put -->


    <owl:NamedIndividual rdf:about="http://example.org/virtualhome2kg/ontology/action/put">
        <rdf:type rdf:resource="http://example.org/virtualhome2kg/ontology/Action"/>
    </owl:NamedIndividual>
    


    <!-- http://example.org/virtualhome2kg/ontology/action/putIn -->


    <owl:NamedIndividual rdf:about="http://example.org/virtualhome2kg/ontology/action/putIn">
        <rdf:type rdf:resource="http://example.org/virtualhome2kg/ontology/Action"/>
    </owl:NamedIndividual>
    


    <!-- http://example.org/virtualhome2kg/ontology/action/putOn -->


    <owl:NamedIndividual rdf:about="http://example.org/virtualhome2kg/ontology/action/putOn">
        <rdf:type rdf:resource="http://example.org/virtualhome2kg/ontology/Action"/>
    </owl:NamedIndividual>
    


    <!-- http://example.org/virtualhome2kg/ontology/action/reach -->


    <owl:NamedIndividual rdf:about="http://example.org/virtualhome2kg/ontology/action/reach">
        <rdf:type rdf:resource="http://example.org/virtualhome2kg/ontology/Action"/>
    </owl:NamedIndividual>
    


    <!-- http://example.org/virtualhome2kg/ontology/action/rinse -->


    <owl:NamedIndividual rdf:about="http://example.org/virtualhome2kg/ontology/action/rinse">
        <rdf:type rdf:resource="http://example.org/virtualhome2kg/ontology/Action"/>
    </owl:NamedIndividual>
    


    <!-- http://example.org/virtualhome2kg/ontology/action/run -->


    <owl:NamedIndividual rdf:about="http://example.org/virtualhome2kg/ontology/action/run">
        <rdf:type rdf:resource="http://example.org/virtualhome2kg/ontology/Action"/>
    </owl:NamedIndividual>
    


    <!-- http://example.org/virtualhome2kg/ontology/action/scrub -->


    <owl:NamedIndividual rdf:about="http://example.org/virtualhome2kg/ontology/action/scrub">
        <rdf:type rdf:resource="http://example.org/virtualhome2kg/ontology/Action"/>
    </owl:NamedIndividual>
    


    <!-- http://example.org/virtualhome2kg/ontology/action/sew -->


    <owl:NamedIndividual rdf:about="http://example.org/virtualhome2kg/ontology/action/sew">
        <rdf:type rdf:resource="http://example.org/virtualhome2kg/ontology/Action"/>
    </owl:NamedIndividual>
    


    <!-- http://example.org/virtualhome2kg/ontology/action/shake -->


    <owl:NamedIndividual rdf:about="http://example.org/virtualhome2kg/ontology/action/shake">
        <rdf:type rdf:resource="http://example.org/virtualhome2kg/ontology/Action"/>
    </owl:NamedIndividual>
    


    <!-- http://example.org/virtualhome2kg/ontology/action/sing -->


    <owl:NamedIndividual rdf:about="http://example.org/virtualhome2kg/ontology/action/sing">
        <rdf:type rdf:resource="http://example.org/virtualhome2kg/ontology/Action"/>
    </owl:NamedIndividual>
    


    <!-- http://example.org/virtualhome2kg/ontology/action/sit -->


    <owl:NamedIndividual rdf:about="http://example.org/virtualhome2kg/ontology/action/sit">
        <rdf:type rdf:resource="http://example.org/virtualhome2kg/ontology/Action"/>
    </owl:NamedIndividual>
    


    <!-- http://example.org/virtualhome2kg/ontology/action/sleep -->


    <owl:NamedIndividual rdf:about="http://example.org/virtualhome2kg/ontology/action/sleep">
        <rdf:type rdf:resource="http://example.org/virtualhome2kg/ontology/Action"/>
    </owl:NamedIndividual>
    


    <!-- http://example.org/virtualhome2kg/ontology/action/smell -->


    <owl:NamedIndividual rdf:about="http://example.org/virtualhome2kg/ontology/action/smell">
        <rdf:type rdf:resource="http://example.org/virtualhome2kg/ontology/Action"/>
    </owl:NamedIndividual>
    


    <!-- http://example.org/virtualhome2kg/ontology/action/soak -->


    <owl:NamedIndividual rdf:about="http://example.org/virtualhome2kg/ontology/action/soak">
        <rdf:type rdf:resource="http://example.org/virtualhome2kg/ontology/Action"/>
    </owl:NamedIndividual>
    


    <!-- http://example.org/virtualhome2kg/ontology/action/speak -->


    <owl:NamedIndividual rdf:about="http://example.org/virtualhome2kg/ontology/action/speak">
        <rdf:type rdf:resource="http://example.org/virtualhome2kg/ontology/Action"/>
    </owl:NamedIndividual>
    


    <!-- http://example.org/virtualhome2kg/ontology/action/spit -->


    <owl:NamedIndividual rdf:about="http://example.org/virtualhome2kg/ontology/action/spit">
        <rdf:type rdf:resource="http://example.org/virtualhome2kg/ontology/Action"/>
    </owl:NamedIndividual>
    


    <!-- http://example.org/virtualhome2kg/ontology/action/spread -->


    <owl:NamedIndividual rdf:about="http://example.org/virtualhome2kg/ontology/action/spread">
        <rdf:type rdf:resource="http://example.org/virtualhome2kg/ontology/Action"/>
    </owl:NamedIndividual>
    


    <!-- http://example.org/virtualhome2kg/ontology/action/squat -->


    <owl:NamedIndividual rdf:about="http://example.org/virtualhome2kg/ontology/action/squat">
        <rdf:type rdf:resource="http://example.org/virtualhome2kg/ontology/Action"/>
    </owl:NamedIndividual>
    


    <!-- http://example.org/virtualhome2kg/ontology/action/squeeze -->


    <owl:NamedIndividual rdf:about="http://example.org/virtualhome2kg/ontology/action/squeeze">
        <rdf:type rdf:resource="http://example.org/virtualhome2kg/ontology/Action"/>
    </owl:NamedIndividual>
    


    <!-- http://example.org/virtualhome2kg/ontology/action/stand -->


    <owl:NamedIndividual rdf:about="http://example.org/virtualhome2kg/ontology/action/stand">
        <rdf:type rdf:resource="http://example.org/virtualhome2kg/ontology/Action"/>
    </owl:NamedIndividual>
    


    <!-- http://example.org/virtualhome2kg/ontology/action/standUp -->


    <owl:NamedIndividual rdf:about="http://example.org/virtualhome2kg/ontology/action/standUp">
        <rdf:type rdf:resource="http://example.org/virtualhome2kg/ontology/Action"/>
    </owl:NamedIndividual>
    


    <!-- http://example.org/virtualhome2kg/ontology/action/stir -->


    <owl:NamedIndividual rdf:about="http://example.org/virtualhome2kg/ontology/action/stir">
        <rdf:type rdf:resource="http://example.org/virtualhome2kg/ontology/Action"/>
    </owl:NamedIndividual>
    


    <!-- http://example.org/virtualhome2kg/ontology/action/straddle -->


    <owl:NamedIndividual rdf:about="http://example.org/virtualhome2kg/ontology/action/straddle">
        <rdf:type rdf:resource="http://example.org/virtualhome2kg/ontology/Action"/>
    </owl:NamedIndividual>
    


    <!-- http://example.org/virtualhome2kg/ontology/action/stretch -->


    <owl:NamedIndividual rdf:about="http://example.org/virtualhome2kg/ontology/action/stretch">
        <rdf:type rdf:resource="http://example.org/virtualhome2kg/ontology/Action"/>
    </owl:NamedIndividual>
    


    <!-- http://example.org/virtualhome2kg/ontology/action/strideOver -->


    <owl:NamedIndividual rdf:about="http://example.org/virtualhome2kg/ontology/action/strideOver">
        <rdf:type rdf:resource="http://example.org/virtualhome2kg/ontology/Action"/>
    </owl:NamedIndividual>
    


    <!-- http://example.org/virtualhome2kg/ontology/action/sweep -->


    <owl:NamedIndividual rdf:about="http://example.org/virtualhome2kg/ontology/action/sweep">
        <rdf:type rdf:resource="http://example.org/virtualhome2kg/ontology/Action"/>
    </owl:NamedIndividual>
    


    <!-- http://example.org/virtualhome2kg/ontology/action/swing -->


    <owl:NamedIndividual rdf:about="http://example.org/virtualhome2kg/ontology/action/swing">
        <rdf:type rdf:resource="http://example.org/virtualhome2kg/ontology/Action"/>
    </owl:NamedIndividual>
    


    <!-- http://example.org/virtualhome2kg/ontology/action/switchOff -->


    <owl:NamedIndividual rdf:about="http://example.org/virtualhome2kg/ontology/action/switchOff">
        <rdf:type rdf:resource="http://example.org/virtualhome2kg/ontology/Action"/>
    </owl:NamedIndividual>
    


    <!-- http://example.org/virtualhome2kg/ontology/action/switchOn -->


    <owl:NamedIndividual rdf:about="http://example.org/virtualhome2kg/ontology/action/switchOn">
        <rdf:type rdf:resource="http://example.org/virtualhome2kg/ontology/Action"/>
    </owl:NamedIndividual>
    


    <!-- http://example.org/virtualhome2kg/ontology/action/takeOff -->


    <owl:NamedIndividual rdf:about="http://example.org/virtualhome2kg/ontology/action/takeOff">
        <rdf:type rdf:resource="http://example.org/virtualhome2kg/ontology/Action"/>
    </owl:NamedIndividual>
    


    <!-- http://example.org/virtualhome2kg/ontology/action/talk -->


    <owl:NamedIndividual rdf:about="http://example.org/virtualhome2kg/ontology/action/talk">
        <rdf:type rdf:resource="http://example.org/virtualhome2kg/ontology/Action"/>
    </owl:NamedIndividual>
    


    <!-- http://example.org/virtualhome2kg/ontology/action/taste -->


    <owl:NamedIndividual rdf:about="http://example.org/virtualhome2kg/ontology/action/taste">
        <rdf:type rdf:resource="http://example.org/virtualhome2kg/ontology/Action"/>
    </owl:NamedIndividual>
    


    <!-- http://example.org/virtualhome2kg/ontology/action/throw -->


    <owl:NamedIndividual rdf:about="http://example.org/virtualhome2kg/ontology/action/throw">
        <rdf:type rdf:resource="http://example.org/virtualhome2kg/ontology/Action"/>
    </owl:NamedIndividual>
    


    <!-- http://example.org/virtualhome2kg/ontology/action/tie -->


    <owl:NamedIndividual rdf:about="http://example.org/virtualhome2kg/ontology/action/tie">
        <rdf:type rdf:resource="http://example.org/virtualhome2kg/ontology/Action"/>
    </owl:NamedIndividual>
    


    <!-- http://example.org/virtualhome2kg/ontology/action/touch -->


    <owl:NamedIndividual rdf:about="http://example.org/virtualhome2kg/ontology/action/touch">
        <rdf:type rdf:resource="http://example.org/virtualhome2kg/ontology/Action"/>
    </owl:NamedIndividual>
    


    <!-- http://example.org/virtualhome2kg/ontology/action/turnTo -->


    <owl:NamedIndividual rdf:about="http://example.org/virtualhome2kg/ontology/action/turnTo">
        <rdf:type rdf:resource="http://example.org/virtualhome2kg/ontology/Action"/>
    </owl:NamedIndividual>
    


    <!-- http://example.org/virtualhome2kg/ontology/action/twist -->


    <owl:NamedIndividual rdf:about="http://example.org/virtualhome2kg/ontology/action/twist">
        <rdf:type rdf:resource="http://example.org/virtualhome2kg/ontology/Action"/>
    </owl:NamedIndividual>
    


    <!-- http://example.org/virtualhome2kg/ontology/action/type -->


    <owl:NamedIndividual rdf:about="http://example.org/virtualhome2kg/ontology/action/type">
        <rdf:type rdf:resource="http://example.org/virtualhome2kg/ontology/Action"/>
    </owl:NamedIndividual>
    


    <!-- http://example.org/virtualhome2kg/ontology/action/uncover -->


    <owl:NamedIndividual rdf:about="http://example.org/virtualhome2kg/ontology/action/uncover">
        <rdf:type rdf:resource="http://example.org/virtualhome2kg/ontology/Action"/>
    </owl:NamedIndividual>
    


    <!-- http://example.org/virtualhome2kg/ontology/action/unfold -->


    <owl:NamedIndividual rdf:about="http://example.org/virtualhome2kg/ontology/action/unfold">
        <rdf:type rdf:resource="http://example.org/virtualhome2kg/ontology/Action"/>
    </owl:NamedIndividual>
    


    <!-- http://example.org/virtualhome2kg/ontology/action/unwrap -->


    <owl:NamedIndividual rdf:about="http://example.org/virtualhome2kg/ontology/action/unwrap">
        <rdf:type rdf:resource="http://example.org/virtualhome2kg/ontology/Action"/>
    </owl:NamedIndividual>
    


    <!-- http://example.org/virtualhome2kg/ontology/action/vacuum -->


    <owl:NamedIndividual rdf:about="http://example.org/virtualhome2kg/ontology/action/vacuum">
        <rdf:type rdf:resource="http://example.org/virtualhome2kg/ontology/Action"/>
    </owl:NamedIndividual>
    


    <!-- http://example.org/virtualhome2kg/ontology/action/wait -->


    <owl:NamedIndividual rdf:about="http://example.org/virtualhome2kg/ontology/action/wait">
        <rdf:type rdf:resource="http://example.org/virtualhome2kg/ontology/Action"/>
    </owl:NamedIndividual>
    


    <!-- http://example.org/virtualhome2kg/ontology/action/wakeUp -->


    <owl:NamedIndividual rdf:about="http://example.org/virtualhome2kg/ontology/action/wakeUp">
        <rdf:type rdf:resource="http://example.org/virtualhome2kg/ontology/Action"/>
    </owl:NamedIndividual>
    


    <!-- http://example.org/virtualhome2kg/ontology/action/walk -->


    <owl:NamedIndividual rdf:about="http://example.org/virtualhome2kg/ontology/action/walk">
        <rdf:type rdf:resource="http://example.org/virtualhome2kg/ontology/Action"/>
    </owl:NamedIndividual>
    


    <!-- http://example.org/virtualhome2kg/ontology/action/watch -->


    <owl:NamedIndividual rdf:about="http://example.org/virtualhome2kg/ontology/action/watch">
        <rdf:type rdf:resource="http://example.org/virtualhome2kg/ontology/Action"/>
    </owl:NamedIndividual>
    


    <!-- http://example.org/virtualhome2kg/ontology/action/wipe -->


    <owl:NamedIndividual rdf:about="http://example.org/virtualhome2kg/ontology/action/wipe">
        <rdf:type rdf:resource="http://example.org/virtualhome2kg/ontology/Action"/>
    </owl:NamedIndividual>
    


    <!-- http://example.org/virtualhome2kg/ontology/action/wrap -->


    <owl:NamedIndividual rdf:about="http://example.org/virtualhome2kg/ontology/action/wrap">
        <rdf:type rdf:resource="http://example.org/virtualhome2kg/ontology/Action"/>
    </owl:NamedIndividual>
    


    <!-- http://example.org/virtualhome2kg/ontology/action/write -->


    <owl:NamedIndividual rdf:about="http://example.org/virtualhome2kg/ontology/action/write">
        <rdf:type rdf:resource="http://example.org/virtualhome2kg/ontology/Action"/>
    </owl:NamedIndividual>
    


    <!-- http://www.w3.org/2006/time#unitSecond -->


    <owl:NamedIndividual rdf:about="http://www.w3.org/2006/time#unitSecond">
        <rdf:type rdf:resource="http://www.w3.org/2006/time#TemporalUnit"/>
    </owl:NamedIndividual>
    


    <!-- 
    ///////////////////////////////////////////////////////////////////////////////////////
    //
    // Annotations
    //
    ///////////////////////////////////////////////////////////////////////////////////////
     -->


    <rdf:Description rdf:about="https://www.web3d.org/specifications/X3dOntology4.0#SFDouble">
        <terms:description>SFDouble is a double-precision floating-point type. Array values are optionally separated by commas in XML syntax. See GeoVRML 1.0 Recommended Practice, Section 2.3, Limitations of Single Precision for rationale.</terms:description>
    </rdf:Description>
    <rdf:Description rdf:about="https://www.web3d.org/specifications/X3dOntology4.0#SFVec3f">
        <terms:description>SFVec3d is a 3-tuple triplet of SFDouble values. See GeoVRML 1.0 Recommended Practice, Section 2.3, Limitations of Single Precision. Hint: SFVec3d can be used to specify a georeferenced 3D coordinate. Warning: comma characters within singleton values do not pass strict XML validation.</terms:description>
    </rdf:Description>
    


    <!-- 
    ///////////////////////////////////////////////////////////////////////////////////////
    //
    // General axioms
    //
    ///////////////////////////////////////////////////////////////////////////////////////
     -->


    <rdf:Description>
        <rdf:type rdf:resource="http://www.w3.org/2002/07/owl#AllDifferent"/>
        <owl:distinctMembers rdf:parseType="Collection">
            <rdf:Description rdf:about="http://example.org/virtualhome2kg/ontology/bright"/>
            <rdf:Description rdf:about="http://example.org/virtualhome2kg/ontology/cold"/>
            <rdf:Description rdf:about="http://example.org/virtualhome2kg/ontology/dark"/>
            <rdf:Description rdf:about="http://example.org/virtualhome2kg/ontology/deep"/>
            <rdf:Description rdf:about="http://example.org/virtualhome2kg/ontology/heavy"/>
            <rdf:Description rdf:about="http://example.org/virtualhome2kg/ontology/high"/>
            <rdf:Description rdf:about="http://example.org/virtualhome2kg/ontology/hot"/>
            <rdf:Description rdf:about="http://example.org/virtualhome2kg/ontology/long"/>
            <rdf:Description rdf:about="http://example.org/virtualhome2kg/ontology/low"/>
            <rdf:Description rdf:about="http://example.org/virtualhome2kg/ontology/shallow"/>
            <rdf:Description rdf:about="http://example.org/virtualhome2kg/ontology/short"/>
            <rdf:Description rdf:about="http://example.org/virtualhome2kg/ontology/thick"/>
            <rdf:Description rdf:about="http://example.org/virtualhome2kg/ontology/thin"/>
        </owl:distinctMembers>
    </rdf:Description>
</rdf:RDF>



<!-- Generated by the OWL API (version 5.1.18) https://github.com/owlcs/owlapi/ -->


